Prefix(:=<http://www.w3.org/ns/dcat#>)
Prefix(org:=<http://www.w3.org/ns/org#>)
Prefix(owl:=<http://www.w3.org/2002/07/owl#>)
Prefix(pav:=<http://purl.org/pav/>)
Prefix(rdf:=<http://www.w3.org/1999/02/22-rdf-syntax-ns#>)
Prefix(sdo:=<http://schema.org/>)
Prefix(xhv:=<http://www.w3.org/1999/xhtml/vocab#>)
Prefix(xml:=<http://www.w3.org/XML/1998/namespace>)
Prefix(xsd:=<http://www.w3.org/2001/XMLSchema#>)
Prefix(adms:=<http://www.w3.org/ns/adms#>)
Prefix(bibo:=<http://purl.org/ontology/bibo/>)
Prefix(dcat:=<http://www.w3.org/ns/dcat#>)
Prefix(foaf:=<http://xmlns.com/foaf/0.1/>)
Prefix(prov:=<http://www.w3.org/ns/prov#>)
Prefix(rdfs:=<http://www.w3.org/2000/01/rdf-schema#>)
Prefix(skos:=<http://www.w3.org/2004/02/skos/core#>)
Prefix(vann:=<http://purl.org/vocab/vann/>)
Prefix(vcard:=<http://www.w3.org/2006/vcard/ns#>)
Prefix(dctype:=<http://purl.org/dc/dcmitype/>)
Prefix(dcterms:=<http://purl.org/dc/terms/>)


Ontology(<http://www.w3.org/ns/dcat>
<http://www.w3.org/ns/dcat3>
Import(<http://www.w3.org/2004/02/skos/core>)
Import(<http://www.w3.org/ns/prov-o#>)
Annotation(dcterms:contributor _:genid2147483659)
Annotation(dcterms:creator <https://www.w3.org/groups/wg/dx>)
Annotation(dcterms:description "DCAT er et RDF-vokabular som har til formål at understøtte interoperabilitet mellem datakataloger udgivet på nettet. Ved at anvende DCAT til at beskrive datasæt i datakataloger, kan udgivere øge findbarhed og gøre det gøre det lettere for applikationer at anvende metadata fra forskellige kataloger. Derudover understøttes decentraliseret udstilling af kataloger og fødererede datasætsøgninger på tværs af websider. Aggregerede DCAT-metadata kan fungere som fortegnelsesfiler der kan understøtte digital bevaring. DCAT er defineret på http://www.w3.org/TR/vocab-dcat/. Enhver forskel mellem det normative dokument og dette schema er en fejl i dette schema."@da)
Annotation(dcterms:description "DCAT es un vocabulario RDF diseñado para facilitar la interoperabilidad entre catálogos de datos publicados en la Web. Utilizando DCAT para describir datos disponibles en catálogos se aumenta la posibilidad de que sean descubiertos y se permite que las aplicaciones consuman fácilmente los metadatos de varios catálogos."@es)
Annotation(dcterms:description "DCAT est un vocabulaire développé pour faciliter l'interopérabilité entre les jeux de données publiées sur le Web. En utilisant DCAT pour décrire les jeux de données dans les catalogues de données, les fournisseurs de données facilitent leur découverte et permettent que les applications consomment facilement les métadonnées de plusieurs catalogues. Il permet de plus la publication décentralisée des catalogues et facilite la recherche fédérée des données entre plusieurs sites. Les métadonnées DCAT aggrégées peuvent servir comme un manifeste pour faciliter la préservation digitale des ressources. DCAT est définie à l'adresse http://www.w3.org/TR/vocab-dcat/. Toute différence entre ce document normatif et le présent vocabulaire est une erreur dans le vocabulaire."@fr)
Annotation(dcterms:description "DCAT is an RDF vocabulary designed to facilitate interoperability between data catalogs published on the Web. By using DCAT to describe datasets in data catalogs, publishers increase discoverability and enable applications easily to consume metadata from multiple catalogs. It further enables decentralized publishing of catalogs and facilitates federated dataset search across sites. Aggregated DCAT metadata can serve as a manifest file to facilitate digital preservation. DCAT is defined at http://www.w3.org/TR/vocab-dcat/. Any variance between that normative document and this schema is an error in this schema."@en)
Annotation(dcterms:description "DCAT je RDF slovník navržený pro zprostředkování interoperability mezi datovými katalogy publikovanými na Webu. Poskytovatelé dat používáním slovníku DCAT pro popis datových sad v datových katalozích zvyšují jejich dohledatelnost a umožňují aplikacím konzumovat metadata z více katalogů. Dále je umožňena decentralizovaná publikace katalogů a federované dotazování na datové sady napříč katalogy. Agregovaná DCAT metadata mohou také sloužit jako průvodka umožňující digitální uchování informace. DCAT je definován na http://www.w3.org/TR/vocab-dcat/. Jakýkoliv nesoulad mezi odkazovaným dokumentem a tímto schématem je chybou v tomto schématu."@cs)
Annotation(dcterms:description "DCAT è un vocabolario RDF progettato per facilitare l'interoperabilità tra i cataloghi di dati pubblicati nel Web. Utilizzando DCAT per descrivere i dataset nei cataloghi di dati, i fornitori migliorano la capacità di individuazione dei dati e abilitano le  applicazioni al consumo di dati provenienti da cataloghi differenti. DCAT permette di decentralizzare la pubblicazione di cataloghi e facilita la ricerca federata dei dataset. L'aggregazione dei metadati federati può fungere da file manifesto per facilitare la conservazione digitale. DCAT è definito all'indirizzo http://www.w3.org/TR/vocab-dcat/. Qualsiasi scostamento tra tale definizione normativa e questo schema è da considerarsi un errore di questo schema."@it)
Annotation(dcterms:description "DCATは、ウェブ上で公開されたデータ・カタログ間の相互運用性の促進を目的とするRDFの語彙です。このドキュメントでは、その利用のために、スキーマを定義し、例を提供します。データ・カタログ内のデータセットを記述するためにDCATを用いると、公開者が、発見可能性を増加させ、アプリケーションが複数のカタログのメタデータを容易に利用できるようになります。さらに、カタログの分散公開を可能にし、複数のサイトにまたがるデータセットの統合検索を促進します。集約されたDCATメタデータは、ディジタル保存を促進するためのマニフェスト・ファイルとして使用できます。"@ja)
Annotation(dcterms:description "Το DCAT είναι ένα RDF λεξιλόγιο που σχεδιάσθηκε για να κάνει εφικτή τη διαλειτουργικότητα μεταξύ καταλόγων δεδομένων στον Παγκόσμιο Ιστό. Χρησιμοποιώντας το DCAT για την περιγραφή συνόλων δεδομένων, οι εκδότες αυτών αυξάνουν την ανακαλυψιμότητα και επιτρέπουν στις εφαρμογές την εύκολη κατανάλωση μεταδεδομένων από πολλαπλούς καταλόγους. Επιπλέον, δίνει τη δυνατότητα για αποκεντρωμένη έκδοση και διάθεση καταλόγων και επιτρέπει δυνατότητες ενοποιημένης αναζήτησης μεταξύ διαφορετικών πηγών. Συγκεντρωτικά μεταδεδομένα που έχουν περιγραφεί με το DCAT μπορούν να χρησιμοποιηθούν σαν ένα δηλωτικό αρχείο (manifest file) ώστε να διευκολύνουν την ψηφιακή συντήρηση."@el)
Annotation(dcterms:description "هي أنطولوجية تسهل تبادل البيانات بين مختلف الفهارس على الوب. استخدام هذه الأنطولوجية يساعد على اكتشاف قوائم  البيانات المنشورة على الوب و يمكن التطبيقات المختلفة من الاستفادة أتوماتيكيا من البيانات المتاحة من مختلف الفهارس."@ar)
Annotation(dcterms:license <https://creativecommons.org/licenses/by/4.0/>)
Annotation(dcterms:publisher _:genid2147483660)
Annotation(dcterms:title "Datakatalogvokabular"@da)
Annotation(dcterms:title "El vocabulario de catálogo de datos"@es)
Annotation(dcterms:title "Il vocabolario del catalogo dei dati"@it)
Annotation(dcterms:title "Le vocabulaire des catalogues de données"@fr)
Annotation(dcterms:title "Slovník pro datové katalogy"@cs)
Annotation(dcterms:title "The data catalog vocabulary"@en)
Annotation(dcterms:title "Το λεξιλόγιο των καταλόγων δεδομένων"@el)
Annotation(dcterms:title "أنطولوجية فهارس قوائم البيانات"@ar)
Annotation(dcterms:title "データ・カタログ語彙（DCAT）"@ja)
Annotation(bibo:editor _:genid2147483648)
Annotation(bibo:editor _:genid2147483649)
Annotation(bibo:editor _:genid2147483650)
Annotation(bibo:editor _:genid2147483651)
Annotation(bibo:editor _:genid2147483652)
Annotation(bibo:editor _:genid2147483653)
Annotation(bibo:translator _:genid2147483654)
Annotation(bibo:translator _:genid2147483655)
Annotation(bibo:translator _:genid2147483656)
Annotation(bibo:translator _:genid2147483657)
Annotation(bibo:translator _:genid2147483658)
Annotation(vann:preferredNamespacePrefix "dcat")
Annotation(vann:preferredNamespaceUri "http://www.w3.org/ns/dcat#")
Annotation(rdfs:comment "DCAT er et RDF-vokabular som har til formål at understøtte interoperabilitet mellem datakataloger udgivet på nettet. Ved at anvende DCAT til at beskrive datasæt i datakataloger, kan udgivere øge findbarhed og gøre det gøre det lettere for applikationer at anvende metadata fra forskellige kataloger. Derudover understøttes decentraliseret udstilling af kataloger og fødererede datasætsøgninger på tværs af websider. Aggregerede DCAT-metadata kan fungere som fortegnelsesfiler der kan understøtte digital bevaring. DCAT er defineret på http://www.w3.org/TR/vocab-dcat/. Enhver forskel mellem det normative dokument og dette schema er en fejl i dette schema."@da)
Annotation(rdfs:comment "DCAT es un vocabulario RDF diseñado para facilitar la interoperabilidad entre catálogos de datos publicados en la Web. Utilizando DCAT para describir datos disponibles en catálogos se aumenta la posibilidad de que sean descubiertos y se permite que las aplicaciones consuman fácilmente los metadatos de varios catálogos."@es)
Annotation(rdfs:comment "DCAT est un vocabulaire développé pour faciliter l'interopérabilité entre les jeux de données publiées sur le Web. En utilisant DCAT pour décrire les jeux de données dans les catalogues de données, les fournisseurs de données facilitent leur découverte et permettent que les applications consomment facilement les métadonnées de plusieurs catalogues. Il permet de plus la publication décentralisée des catalogues et facilite la recherche fédérée des données entre plusieurs sites. Les métadonnées DCAT aggrégées peuvent servir comme un manifeste pour faciliter la préservation digitale des ressources. DCAT est définie à l'adresse http://www.w3.org/TR/vocab-dcat/. Toute différence entre ce document normatif et le présent vocabulaire est une erreur dans le vocabulaire."@fr)
Annotation(rdfs:comment "DCAT is an RDF vocabulary designed to facilitate interoperability between data catalogs published on the Web. By using DCAT to describe datasets in data catalogs, publishers increase discoverability and enable applications easily to consume metadata from multiple catalogs. It further enables decentralized publishing of catalogs and facilitates federated dataset search across sites. Aggregated DCAT metadata can serve as a manifest file to facilitate digital preservation. DCAT is defined at http://www.w3.org/TR/vocab-dcat/. Any variance between that normative document and this schema is an error in this schema."@en)
Annotation(rdfs:comment "DCAT je RDF slovník navržený pro zprostředkování interoperability mezi datovými katalogy publikovanými na Webu. Poskytovatelé dat používáním slovníku DCAT pro popis datových sad v datových katalozích zvyšují jejich dohledatelnost a umožňují aplikacím konzumovat metadata z více katalogů. Dále je umožňena decentralizovaná publikace katalogů a federované dotazování na datové sady napříč katalogy. Agregovaná DCAT metadata mohou také sloužit jako průvodka umožňující digitální uchování informace. DCAT je definován na http://www.w3.org/TR/vocab-dcat/. Jakýkoliv nesoulad mezi odkazovaným dokumentem a tímto schématem je chybou v tomto schématu."@cs)
Annotation(rdfs:comment "DCAT è un vocabolario RDF progettato per facilitare l'interoperabilità tra i cataloghi di dati pubblicati nel Web. Utilizzando DCAT per descrivere i dataset nei cataloghi di dati, i fornitori migliorano la capacità di individuazione dei dati e abilitano le  applicazioni al consumo di dati provenienti da cataloghi differenti. DCAT permette di decentralizzare la pubblicazione di cataloghi e facilita la ricerca federata dei dataset. L'aggregazione dei metadati federati può fungere da file manifesto per facilitare la conservazione digitale. DCAT è definito all'indirizzo http://www.w3.org/TR/vocab-dcat/. Qualsiasi scostamento tra tale definizione normativa e questo schema è da considerarsi un errore di questo schema."@it)
Annotation(rdfs:comment "DCATは、ウェブ上で公開されたデータ・カタログ間の相互運用性の促進を目的とするRDFの語彙です。このドキュメントでは、その利用のために、スキーマを定義し、例を提供します。データ・カタログ内のデータセットを記述するためにDCATを用いると、公開者が、発見可能性を増加させ、アプリケーションが複数のカタログのメタデータを容易に利用できるようになります。さらに、カタログの分散公開を可能にし、複数のサイトにまたがるデータセットの統合検索を促進します。集約されたDCATメタデータは、ディジタル保存を促進するためのマニフェスト・ファイルとして使用できます。"@ja)
Annotation(rdfs:comment "Το DCAT είναι ένα RDF λεξιλόγιο που σχεδιάσθηκε για να κάνει εφικτή τη διαλειτουργικότητα μεταξύ καταλόγων δεδομένων στον Παγκόσμιο Ιστό. Χρησιμοποιώντας το DCAT για την περιγραφή συνόλων δεδομένων, οι εκδότες αυτών αυξάνουν την ανακαλυψιμότητα και επιτρέπουν στις εφαρμογές την εύκολη κατανάλωση μεταδεδομένων από πολλαπλούς καταλόγους. Επιπλέον, δίνει τη δυνατότητα για αποκεντρωμένη έκδοση και διάθεση καταλόγων και επιτρέπει δυνατότητες ενοποιημένης αναζήτησης μεταξύ διαφορετικών πηγών. Συγκεντρωτικά μεταδεδομένα που έχουν περιγραφεί με το DCAT μπορούν να χρησιμοποιηθούν σαν ένα δηλωτικό αρχείο (manifest file) ώστε να διευκολύνουν την ψηφιακή συντήρηση."@el)
Annotation(rdfs:comment "هي أنطولوجية تسهل تبادل البيانات بين مختلف الفهارس على الوب. استخدام هذه الأنطولوجية يساعد على اكتشاف قوائم  البيانات المنشورة على الوب و يمكن التطبيقات المختلفة من الاستفادة أتوماتيكيا من البيانات المتاحة من مختلف الفهارس."@ar)
Annotation(rdfs:label "Datakatalogvokabular"@da)
Annotation(rdfs:label "El vocabulario de catálogo de datos"@es)
Annotation(rdfs:label "Il vocabolario del catalogo dei dati"@it)
Annotation(rdfs:label "Le vocabulaire des jeux de données"@fr)
Annotation(rdfs:label "Slovník pro datové katalogy"@cs)
Annotation(rdfs:label "The data catalog vocabulary"@en)
Annotation(rdfs:label "Το λεξιλόγιο των καταλόγων δεδομένων"@el)
Annotation(rdfs:label "أنطولوجية فهارس قوائم البيانات"@ar)
Annotation(rdfs:label "データ・カタログ語彙（DCAT）"@ja)
Annotation(owl:backwardCompatibleWith <http://www.w3.org/ns/dcat2>)
Annotation(owl:backwardCompatibleWith <http://www.w3.org/ns/dcat2014>)
Annotation(owl:priorVersion <http://www.w3.org/ns/dcat2>)
Annotation(owl:versionInfo "3")
Annotation(skos:editorialNote "English language definitions updated in this revision in line with ED. Multilingual text unevenly updated."@en)
Annotation(adms:versionNotes "Dette er en opdateret kopi af DCAT 3 som er tilgænglig på https://www.w3.org/ns/dcat.ttl"@da)
Annotation(adms:versionNotes "Esta es una copia del vocabulario DCAT 3 disponible en https://www.w3.org/ns/dcat.ttl"@es)
Annotation(adms:versionNotes "Questa è una copia aggiornata del vocabolario DCAT 3 disponibile in https://www.w3.org/ns/dcat.ttl"@it)
Annotation(adms:versionNotes "This is an updated copy of the DCAT 3 vocabulary, taken from https://www.w3.org/ns/dcat.ttl"@en)
Annotation(adms:versionNotes "Toto je aktualizovaná kopie slovníku DCAT 3, převzatá z https://www.w3.org/ns/dcat.ttl"@cs)
Annotation(foaf:depiction <https://www.w3.org/TR/vocab-dcat-3/images/dcat-all-attributes.svg>)

Declaration(Class(<http://purl.org/dc/dcam/VocabularyEncodingScheme>))
Declaration(Class(dctype:Service))
Declaration(Class(dcterms:Agent))
Declaration(Class(dcterms:AgentClass))
Declaration(Class(dcterms:BibliographicResource))
Declaration(Class(dcterms:FileFormat))
Declaration(Class(dcterms:Frequency))
Declaration(Class(dcterms:Jurisdiction))
Declaration(Class(dcterms:LicenseDocument))
Declaration(Class(dcterms:LinguisticSystem))
Declaration(Class(dcterms:Location))
Declaration(Class(dcterms:LocationPeriodOrJurisdiction))
Declaration(Class(dcterms:MediaType))
Declaration(Class(dcterms:MediaTypeOrExtent))
Declaration(Class(dcterms:MethodOfAccrual))
Declaration(Class(dcterms:MethodOfInstruction))
Declaration(Class(dcterms:PeriodOfTime))
Declaration(Class(dcterms:PhysicalMedium))
Declaration(Class(dcterms:PhysicalResource))
Declaration(Class(dcterms:Policy))
Declaration(Class(dcterms:ProvenanceStatement))
Declaration(Class(dcterms:RightsStatement))
Declaration(Class(dcterms:SizeOrDuration))
Declaration(Class(dcterms:Standard))
Declaration(Class(rdf:List))
Declaration(Class(rdfs:Class))
Declaration(Class(rdfs:Resource))
Declaration(Class(vcard:Kind))
Declaration(Class(dcat:Catalog))
Declaration(Class(dcat:CatalogRecord))
Declaration(Class(dcat:DataService))
Declaration(Class(dcat:Dataset))
Declaration(Class(dcat:DatasetSeries))
Declaration(Class(dcat:Distribution))
Declaration(Class(dcat:Relationship))
Declaration(Class(dcat:Resource))
Declaration(Class(dcat:Role))
Declaration(Class(org:Organization))
Declaration(Class(foaf:Document))
Declaration(Class(foaf:Person))
Declaration(ObjectProperty(pav:hasVersion))
Declaration(ObjectProperty(xhv:first))
Declaration(ObjectProperty(xhv:last))
Declaration(ObjectProperty(xhv:prev))
Declaration(ObjectProperty(dcat:accessService))
Declaration(ObjectProperty(dcat:accessURL))
Declaration(ObjectProperty(dcat:catalog))
Declaration(ObjectProperty(dcat:compressFormat))
Declaration(ObjectProperty(dcat:contactPoint))
Declaration(ObjectProperty(dcat:dataset))
Declaration(ObjectProperty(dcat:distribution))
Declaration(ObjectProperty(dcat:downloadURL))
Declaration(ObjectProperty(dcat:endpointDescription))
Declaration(ObjectProperty(dcat:endpointURL))
Declaration(ObjectProperty(dcat:first))
Declaration(ObjectProperty(dcat:hadRole))
Declaration(ObjectProperty(dcat:hasCurrentVersion))
Declaration(ObjectProperty(dcat:hasVersion))
Declaration(ObjectProperty(dcat:inCatalog))
Declaration(ObjectProperty(dcat:inSeries))
Declaration(ObjectProperty(dcat:isDistributionOf))
Declaration(ObjectProperty(dcat:isVersionOf))
Declaration(ObjectProperty(dcat:landingPage))
Declaration(ObjectProperty(dcat:last))
Declaration(ObjectProperty(dcat:mediaType))
Declaration(ObjectProperty(dcat:next))
Declaration(ObjectProperty(dcat:nextVersion))
Declaration(ObjectProperty(dcat:packageFormat))
Declaration(ObjectProperty(dcat:prev))
Declaration(ObjectProperty(dcat:previousVersion))
Declaration(ObjectProperty(dcat:qualifiedRelation))
Declaration(ObjectProperty(dcat:record))
Declaration(ObjectProperty(dcat:resource))
Declaration(ObjectProperty(dcat:seriesMember))
Declaration(ObjectProperty(dcat:servesDataset))
Declaration(ObjectProperty(dcat:service))
Declaration(ObjectProperty(dcat:theme))
Declaration(ObjectProperty(dcat:themeTaxonomy))
Declaration(ObjectProperty(prov:generalizationOf))
Declaration(ObjectProperty(foaf:homepage))
Declaration(ObjectProperty(foaf:page))
Declaration(ObjectProperty(foaf:primaryTopic))
Declaration(DataProperty(dcat:bbox))
Declaration(DataProperty(dcat:byteSize))
Declaration(DataProperty(dcat:centroid))
Declaration(DataProperty(dcat:endDate))
Declaration(DataProperty(dcat:keyword))
Declaration(DataProperty(dcat:spatialResolutionInMeters))
Declaration(DataProperty(dcat:startDate))
Declaration(DataProperty(dcat:temporalResolution))
Declaration(DataProperty(dcat:version))
Declaration(NamedIndividual(<http://stfc.ac.uk>))
Declaration(NamedIndividual(<http://ec.europa.eu/dgs/informatics/>))
Declaration(NamedIndividual(<http://makxdekkers.com/>))
Declaration(NamedIndividual(<http://purl.org/dc/terms/>))
Declaration(NamedIndividual(dcterms:Agent))
Declaration(NamedIndividual(dcterms:AgentClass))
Declaration(NamedIndividual(dcterms:BibliographicResource))
Declaration(NamedIndividual(dcterms:Box))
Declaration(NamedIndividual(dcterms:DCMIType))
Declaration(NamedIndividual(dcterms:DDC))
Declaration(NamedIndividual(dcterms:FileFormat))
Declaration(NamedIndividual(dcterms:Frequency))
Declaration(NamedIndividual(dcterms:IMT))
Declaration(NamedIndividual(dcterms:ISO3166))
Declaration(NamedIndividual(dcterms:ISO639-2))
Declaration(NamedIndividual(dcterms:ISO639-3))
Declaration(NamedIndividual(dcterms:Jurisdiction))
Declaration(NamedIndividual(dcterms:LCC))
Declaration(NamedIndividual(dcterms:LCSH))
Declaration(NamedIndividual(dcterms:LicenseDocument))
Declaration(NamedIndividual(dcterms:LinguisticSystem))
Declaration(NamedIndividual(dcterms:Location))
Declaration(NamedIndividual(dcterms:LocationPeriodOrJurisdiction))
Declaration(NamedIndividual(dcterms:MESH))
Declaration(NamedIndividual(dcterms:MediaType))
Declaration(NamedIndividual(dcterms:MediaTypeOrExtent))
Declaration(NamedIndividual(dcterms:MethodOfAccrual))
Declaration(NamedIndividual(dcterms:MethodOfInstruction))
Declaration(NamedIndividual(dcterms:NLM))
Declaration(NamedIndividual(dcterms:Period))
Declaration(NamedIndividual(dcterms:PeriodOfTime))
Declaration(NamedIndividual(dcterms:PhysicalMedium))
Declaration(NamedIndividual(dcterms:PhysicalResource))
Declaration(NamedIndividual(dcterms:Point))
Declaration(NamedIndividual(dcterms:Policy))
Declaration(NamedIndividual(dcterms:ProvenanceStatement))
Declaration(NamedIndividual(dcterms:RFC1766))
Declaration(NamedIndividual(dcterms:RFC3066))
Declaration(NamedIndividual(dcterms:RFC4646))
Declaration(NamedIndividual(dcterms:RFC5646))
Declaration(NamedIndividual(dcterms:RightsStatement))
Declaration(NamedIndividual(dcterms:SizeOrDuration))
Declaration(NamedIndividual(dcterms:Standard))
Declaration(NamedIndividual(dcterms:TGN))
Declaration(NamedIndividual(dcterms:UDC))
Declaration(NamedIndividual(dcterms:URI))
Declaration(NamedIndividual(dcterms:W3CDTF))
Declaration(NamedIndividual(dcterms:abstract))
Declaration(NamedIndividual(dcterms:accessRights))
Declaration(NamedIndividual(dcterms:accrualMethod))
Declaration(NamedIndividual(dcterms:accrualPeriodicity))
Declaration(NamedIndividual(dcterms:accrualPolicy))
Declaration(NamedIndividual(dcterms:audience))
Declaration(NamedIndividual(dcterms:conformsTo))
Declaration(NamedIndividual(dcterms:contributor))
Declaration(NamedIndividual(dcterms:coverage))
Declaration(NamedIndividual(dcterms:creator))
Declaration(NamedIndividual(dcterms:description))
Declaration(NamedIndividual(dcterms:educationLevel))
Declaration(NamedIndividual(dcterms:extent))
Declaration(NamedIndividual(dcterms:hasFormat))
Declaration(NamedIndividual(dcterms:instructionalMethod))
Declaration(NamedIndividual(dcterms:isFormatOf))
Declaration(NamedIndividual(dcterms:isReferencedBy))
Declaration(NamedIndividual(dcterms:isReplacedBy))
Declaration(NamedIndividual(dcterms:isRequiredBy))
Declaration(NamedIndividual(dcterms:isVersionOf))
Declaration(NamedIndividual(dcterms:language))
Declaration(NamedIndividual(dcterms:license))
Declaration(NamedIndividual(dcterms:mediator))
Declaration(NamedIndividual(dcterms:medium))
Declaration(NamedIndividual(dcterms:provenance))
Declaration(NamedIndividual(dcterms:publisher))
Declaration(NamedIndividual(dcterms:references))
Declaration(NamedIndividual(dcterms:replaces))
Declaration(NamedIndividual(dcterms:requires))
Declaration(NamedIndividual(dcterms:rights))
Declaration(NamedIndividual(dcterms:rightsHolder))
Declaration(NamedIndividual(dcterms:source))
Declaration(NamedIndividual(dcterms:spatial))
Declaration(NamedIndividual(dcterms:tableOfContents))
Declaration(NamedIndividual(dcterms:temporal))
Declaration(NamedIndividual(dcterms:type))
Declaration(NamedIndividual(<http://www.asahi-net.or.jp/~ax2s-kmtn/>))
Declaration(NamedIndividual(<http://www.deri.ie/>))
Declaration(NamedIndividual(<http://www.w3.org/ns/dcat>))
Declaration(NamedIndividual(<http://www.w3.org/ns/dcat2>))
Declaration(NamedIndividual(<http://www.w3.org/ns/dcat2014>))
Declaration(NamedIndividual(<http://www.w3.org/ns/dcat3>))
Declaration(NamedIndividual(<http://www.w3.org/ns/prov-o>))
Declaration(NamedIndividual(<http://www.w3.org/ns/prov-o-20130312>))
Declaration(NamedIndividual(<http://www.w3.org/ns/prov-o#>))
Declaration(NamedIndividual(<https://agbeltran.github.io>))
Declaration(NamedIndividual(<https://www.csiro.au>))
Declaration(NamedIndividual(<https://jakub.klímek.com/>))
Declaration(NamedIndividual(<https://w3id.org/people/ralbertoni/>))
Declaration(NamedIndividual(<https://www.w3.org/>))
Declaration(AnnotationProperty(<http://purl.org/dc/dcam/domainIncludes>))
Declaration(AnnotationProperty(<http://purl.org/dc/dcam/rangeIncludes>))
Declaration(AnnotationProperty(<http://purl.org/dc/elements/1.1/contributor>))
Declaration(AnnotationProperty(<http://purl.org/dc/elements/1.1/coverage>))
Declaration(AnnotationProperty(<http://purl.org/dc/elements/1.1/creator>))
Declaration(AnnotationProperty(<http://purl.org/dc/elements/1.1/date>))
Declaration(AnnotationProperty(<http://purl.org/dc/elements/1.1/description>))
Declaration(AnnotationProperty(<http://purl.org/dc/elements/1.1/format>))
Declaration(AnnotationProperty(<http://purl.org/dc/elements/1.1/identifier>))
Declaration(AnnotationProperty(<http://purl.org/dc/elements/1.1/language>))
Declaration(AnnotationProperty(<http://purl.org/dc/elements/1.1/publisher>))
Declaration(AnnotationProperty(<http://purl.org/dc/elements/1.1/relation>))
Declaration(AnnotationProperty(<http://purl.org/dc/elements/1.1/rights>))
Declaration(AnnotationProperty(<http://purl.org/dc/elements/1.1/source>))
Declaration(AnnotationProperty(<http://purl.org/dc/elements/1.1/subject>))
Declaration(AnnotationProperty(<http://purl.org/dc/elements/1.1/title>))
Declaration(AnnotationProperty(<http://purl.org/dc/elements/1.1/type>))
Declaration(AnnotationProperty(dcterms:abstract))
Declaration(AnnotationProperty(dcterms:accessRights))
Declaration(AnnotationProperty(dcterms:accrualMethod))
Declaration(AnnotationProperty(dcterms:accrualPeriodicity))
Declaration(AnnotationProperty(dcterms:accrualPolicy))
Declaration(AnnotationProperty(dcterms:audience))
Declaration(AnnotationProperty(dcterms:conformsTo))
Declaration(AnnotationProperty(dcterms:contributor))
Declaration(AnnotationProperty(dcterms:coverage))
Declaration(AnnotationProperty(dcterms:creator))
Declaration(AnnotationProperty(dcterms:description))
Declaration(AnnotationProperty(dcterms:educationLevel))
Declaration(AnnotationProperty(dcterms:extent))
Declaration(AnnotationProperty(dcterms:hasFormat))
Declaration(AnnotationProperty(dcterms:isFormatOf))
Declaration(AnnotationProperty(dcterms:isReferencedBy))
Declaration(AnnotationProperty(dcterms:isReplacedBy))
Declaration(AnnotationProperty(dcterms:isRequiredBy))
Declaration(AnnotationProperty(dcterms:isVersionOf))
Declaration(AnnotationProperty(dcterms:language))
Declaration(AnnotationProperty(dcterms:license))
Declaration(AnnotationProperty(dcterms:mediator))
Declaration(AnnotationProperty(dcterms:medium))
Declaration(AnnotationProperty(dcterms:publisher))
Declaration(AnnotationProperty(dcterms:references))
Declaration(AnnotationProperty(dcterms:replaces))
Declaration(AnnotationProperty(dcterms:requires))
Declaration(AnnotationProperty(dcterms:rights))
Declaration(AnnotationProperty(dcterms:source))
Declaration(AnnotationProperty(dcterms:spatial))
Declaration(AnnotationProperty(dcterms:tableOfContents))
Declaration(AnnotationProperty(dcterms:temporal))
Declaration(AnnotationProperty(dcterms:type))
Declaration(AnnotationProperty(bibo:editor))
Declaration(AnnotationProperty(bibo:translator))
Declaration(AnnotationProperty(vann:preferredNamespacePrefix))
Declaration(AnnotationProperty(vann:preferredNamespaceUri))
Declaration(AnnotationProperty(sdo:rangeIncludes))
Declaration(AnnotationProperty(adms:versionNotes))
Declaration(AnnotationProperty(org:memberOf))
Declaration(AnnotationProperty(foaf:depiction))
Declaration(AnnotationProperty(foaf:name))
Declaration(AnnotationProperty(foaf:workInfoHomepage))
Declaration(Datatype(dcterms:Box))
Declaration(Datatype(dcterms:ISO3166))
Declaration(Datatype(dcterms:ISO639-2))
Declaration(Datatype(dcterms:ISO639-3))
Declaration(Datatype(dcterms:Period))
Declaration(Datatype(dcterms:Point))
Declaration(Datatype(dcterms:RFC1766))
Declaration(Datatype(dcterms:RFC3066))
Declaration(Datatype(dcterms:RFC4646))
Declaration(Datatype(dcterms:RFC5646))
Declaration(Datatype(dcterms:URI))
Declaration(Datatype(dcterms:W3CDTF))
Declaration(Datatype(xsd:date))
Declaration(Datatype(xsd:duration))
############################
#   Annotation Properties
############################

# Annotation Property: dcterms:abstract (Abstract)

AnnotationAssertion(rdfs:comment dcterms:abstract "A summary of the resource."@en)
AnnotationAssertion(rdfs:isDefinedBy dcterms:abstract <http://purl.org/dc/terms/>)
AnnotationAssertion(rdfs:label dcterms:abstract "Abstract"@en)
SubAnnotationPropertyOf(dcterms:abstract <http://purl.org/dc/elements/1.1/description>)
SubAnnotationPropertyOf(dcterms:abstract dcterms:description)

# Annotation Property: dcterms:accessRights (Access Rights)

AnnotationAssertion(<http://purl.org/dc/dcam/rangeIncludes> dcterms:accessRights dcterms:RightsStatement)
AnnotationAssertion(dcterms:description dcterms:accessRights "Access Rights may include information regarding access or restrictions based on privacy, security, or other policies."@en)
AnnotationAssertion(rdfs:comment dcterms:accessRights "Information about who access the resource or an indication of its security status."@en)
AnnotationAssertion(rdfs:isDefinedBy dcterms:accessRights <http://purl.org/dc/terms/>)
AnnotationAssertion(rdfs:label dcterms:accessRights "Access Rights"@en)
SubAnnotationPropertyOf(dcterms:accessRights <http://purl.org/dc/elements/1.1/rights>)
SubAnnotationPropertyOf(dcterms:accessRights dcterms:rights)

# Annotation Property: dcterms:accrualMethod (Accrual Method)

AnnotationAssertion(<http://purl.org/dc/dcam/rangeIncludes> dcterms:accrualMethod dcterms:MethodOfAccrual)
AnnotationAssertion(dcterms:description dcterms:accrualMethod "Recommended practice is to use a value from the Collection Description Accrual Method Vocabulary [[DCMI-ACCRUALMETHOD](https://dublincore.org/groups/collections/accrual-method/)]."@en)
AnnotationAssertion(rdfs:comment dcterms:accrualMethod "The method by which items are added to a collection."@en)
AnnotationAssertion(rdfs:isDefinedBy dcterms:accrualMethod <http://purl.org/dc/terms/>)
AnnotationAssertion(rdfs:label dcterms:accrualMethod "Accrual Method"@en)
AnnotationPropertyDomain(dcterms:accrualMethod dctype:Collection)

# Annotation Property: dcterms:accrualPeriodicity (Accrual Periodicity)

AnnotationAssertion(<http://purl.org/dc/dcam/rangeIncludes> dcterms:accrualPeriodicity dcterms:Frequency)
AnnotationAssertion(dcterms:description dcterms:accrualPeriodicity "Recommended practice is to use a value from the Collection Description Frequency Vocabulary [[DCMI-COLLFREQ](https://dublincore.org/groups/collections/frequency/)]."@en)
AnnotationAssertion(rdfs:comment dcterms:accrualPeriodicity "The frequency with which items are added to a collection."@en)
AnnotationAssertion(rdfs:isDefinedBy dcterms:accrualPeriodicity <http://purl.org/dc/terms/>)
AnnotationAssertion(rdfs:label dcterms:accrualPeriodicity "Accrual Periodicity"@en)
AnnotationPropertyDomain(dcterms:accrualPeriodicity dctype:Collection)

# Annotation Property: dcterms:accrualPolicy (Accrual Policy)

AnnotationAssertion(<http://purl.org/dc/dcam/rangeIncludes> dcterms:accrualPolicy dcterms:Policy)
AnnotationAssertion(dcterms:description dcterms:accrualPolicy "Recommended practice is to use a value from the Collection Description Accrual Policy Vocabulary [[DCMI-ACCRUALPOLICY](https://dublincore.org/groups/collections/accrual-policy/)]."@en)
AnnotationAssertion(rdfs:comment dcterms:accrualPolicy "The policy governing the addition of items to a collection."@en)
AnnotationAssertion(rdfs:isDefinedBy dcterms:accrualPolicy <http://purl.org/dc/terms/>)
AnnotationAssertion(rdfs:label dcterms:accrualPolicy "Accrual Policy"@en)
AnnotationPropertyDomain(dcterms:accrualPolicy dctype:Collection)

# Annotation Property: dcterms:alternative (Alternative Title)

AnnotationAssertion(dcterms:description dcterms:alternative "The distinction between titles and alternative titles is application-specific."@en)
AnnotationAssertion(rdfs:comment dcterms:alternative "An alternative name for the resource."@en)
AnnotationAssertion(rdfs:isDefinedBy dcterms:alternative <http://purl.org/dc/terms/>)
AnnotationAssertion(rdfs:label dcterms:alternative "Alternative Title"@en)
SubAnnotationPropertyOf(dcterms:alternative <http://purl.org/dc/elements/1.1/title>)

# Annotation Property: dcterms:audience (Audience)

AnnotationAssertion(<http://purl.org/dc/dcam/rangeIncludes> dcterms:audience dcterms:AgentClass)
AnnotationAssertion(dcterms:description dcterms:audience "Recommended practice is to use this property with non-literal values from a vocabulary of audience types."@en)
AnnotationAssertion(rdfs:comment dcterms:audience "A class of agents for whom the resource is intended or useful."@en)
AnnotationAssertion(rdfs:isDefinedBy dcterms:audience <http://purl.org/dc/terms/>)
AnnotationAssertion(rdfs:label dcterms:audience "Audience"@en)

# Annotation Property: dcterms:available (Date Available)

AnnotationAssertion(dcterms:description dcterms:available "Recommended practice is to describe the date, date/time, or period of time as recommended for the property Date, of which this is a subproperty."@en)
AnnotationAssertion(rdfs:comment dcterms:available "Date that the resource became or will become available."@en)
AnnotationAssertion(rdfs:isDefinedBy dcterms:available <http://purl.org/dc/terms/>)
AnnotationAssertion(rdfs:label dcterms:available "Date Available"@en)
SubAnnotationPropertyOf(dcterms:available <http://purl.org/dc/elements/1.1/date>)

# Annotation Property: dcterms:bibliographicCitation (Bibliographic Citation)

AnnotationAssertion(dcterms:description dcterms:bibliographicCitation "Recommended practice is to include sufficient bibliographic detail to identify the resource as unambiguously as possible."@en)
AnnotationAssertion(rdfs:comment dcterms:bibliographicCitation "A bibliographic reference for the resource."@en)
AnnotationAssertion(rdfs:isDefinedBy dcterms:bibliographicCitation <http://purl.org/dc/terms/>)
AnnotationAssertion(rdfs:label dcterms:bibliographicCitation "Bibliographic Citation"@en)
SubAnnotationPropertyOf(dcterms:bibliographicCitation <http://purl.org/dc/elements/1.1/identifier>)

# Annotation Property: dcterms:conformsTo (Conforms To)

AnnotationAssertion(<http://purl.org/dc/dcam/rangeIncludes> dcterms:conformsTo dcterms:Standard)
AnnotationAssertion(rdfs:comment dcterms:conformsTo "An established standard to which the described resource conforms."@en)
AnnotationAssertion(rdfs:isDefinedBy dcterms:conformsTo <http://purl.org/dc/terms/>)
AnnotationAssertion(rdfs:label dcterms:conformsTo "Conforms To"@en)
SubAnnotationPropertyOf(dcterms:conformsTo <http://purl.org/dc/elements/1.1/relation>)
SubAnnotationPropertyOf(dcterms:conformsTo dcterms:relation)

# Annotation Property: dcterms:contributor (Contributor)

AnnotationAssertion(<http://purl.org/dc/dcam/rangeIncludes> dcterms:contributor dcterms:Agent)
AnnotationAssertion(dcterms:description dcterms:contributor "The guidelines for using names of persons or organizations as creators apply to contributors."@en)
AnnotationAssertion(rdfs:comment dcterms:contributor "An entity responsible for making contributions to the resource."@en)
AnnotationAssertion(rdfs:isDefinedBy dcterms:contributor <http://purl.org/dc/terms/>)
AnnotationAssertion(rdfs:label dcterms:contributor "Contributor"@en)
SubAnnotationPropertyOf(dcterms:contributor <http://purl.org/dc/elements/1.1/contributor>)

# Annotation Property: dcterms:coverage (Coverage)

AnnotationAssertion(<http://purl.org/dc/dcam/rangeIncludes> dcterms:coverage dcterms:Jurisdiction)
AnnotationAssertion(<http://purl.org/dc/dcam/rangeIncludes> dcterms:coverage dcterms:Location)
AnnotationAssertion(<http://purl.org/dc/dcam/rangeIncludes> dcterms:coverage dcterms:Period)
AnnotationAssertion(dcterms:description dcterms:coverage "Spatial topic and spatial applicability may be a named place or a location specified by its geographic coordinates. Temporal topic may be a named period, date, or date range. A jurisdiction may be a named administrative entity or a geographic place to which the resource applies. Recommended practice is to use a controlled vocabulary such as the Getty Thesaurus of Geographic Names [[TGN](https://www.getty.edu/research/tools/vocabulary/tgn/index.html)]. Where appropriate, named places or time periods may be used in preference to numeric identifiers such as sets of coordinates or date ranges.  Because coverage is so broadly defined, it is preferable to use the more specific subproperties Temporal Coverage and Spatial Coverage."@en)
AnnotationAssertion(rdfs:comment dcterms:coverage "The spatial or temporal topic of the resource, spatial applicability of the resource, or jurisdiction under which the resource is relevant."@en)
AnnotationAssertion(rdfs:isDefinedBy dcterms:coverage <http://purl.org/dc/terms/>)
AnnotationAssertion(rdfs:label dcterms:coverage "Coverage"@en)
SubAnnotationPropertyOf(dcterms:coverage <http://purl.org/dc/elements/1.1/coverage>)

# Annotation Property: dcterms:created (Date Created)

AnnotationAssertion(dcterms:description dcterms:created "Recommended practice is to describe the date, date/time, or period of time as recommended for the property Date, of which this is a subproperty."@en)
AnnotationAssertion(rdfs:comment dcterms:created "Date of creation of the resource."@en)
AnnotationAssertion(rdfs:isDefinedBy dcterms:created <http://purl.org/dc/terms/>)
AnnotationAssertion(rdfs:label dcterms:created "Date Created"@en)
SubAnnotationPropertyOf(dcterms:created <http://purl.org/dc/elements/1.1/date>)

# Annotation Property: dcterms:creator (Creator)

AnnotationAssertion(<http://purl.org/dc/dcam/rangeIncludes> dcterms:creator dcterms:Agent)
AnnotationAssertion(dcterms:description dcterms:creator "Recommended practice is to identify the creator with a URI.  If this is not possible or feasible, a literal value that identifies the creator may be provided."@en)
AnnotationAssertion(rdfs:comment dcterms:creator "An entity responsible for making the resource."@en)
AnnotationAssertion(rdfs:isDefinedBy dcterms:creator <http://purl.org/dc/terms/>)
AnnotationAssertion(rdfs:label dcterms:creator "Creator"@en)
SubAnnotationPropertyOf(dcterms:creator <http://purl.org/dc/elements/1.1/creator>)
SubAnnotationPropertyOf(dcterms:creator dcterms:contributor)

# Annotation Property: dcterms:date (Date)

AnnotationAssertion(dcterms:description dcterms:date "Date may be used to express temporal information at any level of granularity.  Recommended practice is to express the date, date/time, or period of time according to ISO 8601-1 [[ISO 8601-1](https://www.iso.org/iso-8601-date-and-time-format.html)] or a published profile of the ISO standard, such as the W3C Note on Date and Time Formats [[W3CDTF](https://www.w3.org/TR/NOTE-datetime)] or the Extended Date/Time Format Specification [[EDTF](http://www.loc.gov/standards/datetime/)].  If the full date is unknown, month and year (YYYY-MM) or just year (YYYY) may be used. Date ranges may be specified using ISO 8601 period of time specification in which start and end dates are separated by a '/' (slash) character.  Either the start or end date may be missing."@en)
AnnotationAssertion(rdfs:comment dcterms:date "A point or period of time associated with an event in the lifecycle of the resource."@en)
AnnotationAssertion(rdfs:isDefinedBy dcterms:date <http://purl.org/dc/terms/>)
AnnotationAssertion(rdfs:label dcterms:date "Date"@en)
SubAnnotationPropertyOf(dcterms:date <http://purl.org/dc/elements/1.1/date>)

# Annotation Property: dcterms:dateAccepted (Date Accepted)

AnnotationAssertion(dcterms:description dcterms:dateAccepted "Recommended practice is to describe the date, date/time, or period of time as recommended for the property Date, of which this is a subproperty.  Examples of resources to which a date of acceptance may be relevant are a thesis (accepted by a university department) or an article (accepted by a journal)."@en)
AnnotationAssertion(rdfs:comment dcterms:dateAccepted "Date of acceptance of the resource."@en)
AnnotationAssertion(rdfs:isDefinedBy dcterms:dateAccepted <http://purl.org/dc/terms/>)
AnnotationAssertion(rdfs:label dcterms:dateAccepted "Date Accepted"@en)
SubAnnotationPropertyOf(dcterms:dateAccepted <http://purl.org/dc/elements/1.1/date>)

# Annotation Property: dcterms:dateCopyrighted (Date Copyrighted)

AnnotationAssertion(dcterms:description dcterms:dateCopyrighted "Typically a year.  Recommended practice is to describe the date, date/time, or period of time as recommended for the property Date, of which this is a subproperty."@en)
AnnotationAssertion(rdfs:comment dcterms:dateCopyrighted "Date of copyright of the resource."@en)
AnnotationAssertion(rdfs:isDefinedBy dcterms:dateCopyrighted <http://purl.org/dc/terms/>)
AnnotationAssertion(rdfs:label dcterms:dateCopyrighted "Date Copyrighted"@en)
SubAnnotationPropertyOf(dcterms:dateCopyrighted <http://purl.org/dc/elements/1.1/date>)

# Annotation Property: dcterms:dateSubmitted (Date Submitted)

AnnotationAssertion(dcterms:description dcterms:dateSubmitted "Recommended practice is to describe the date, date/time, or period of time as recommended for the property Date, of which this is a subproperty.  Examples of resources to which a 'Date Submitted' may be relevant include a thesis (submitted to a university department) or an article (submitted to a journal)."@en)
AnnotationAssertion(rdfs:comment dcterms:dateSubmitted "Date of submission of the resource."@en)
AnnotationAssertion(rdfs:isDefinedBy dcterms:dateSubmitted <http://purl.org/dc/terms/>)
AnnotationAssertion(rdfs:label dcterms:dateSubmitted "Date Submitted"@en)
SubAnnotationPropertyOf(dcterms:dateSubmitted <http://purl.org/dc/elements/1.1/date>)

# Annotation Property: dcterms:description (Description)

AnnotationAssertion(dcterms:description dcterms:description "Description may include but is not limited to: an abstract, a table of contents, a graphical representation, or a free-text account of the resource."@en)
AnnotationAssertion(rdfs:comment dcterms:description "An account of the resource."@en)
AnnotationAssertion(rdfs:isDefinedBy dcterms:description <http://purl.org/dc/terms/>)
AnnotationAssertion(rdfs:label dcterms:description "Description"@en)
SubAnnotationPropertyOf(dcterms:description <http://purl.org/dc/elements/1.1/description>)

# Annotation Property: dcterms:educationLevel (Audience Education Level)

AnnotationAssertion(<http://purl.org/dc/dcam/rangeIncludes> dcterms:educationLevel dcterms:AgentClass)
AnnotationAssertion(rdfs:comment dcterms:educationLevel "A class of agents, defined in terms of progression through an educational or training context, for which the described resource is intended."@en)
AnnotationAssertion(rdfs:isDefinedBy dcterms:educationLevel <http://purl.org/dc/terms/>)
AnnotationAssertion(rdfs:label dcterms:educationLevel "Audience Education Level"@en)
SubAnnotationPropertyOf(dcterms:educationLevel dcterms:audience)

# Annotation Property: dcterms:extent (Extent)

AnnotationAssertion(<http://purl.org/dc/dcam/rangeIncludes> dcterms:extent dcterms:SizeOrDuration)
AnnotationAssertion(dcterms:description dcterms:extent "Recommended practice is to specify the file size in megabytes and duration in ISO 8601 format."@en)
AnnotationAssertion(rdfs:comment dcterms:extent "The size or duration of the resource."@en)
AnnotationAssertion(rdfs:isDefinedBy dcterms:extent <http://purl.org/dc/terms/>)
AnnotationAssertion(rdfs:label dcterms:extent "Extent"@en)
SubAnnotationPropertyOf(dcterms:extent <http://purl.org/dc/elements/1.1/format>)
SubAnnotationPropertyOf(dcterms:extent dcterms:format)

# Annotation Property: dcterms:format (Format)

AnnotationAssertion(<http://purl.org/dc/dcam/rangeIncludes> dcterms:format dcterms:Extent)
AnnotationAssertion(<http://purl.org/dc/dcam/rangeIncludes> dcterms:format dcterms:MediaType)
AnnotationAssertion(dcterms:description dcterms:format "Recommended practice is to use a controlled vocabulary where available. For example, for file formats one could use the list of Internet Media Types [[MIME](https://www.iana.org/assignments/media-types/media-types.xhtml)].  Examples of dimensions include size and duration."@en)
AnnotationAssertion(rdfs:comment dcterms:format "The file format, physical medium, or dimensions of the resource."@en)
AnnotationAssertion(rdfs:isDefinedBy dcterms:format <http://purl.org/dc/terms/>)
AnnotationAssertion(rdfs:label dcterms:format "Format"@en)
SubAnnotationPropertyOf(dcterms:format <http://purl.org/dc/elements/1.1/format>)

# Annotation Property: dcterms:hasFormat (Has Format)

AnnotationAssertion(dcterms:description dcterms:hasFormat "This property is intended to be used with non-literal values. This property is an inverse property of Is Format Of."@en)
AnnotationAssertion(rdfs:comment dcterms:hasFormat "A related resource that is substantially the same as the pre-existing described resource, but in another format."@en)
AnnotationAssertion(rdfs:isDefinedBy dcterms:hasFormat <http://purl.org/dc/terms/>)
AnnotationAssertion(rdfs:label dcterms:hasFormat "Has Format"@en)
SubAnnotationPropertyOf(dcterms:hasFormat <http://purl.org/dc/elements/1.1/relation>)
SubAnnotationPropertyOf(dcterms:hasFormat dcterms:relation)

# Annotation Property: dcterms:hasPart (Has Part)

AnnotationAssertion(dcterms:description dcterms:hasPart "This property is intended to be used with non-literal values. This property is an inverse property of Is Part Of."@en)
AnnotationAssertion(rdfs:comment dcterms:hasPart "A related resource that is included either physically or logically in the described resource."@en)
AnnotationAssertion(rdfs:isDefinedBy dcterms:hasPart <http://purl.org/dc/terms/>)
AnnotationAssertion(rdfs:label dcterms:hasPart "Has Part"@en)
SubAnnotationPropertyOf(dcterms:hasPart <http://purl.org/dc/elements/1.1/relation>)
SubAnnotationPropertyOf(dcterms:hasPart dcterms:relation)

# Annotation Property: dcterms:hasVersion (Has Version)

AnnotationAssertion(dcterms:description dcterms:hasVersion "Changes in version imply substantive changes in content rather than differences in format. This property is intended to be used with non-literal values. This property is an inverse property of Is Version Of."@en)
AnnotationAssertion(rdfs:comment dcterms:hasVersion "A related resource that is a version, edition, or adaptation of the described resource."@en)
AnnotationAssertion(rdfs:isDefinedBy dcterms:hasVersion <http://purl.org/dc/terms/>)
AnnotationAssertion(rdfs:label dcterms:hasVersion "Has Version"@en)
SubAnnotationPropertyOf(dcterms:hasVersion <http://purl.org/dc/elements/1.1/relation>)
SubAnnotationPropertyOf(dcterms:hasVersion dcterms:relation)

# Annotation Property: dcterms:identifier (Identifier)

AnnotationAssertion(dcterms:description dcterms:identifier "Recommended practice is to identify the resource by means of a string conforming to an identification system. Examples include International Standard Book Number (ISBN), Digital Object Identifier (DOI), and Uniform Resource Name (URN).  Persistent identifiers should be provided as HTTP URIs."@en)
AnnotationAssertion(rdfs:comment dcterms:identifier "An unambiguous reference to the resource within a given context."@en)
AnnotationAssertion(rdfs:isDefinedBy dcterms:identifier <http://purl.org/dc/terms/>)
AnnotationAssertion(rdfs:label dcterms:identifier "Identifier"@en)
SubAnnotationPropertyOf(dcterms:identifier <http://purl.org/dc/elements/1.1/identifier>)

# Annotation Property: dcterms:isFormatOf (Is Format Of)

AnnotationAssertion(dcterms:description dcterms:isFormatOf "This property is intended to be used with non-literal values. This property is an inverse property of Has Format."@en)
AnnotationAssertion(rdfs:comment dcterms:isFormatOf "A pre-existing related resource that is substantially the same as the described resource, but in another format."@en)
AnnotationAssertion(rdfs:isDefinedBy dcterms:isFormatOf <http://purl.org/dc/terms/>)
AnnotationAssertion(rdfs:label dcterms:isFormatOf "Is Format Of"@en)
SubAnnotationPropertyOf(dcterms:isFormatOf <http://purl.org/dc/elements/1.1/relation>)
SubAnnotationPropertyOf(dcterms:isFormatOf dcterms:relation)

# Annotation Property: dcterms:isPartOf (Is Part Of)

AnnotationAssertion(dcterms:description dcterms:isPartOf "This property is intended to be used with non-literal values. This property is an inverse property of Has Part."@en)
AnnotationAssertion(rdfs:comment dcterms:isPartOf "A related resource in which the described resource is physically or logically included."@en)
AnnotationAssertion(rdfs:isDefinedBy dcterms:isPartOf <http://purl.org/dc/terms/>)
AnnotationAssertion(rdfs:label dcterms:isPartOf "Is Part Of"@en)
SubAnnotationPropertyOf(dcterms:isPartOf <http://purl.org/dc/elements/1.1/relation>)
SubAnnotationPropertyOf(dcterms:isPartOf dcterms:relation)

# Annotation Property: dcterms:isReferencedBy (Is Referenced By)

AnnotationAssertion(dcterms:description dcterms:isReferencedBy "This property is intended to be used with non-literal values. This property is an inverse property of References."@en)
AnnotationAssertion(rdfs:comment dcterms:isReferencedBy "A related resource that references, cites, or otherwise points to the described resource."@en)
AnnotationAssertion(rdfs:isDefinedBy dcterms:isReferencedBy <http://purl.org/dc/terms/>)
AnnotationAssertion(rdfs:label dcterms:isReferencedBy "Is Referenced By"@en)
SubAnnotationPropertyOf(dcterms:isReferencedBy <http://purl.org/dc/elements/1.1/relation>)
SubAnnotationPropertyOf(dcterms:isReferencedBy dcterms:relation)

# Annotation Property: dcterms:isReplacedBy (Is Replaced By)

AnnotationAssertion(dcterms:description dcterms:isReplacedBy "This property is intended to be used with non-literal values. This property is an inverse property of Replaces."@en)
AnnotationAssertion(rdfs:comment dcterms:isReplacedBy "A related resource that supplants, displaces, or supersedes the described resource."@en)
AnnotationAssertion(rdfs:isDefinedBy dcterms:isReplacedBy <http://purl.org/dc/terms/>)
AnnotationAssertion(rdfs:label dcterms:isReplacedBy "Is Replaced By"@en)
SubAnnotationPropertyOf(dcterms:isReplacedBy <http://purl.org/dc/elements/1.1/relation>)
SubAnnotationPropertyOf(dcterms:isReplacedBy dcterms:relation)

# Annotation Property: dcterms:isRequiredBy (Is Required By)

AnnotationAssertion(dcterms:description dcterms:isRequiredBy "This property is intended to be used with non-literal values. This property is an inverse property of Requires."@en)
AnnotationAssertion(rdfs:comment dcterms:isRequiredBy "A related resource that requires the described resource to support its function, delivery, or coherence."@en)
AnnotationAssertion(rdfs:isDefinedBy dcterms:isRequiredBy <http://purl.org/dc/terms/>)
AnnotationAssertion(rdfs:label dcterms:isRequiredBy "Is Required By"@en)
SubAnnotationPropertyOf(dcterms:isRequiredBy <http://purl.org/dc/elements/1.1/relation>)
SubAnnotationPropertyOf(dcterms:isRequiredBy dcterms:relation)

# Annotation Property: dcterms:isVersionOf (Is Version Of)

AnnotationAssertion(dcterms:description dcterms:isVersionOf "Changes in version imply substantive changes in content rather than differences in format. This property is intended to be used with non-literal values. This property is an inverse property of Has Version."@en)
AnnotationAssertion(rdfs:comment dcterms:isVersionOf "A related resource of which the described resource is a version, edition, or adaptation."@en)
AnnotationAssertion(rdfs:isDefinedBy dcterms:isVersionOf <http://purl.org/dc/terms/>)
AnnotationAssertion(rdfs:label dcterms:isVersionOf "Is Version Of"@en)
SubAnnotationPropertyOf(dcterms:isVersionOf <http://purl.org/dc/elements/1.1/relation>)
SubAnnotationPropertyOf(dcterms:isVersionOf dcterms:relation)

# Annotation Property: dcterms:issued (Date Issued)

AnnotationAssertion(dcterms:description dcterms:issued "Recommended practice is to describe the date, date/time, or period of time as recommended for the property Date, of which this is a subproperty."@en)
AnnotationAssertion(rdfs:comment dcterms:issued "Date of formal issuance of the resource."@en)
AnnotationAssertion(rdfs:isDefinedBy dcterms:issued <http://purl.org/dc/terms/>)
AnnotationAssertion(rdfs:label dcterms:issued "Date Issued"@en)
SubAnnotationPropertyOf(dcterms:issued <http://purl.org/dc/elements/1.1/date>)

# Annotation Property: dcterms:language (Language)

AnnotationAssertion(<http://purl.org/dc/dcam/rangeIncludes> dcterms:language dcterms:LinguisticSystem)
AnnotationAssertion(dcterms:description dcterms:language "Recommended practice is to use either a non-literal value representing a language from a controlled vocabulary such as ISO 639-2 or ISO 639-3, or a literal value consisting of an IETF Best Current Practice 47 [[IETF-BCP47](https://tools.ietf.org/html/bcp47)] language tag."@en)
AnnotationAssertion(rdfs:comment dcterms:language "A language of the resource."@en)
AnnotationAssertion(rdfs:isDefinedBy dcterms:language <http://purl.org/dc/terms/>)
AnnotationAssertion(rdfs:label dcterms:language "Language"@en)
SubAnnotationPropertyOf(dcterms:language <http://purl.org/dc/elements/1.1/language>)

# Annotation Property: dcterms:license (License)

AnnotationAssertion(<http://purl.org/dc/dcam/rangeIncludes> dcterms:license dcterms:LicenseDocument)
AnnotationAssertion(dcterms:description dcterms:license "Recommended practice is to identify the license document with a URI. If this is not possible or feasible, a literal value that identifies the license may be provided."@en)
AnnotationAssertion(rdfs:comment dcterms:license "A legal document giving official permission to do something with the resource."@en)
AnnotationAssertion(rdfs:isDefinedBy dcterms:license <http://purl.org/dc/terms/>)
AnnotationAssertion(rdfs:label dcterms:license "License"@en)
SubAnnotationPropertyOf(dcterms:license <http://purl.org/dc/elements/1.1/rights>)
SubAnnotationPropertyOf(dcterms:license dcterms:rights)

# Annotation Property: dcterms:mediator (Mediator)

AnnotationAssertion(<http://purl.org/dc/dcam/rangeIncludes> dcterms:mediator dcterms:AgentClass)
AnnotationAssertion(dcterms:description dcterms:mediator "In an educational context, a mediator might be a parent, teacher, teaching assistant, or care-giver."@en)
AnnotationAssertion(rdfs:comment dcterms:mediator "An entity that mediates access to the resource."@en)
AnnotationAssertion(rdfs:isDefinedBy dcterms:mediator <http://purl.org/dc/terms/>)
AnnotationAssertion(rdfs:label dcterms:mediator "Mediator"@en)
SubAnnotationPropertyOf(dcterms:mediator dcterms:audience)

# Annotation Property: dcterms:medium (Medium)

AnnotationAssertion(<http://purl.org/dc/dcam/domainIncludes> dcterms:medium dcterms:PhysicalResource)
AnnotationAssertion(<http://purl.org/dc/dcam/rangeIncludes> dcterms:medium dcterms:PhysicalMedium)
AnnotationAssertion(rdfs:comment dcterms:medium "The material or physical carrier of the resource."@en)
AnnotationAssertion(rdfs:isDefinedBy dcterms:medium <http://purl.org/dc/terms/>)
AnnotationAssertion(rdfs:label dcterms:medium "Medium"@en)
SubAnnotationPropertyOf(dcterms:medium <http://purl.org/dc/elements/1.1/format>)
SubAnnotationPropertyOf(dcterms:medium dcterms:format)

# Annotation Property: dcterms:modified (Date Modified)

AnnotationAssertion(dcterms:description dcterms:modified "Recommended practice is to describe the date, date/time, or period of time as recommended for the property Date, of which this is a subproperty."@en)
AnnotationAssertion(rdfs:comment dcterms:modified "Date on which the resource was changed."@en)
AnnotationAssertion(rdfs:isDefinedBy dcterms:modified <http://purl.org/dc/terms/>)
AnnotationAssertion(rdfs:label dcterms:modified "Date Modified"@en)
SubAnnotationPropertyOf(dcterms:modified <http://purl.org/dc/elements/1.1/date>)

# Annotation Property: dcterms:publisher (Publisher)

AnnotationAssertion(<http://purl.org/dc/dcam/rangeIncludes> dcterms:publisher dcterms:Agent)
AnnotationAssertion(rdfs:comment dcterms:publisher "An entity responsible for making the resource available."@en)
AnnotationAssertion(rdfs:isDefinedBy dcterms:publisher <http://purl.org/dc/terms/>)
AnnotationAssertion(rdfs:label dcterms:publisher "Publisher"@en)
SubAnnotationPropertyOf(dcterms:publisher <http://purl.org/dc/elements/1.1/publisher>)

# Annotation Property: dcterms:references (References)

AnnotationAssertion(dcterms:description dcterms:references "This property is intended to be used with non-literal values. This property is an inverse property of Is Referenced By."@en)
AnnotationAssertion(rdfs:comment dcterms:references "A related resource that is referenced, cited, or otherwise pointed to by the described resource."@en)
AnnotationAssertion(rdfs:isDefinedBy dcterms:references <http://purl.org/dc/terms/>)
AnnotationAssertion(rdfs:label dcterms:references "References"@en)
SubAnnotationPropertyOf(dcterms:references <http://purl.org/dc/elements/1.1/relation>)
SubAnnotationPropertyOf(dcterms:references dcterms:relation)

# Annotation Property: dcterms:relation (Relation)

AnnotationAssertion(dcterms:description dcterms:relation "Recommended practice is to identify the related resource by means of a URI.  If this is not possible or feasible, a string conforming to a formal identification system may be provided."@en)
AnnotationAssertion(rdfs:comment dcterms:relation "A related resource."@en)
AnnotationAssertion(rdfs:isDefinedBy dcterms:relation <http://purl.org/dc/terms/>)
AnnotationAssertion(rdfs:label dcterms:relation "Relation"@en)
SubAnnotationPropertyOf(dcterms:relation <http://purl.org/dc/elements/1.1/relation>)

# Annotation Property: dcterms:replaces (Replaces)

AnnotationAssertion(dcterms:description dcterms:replaces "This property is intended to be used with non-literal values. This property is an inverse property of Is Replaced By."@en)
AnnotationAssertion(rdfs:comment dcterms:replaces "A related resource that is supplanted, displaced, or superseded by the described resource."@en)
AnnotationAssertion(rdfs:isDefinedBy dcterms:replaces <http://purl.org/dc/terms/>)
AnnotationAssertion(rdfs:label dcterms:replaces "Replaces"@en)
SubAnnotationPropertyOf(dcterms:replaces <http://purl.org/dc/elements/1.1/relation>)
SubAnnotationPropertyOf(dcterms:replaces dcterms:relation)

# Annotation Property: dcterms:requires (Requires)

AnnotationAssertion(dcterms:description dcterms:requires "This property is intended to be used with non-literal values. This property is an inverse property of Is Required By."@en)
AnnotationAssertion(rdfs:comment dcterms:requires "A related resource that is required by the described resource to support its function, delivery, or coherence."@en)
AnnotationAssertion(rdfs:isDefinedBy dcterms:requires <http://purl.org/dc/terms/>)
AnnotationAssertion(rdfs:label dcterms:requires "Requires"@en)
SubAnnotationPropertyOf(dcterms:requires <http://purl.org/dc/elements/1.1/relation>)
SubAnnotationPropertyOf(dcterms:requires dcterms:relation)

# Annotation Property: dcterms:rights (Rights)

AnnotationAssertion(<http://purl.org/dc/dcam/rangeIncludes> dcterms:rights dcterms:RightsStatement)
AnnotationAssertion(dcterms:description dcterms:rights "Typically, rights information includes a statement about various property rights associated with the resource, including intellectual property rights.  Recommended practice is to refer to a rights statement with a URI.  If this is not possible or feasible, a literal value (name, label, or short text) may be provided."@en)
AnnotationAssertion(rdfs:comment dcterms:rights "Information about rights held in and over the resource."@en)
AnnotationAssertion(rdfs:isDefinedBy dcterms:rights <http://purl.org/dc/terms/>)
AnnotationAssertion(rdfs:label dcterms:rights "Rights"@en)
SubAnnotationPropertyOf(dcterms:rights <http://purl.org/dc/elements/1.1/rights>)

# Annotation Property: dcterms:source (Source)

AnnotationAssertion(dcterms:description dcterms:source "This property is intended to be used with non-literal values. The described resource may be derived from the related resource in whole or in part. Best practice is to identify the related resource by means of a URI or a string conforming to a formal identification system."@en)
AnnotationAssertion(rdfs:comment dcterms:source "A related resource from which the described resource is derived."@en)
AnnotationAssertion(rdfs:isDefinedBy dcterms:source <http://purl.org/dc/terms/>)
AnnotationAssertion(rdfs:label dcterms:source "Source"@en)
SubAnnotationPropertyOf(dcterms:source <http://purl.org/dc/elements/1.1/source>)
SubAnnotationPropertyOf(dcterms:source dcterms:relation)

# Annotation Property: dcterms:spatial (Spatial Coverage)

AnnotationAssertion(<http://purl.org/dc/dcam/rangeIncludes> dcterms:spatial dcterms:Location)
AnnotationAssertion(rdfs:comment dcterms:spatial "Spatial characteristics of the resource."@en)
AnnotationAssertion(rdfs:isDefinedBy dcterms:spatial <http://purl.org/dc/terms/>)
AnnotationAssertion(rdfs:label dcterms:spatial "Spatial Coverage"@en)
SubAnnotationPropertyOf(dcterms:spatial <http://purl.org/dc/elements/1.1/coverage>)
SubAnnotationPropertyOf(dcterms:spatial dcterms:coverage)

# Annotation Property: dcterms:subject (Subject)

AnnotationAssertion(dcterms:description dcterms:subject "Recommended practice is to refer to the subject with a URI. If this is not possible or feasible, a literal value that identifies the subject may be provided. Both should preferably refer to a subject in a controlled vocabulary."@en)
AnnotationAssertion(rdfs:comment dcterms:subject "A topic of the resource."@en)
AnnotationAssertion(rdfs:isDefinedBy dcterms:subject <http://purl.org/dc/terms/>)
AnnotationAssertion(rdfs:label dcterms:subject "Subject"@en)
SubAnnotationPropertyOf(dcterms:subject <http://purl.org/dc/elements/1.1/subject>)

# Annotation Property: dcterms:tableOfContents (Table Of Contents)

AnnotationAssertion(rdfs:comment dcterms:tableOfContents "A list of subunits of the resource."@en)
AnnotationAssertion(rdfs:isDefinedBy dcterms:tableOfContents <http://purl.org/dc/terms/>)
AnnotationAssertion(rdfs:label dcterms:tableOfContents "Table Of Contents"@en)
SubAnnotationPropertyOf(dcterms:tableOfContents <http://purl.org/dc/elements/1.1/description>)
SubAnnotationPropertyOf(dcterms:tableOfContents dcterms:description)

# Annotation Property: dcterms:temporal (Temporal Coverage)

AnnotationAssertion(<http://purl.org/dc/dcam/rangeIncludes> dcterms:temporal dcterms:PeriodOfTime)
AnnotationAssertion(rdfs:comment dcterms:temporal "Temporal characteristics of the resource."@en)
AnnotationAssertion(rdfs:isDefinedBy dcterms:temporal <http://purl.org/dc/terms/>)
AnnotationAssertion(rdfs:label dcterms:temporal "Temporal Coverage"@en)
SubAnnotationPropertyOf(dcterms:temporal <http://purl.org/dc/elements/1.1/coverage>)
SubAnnotationPropertyOf(dcterms:temporal dcterms:coverage)

# Annotation Property: dcterms:title (Title)

AnnotationAssertion(rdfs:comment dcterms:title "A name given to the resource."@en)
AnnotationAssertion(rdfs:isDefinedBy dcterms:title <http://purl.org/dc/terms/>)
AnnotationAssertion(rdfs:label dcterms:title "Title"@en)
SubAnnotationPropertyOf(dcterms:title <http://purl.org/dc/elements/1.1/title>)

# Annotation Property: dcterms:type (Type)

AnnotationAssertion(dcterms:description dcterms:type "Recommended practice is to use a controlled vocabulary such as the DCMI Type Vocabulary [[DCMI-TYPE](http://dublincore.org/documents/dcmi-type-vocabulary/)]. To describe the file format, physical medium, or dimensions of the resource, use the property Format."@en)
AnnotationAssertion(rdfs:comment dcterms:type "The nature or genre of the resource."@en)
AnnotationAssertion(rdfs:isDefinedBy dcterms:type <http://purl.org/dc/terms/>)
AnnotationAssertion(rdfs:label dcterms:type "Type"@en)
SubAnnotationPropertyOf(dcterms:type <http://purl.org/dc/elements/1.1/type>)

# Annotation Property: dcterms:valid (Date Valid)

AnnotationAssertion(dcterms:description dcterms:valid "Recommended practice is to describe the date, date/time, or period of time as recommended for the property Date, of which this is a subproperty."@en)
AnnotationAssertion(rdfs:comment dcterms:valid "Date (often a range) of validity of a resource."@en)
AnnotationAssertion(rdfs:isDefinedBy dcterms:valid <http://purl.org/dc/terms/>)
AnnotationAssertion(rdfs:label dcterms:valid "Date Valid"@en)
SubAnnotationPropertyOf(dcterms:valid <http://purl.org/dc/elements/1.1/date>)


############################
#   Object Properties
############################

# Object Property: pav:hasVersion (pav:hasVersion)

EquivalentObjectProperties(pav:hasVersion dcat:hasVersion)

# Object Property: dcat:accessService (servicio de acceso de datos)

AnnotationAssertion(rdfs:comment dcat:accessService "A site or end-point that gives access to the distribution of the dataset."@en)
AnnotationAssertion(rdfs:comment dcat:accessService "Et websted eller endpoint der giver adgang til en repræsentation af datasættet."@da)
AnnotationAssertion(rdfs:comment dcat:accessService "Umístění či přístupový bod zpřístupňující distribuci datové sady."@cs)
AnnotationAssertion(rdfs:comment dcat:accessService "Un sitio o end-point que da acceso a la distribución de un conjunto de datos."@es)
AnnotationAssertion(rdfs:comment dcat:accessService "Un sito o end-point che dà accesso alla distribuzione del set di dati."@it)
AnnotationAssertion(rdfs:isDefinedBy dcat:accessService <https://www.w3.org/TR/vocab-dcat-2/>)
AnnotationAssertion(rdfs:label dcat:accessService "data access service"@en)
AnnotationAssertion(rdfs:label dcat:accessService "dataadgangstjeneste"@da)
AnnotationAssertion(rdfs:label dcat:accessService "servicio de acceso de datos"@es)
AnnotationAssertion(rdfs:label dcat:accessService "servizio di accesso ai dati"@it)
AnnotationAssertion(rdfs:label dcat:accessService "služba pro přístup k datům"@cs)
AnnotationAssertion(skos:changeNote dcat:accessService "New property added in DCAT 2."@en)
AnnotationAssertion(skos:changeNote dcat:accessService "Nová vlastnost přidaná ve verzi DCAT 2."@cs)
AnnotationAssertion(skos:changeNote dcat:accessService "Nueva propiedad agregada en DCAT 2."@es)
AnnotationAssertion(skos:changeNote dcat:accessService "Nuova proprietà aggiunta in DCAT 2."@it)
AnnotationAssertion(skos:changeNote dcat:accessService "Ny egenskab tilføjet i DCAT 2."@da)
AnnotationAssertion(skos:definition dcat:accessService "A site or end-point that gives access to the distribution of the dataset."@en)
AnnotationAssertion(skos:definition dcat:accessService "Et websted eller endpoint der giver adgang til en repræsentation af datasættet."@da)
AnnotationAssertion(skos:definition dcat:accessService "Umístění či přístupový bod zpřístupňující distribuci datové sady."@cs)
AnnotationAssertion(skos:definition dcat:accessService "Un sitio o end-point que da acceso a la distribución de un conjunto de datos."@es)
AnnotationAssertion(skos:definition dcat:accessService "Un sito o end-point che dà accesso alla distribuzione del set di dati."@it)
ObjectPropertyRange(dcat:accessService dcat:DataService)

# Object Property: dcat:accessURL (přístupová adresa)

AnnotationAssertion(rdfs:comment dcat:accessURL "A URL of a resource that gives access to a distribution of the dataset. E.g. landing page, feed, SPARQL endpoint. Use for all cases except a simple download link, in which case downloadURL is preferred."@en)
AnnotationAssertion(rdfs:comment dcat:accessURL "Ceci peut être tout type d'URL qui donne accès à une distribution du jeu de données. Par exemple, un lien à une page HTML contenant un lien au jeu de données, un Flux RSS, un point d'accès SPARQL. Utilisez le lorsque votre catalogue ne contient pas d'information sur quoi il est ou quand ce n'est pas téléchargeable."@fr)
AnnotationAssertion(rdfs:comment dcat:accessURL "En URL for en ressource som giver adgang til en repræsentation af datsættet. Fx destinationsside, feed, SPARQL-endpoint. Anvendes i alle sammenhænge undtagen til angivelse af et simpelt download link hvor anvendelse af egenskaben downloadURL foretrækkes."@da)
AnnotationAssertion(rdfs:comment dcat:accessURL "Puede ser cualquier tipo de URL que de acceso a una distribución del conjunto de datos, e.g., página de destino, descarga, URL feed, punto de acceso SPARQL. Esta propriedad se debe usar cuando su catálogo de datos no tiene información sobre donde está o cuando no se puede descargar."@es)
AnnotationAssertion(rdfs:comment dcat:accessURL "URL zdroje, přes které je přístupná distribuce datové sady. Příkladem může být vstupní stránka, RSS kanál či SPARQL endpoint. Použijte ve všech případech kromě URL souboru ke stažení, pro které je lepší použít dcat:downloadURL."@cs)
AnnotationAssertion(rdfs:comment dcat:accessURL "Un URL di una risorsa che consente di accedere a una distribuzione del set di dati. Per esempio, pagina di destinazione, feed, endpoint SPARQL. Da utilizzare per tutti i casi, tranne  quando  si tratta di un semplice link per il download nel qual caso è preferito downloadURL."@it)
AnnotationAssertion(rdfs:comment dcat:accessURL "Μπορεί να είναι οποιουδήποτε είδους URL που δίνει πρόσβαση στη διανομή ενός συνόλου δεδομένων. Π.χ. ιστοσελίδα αρχικής πρόσβασης, μεταφόρτωση, feed URL, σημείο διάθεσης SPARQL. Να χρησιμοποιείται όταν ο κατάλογος δεν περιέχει πληροφορίες εαν πρόκειται ή όχι για μεταφορτώσιμο αρχείο."@el)
AnnotationAssertion(rdfs:comment dcat:accessURL "أي رابط يتيح الوصول إلى البيانات. إذا كان الرابط هو ربط مباشر لملف يمكن تحميله استخدم الخاصية downloadURL"@ar)
AnnotationAssertion(rdfs:comment dcat:accessURL "データセットの配信にアクセス権を与えるランディング・ページ、フィード、SPARQLエンドポイント、その他の種類の資源。"@ja)
AnnotationAssertion(rdfs:isDefinedBy dcat:accessURL <http://www.w3.org/TR/vocab-dcat/>)
AnnotationAssertion(rdfs:label dcat:accessURL "URL d'accès"@fr)
AnnotationAssertion(rdfs:label dcat:accessURL "URL de acceso"@es)
AnnotationAssertion(rdfs:label dcat:accessURL "URL πρόσβασης"@el)
AnnotationAssertion(rdfs:label dcat:accessURL "access address"@en)
AnnotationAssertion(rdfs:label dcat:accessURL "adgangsadresse"@da)
AnnotationAssertion(rdfs:label dcat:accessURL "indirizzo di accesso"@it)
AnnotationAssertion(rdfs:label dcat:accessURL "přístupová adresa"@cs)
AnnotationAssertion(rdfs:label dcat:accessURL "رابط وصول"@ar)
AnnotationAssertion(rdfs:label dcat:accessURL "アクセスURL"@ja)
AnnotationAssertion(skos:altLabel dcat:accessURL "adgangsURL"@da)
AnnotationAssertion(skos:definition dcat:accessURL "A URL of a resource that gives access to a distribution of the dataset. E.g. landing page, feed, SPARQL endpoint. Use for all cases except a simple download link, in which case downloadURL is preferred."@en)
AnnotationAssertion(skos:definition dcat:accessURL "Ceci peut être tout type d'URL qui donne accès à une distribution du jeu de données. Par exemple, un lien à une page HTML contenant un lien au jeu de données, un Flux RSS, un point d'accès SPARQL. Utilisez le lorsque votre catalogue ne contient pas d'information sur quoi il est ou quand ce n'est pas téléchargeable."@fr)
AnnotationAssertion(skos:definition dcat:accessURL "En URL for en ressource som giver adgang til en repræsentation af datsættet. Fx destinationsside, feed, SPARQL-endpoint. Anvendes i alle sammenhænge undtagen til angivelse af et simpelt download link hvor anvendelse af egenskaben downloadURL foretrækkes."@da)
AnnotationAssertion(skos:definition dcat:accessURL "Puede ser cualquier tipo de URL que de acceso a una distribución del conjunto de datos, e.g., página de destino, descarga, URL feed, punto de acceso SPARQL. Esta propriedad se debe usar cuando su catálogo de datos no tiene información sobre donde está o cuando no se puede descargar."@es)
AnnotationAssertion(skos:definition dcat:accessURL "URL zdroje, přes které je přístupná distribuce datové sady. Příkladem může být vstupní stránka, RSS kanál či SPARQL endpoint. Použijte ve všech případech kromě URL souboru ke stažení, pro které je lepší použít dcat:downloadURL."@cs)
AnnotationAssertion(skos:definition dcat:accessURL "Un URL di una risorsa che consente di accedere a una distribuzione del set di dati. Per esempio, pagina di destinazione, feed, endpoint SPARQL. Da utilizzare per tutti i casi, tranne  quando  si tratta di un semplice link per il download nel qual caso è preferito downloadURL."@it)
AnnotationAssertion(skos:definition dcat:accessURL "Μπορεί να είναι οποιουδήποτε είδους URL που δίνει πρόσβαση στη διανομή ενός συνόλου δεδομένων. Π.χ. ιστοσελίδα αρχικής πρόσβασης, μεταφόρτωση, feed URL, σημείο διάθεσης SPARQL. Να χρησιμοποιείται όταν ο κατάλογος δεν περιέχει πληροφορίες εαν πρόκειται ή όχι για μεταφορτώσιμο αρχείο."@el)
AnnotationAssertion(skos:definition dcat:accessURL "أي رابط يتيح الوصول إلى البيانات. إذا كان الرابط هو ربط مباشر لملف يمكن تحميله استخدم الخاصية downloadURL"@ar)
AnnotationAssertion(skos:definition dcat:accessURL "データセットの配信にアクセス権を与えるランディング・ページ、フィード、SPARQLエンドポイント、その他の種類の資源。"@ja)
AnnotationAssertion(skos:editorialNote dcat:accessURL "Status: English Definition text modified by DCAT revision team, updated Italian and Czech translation provided, translations for other languages pending."@en)
AnnotationAssertion(skos:editorialNote dcat:accessURL "rdfs:label, rdfs:comment and skos:scopeNote have been modified. Non-english versions except for Italian must be updated."@en)
AnnotationAssertion(skos:scopeNote dcat:accessURL "El rango es una URL. Si la distribución es accesible solamente través de una página de destino (es decir, si no se conoce una URL de descarga directa), entonces el enlance a la página de destino debe ser duplicado como accessURL en la distribución."@es)
AnnotationAssertion(skos:scopeNote dcat:accessURL "Hvis en eller flere distributioner kun er tilgængelige via en destinationsside (dvs. en URL til direkte download er ikke kendt), så bør destinationssidelinket gentages som adgangsadresse for distributionen."@da)
AnnotationAssertion(skos:scopeNote dcat:accessURL "If the distribution(s) are accessible only through a landing page (i.e. direct download URLs are not known), then the landing page link should be duplicated as accessURL on a distribution."@en)
AnnotationAssertion(skos:scopeNote dcat:accessURL "La valeur est une URL. Si la distribution est accessible seulement au travers d'une page d'atterrissage (c-à-dire on n'ignore une URL de téléchargement direct), alors le lien à la page d'atterrissage doit être dupliqué comee accessURL sur la distribution."@fr)
AnnotationAssertion(skos:scopeNote dcat:accessURL "Pokud jsou distribuce přístupné pouze přes vstupní stránku (tj. URL pro přímé stažení nejsou známa), pak by URL přístupové stránky mělo být duplikováno ve vlastnosti distribuce accessURL."@cs)
AnnotationAssertion(skos:scopeNote dcat:accessURL "Se le distribuzioni sono accessibili solo attraverso una pagina web (ad esempio, gli URL per il download diretto non sono noti), allora il link della pagina web deve essere duplicato come accessURL sulla distribuzione."@it)
AnnotationAssertion(skos:scopeNote dcat:accessURL "Η τιμή είναι ένα URL. Αν η/οι διανομή/ές είναι προσβάσιμη/ες μόνο μέσω μίας ιστοσελίδας αρχικής πρόσβασης (δηλαδή αν δεν υπάρχουν γνωστές διευθύνσεις άμεσης μεταφόρτωσης), τότε ο σύνδεσμος της ιστοσελίδας αρχικής πρόσβασης πρέπει να αναπαραχθεί ως accessURL σε μία διανομή."@el)
AnnotationAssertion(skos:scopeNote dcat:accessURL "確実にダウンロードでない場合や、ダウンロードかどうかが不明である場合は、downloadURLではなく、accessURLを用いてください。ランディング・ページを通じてしか配信にアクセスできない場合（つまり、直接的なダウンロードURLが不明）は、配信におけるaccessURLとしてランディング・ページのリンクをコピーすべきです（SHOULD）。"@ja)
ObjectPropertyDomain(dcat:accessURL dcat:Distribution)
ObjectPropertyRange(dcat:accessURL rdfs:Resource)

# Object Property: dcat:catalog (katalog)

AnnotationAssertion(rdfs:comment dcat:catalog "A catalog that is listed in the catalog."@en)
AnnotationAssertion(rdfs:comment dcat:catalog "Et katalog hvis indhold er relevant i forhold til det aktuelle katalog."@da)
AnnotationAssertion(rdfs:comment dcat:catalog "Katalog, jehož obsah je v kontextu tohoto katalogu zajímavý."@cs)
AnnotationAssertion(rdfs:comment dcat:catalog "Un catalogo i cui contenuti sono di interesse nel contesto di questo catalogo."@it)
AnnotationAssertion(rdfs:comment dcat:catalog "Un catálogo cuyo contenido es de interés en el contexto del catálogo que está siendo descripto."@es)
AnnotationAssertion(rdfs:isDefinedBy dcat:catalog <https://www.w3.org/TR/vocab-dcat-2/>)
AnnotationAssertion(rdfs:label dcat:catalog "catalog"@en)
AnnotationAssertion(rdfs:label dcat:catalog "catalogo"@it)
AnnotationAssertion(rdfs:label dcat:catalog "catálogo"@es)
AnnotationAssertion(rdfs:label dcat:catalog "katalog"@cs)
AnnotationAssertion(rdfs:label dcat:catalog "katalog"@da)
AnnotationAssertion(skos:altLabel dcat:catalog "har delkatalog"@da)
AnnotationAssertion(skos:altLabel dcat:catalog "has catalog"@en)
AnnotationAssertion(skos:changeNote dcat:catalog "New property added in DCAT 2."@en)
AnnotationAssertion(skos:changeNote dcat:catalog "Nová vlastnost přidaná ve verzi DCAT 2."@cs)
AnnotationAssertion(skos:changeNote dcat:catalog "Nueva propiedad agregada en DCAT 2."@es)
AnnotationAssertion(skos:changeNote dcat:catalog "Nuova proprietà aggiunta in DCAT 2."@it)
AnnotationAssertion(skos:definition dcat:catalog "A catalog that is listed in the catalog."@en)
AnnotationAssertion(skos:definition dcat:catalog "Et katalog hvis indhold er relevant i forhold til det aktuelle katalog."@da)
AnnotationAssertion(skos:definition dcat:catalog "Katalog, jehož obsah je v kontextu tohoto katalogu zajímavý."@cs)
AnnotationAssertion(skos:definition dcat:catalog "Un catalogo i cui contenuti sono di interesse nel contesto di questo catalogo."@it)
AnnotationAssertion(skos:definition dcat:catalog "Un catálogo cuyo contenido es de interés en el contexto del catálogo que está siendo descripto."@es)
AnnotationAssertion(skos:editorialNote dcat:catalog "Status: English Definition text modified by DCAT 3 revision team, translations pending."@en)
SubObjectPropertyOf(dcat:catalog dcat:resource)
ObjectPropertyDomain(dcat:catalog dcat:Catalog)
ObjectPropertyRange(dcat:catalog dcat:Catalog)

# Object Property: dcat:compressFormat (formato de compresión)

AnnotationAssertion(rdfs:comment dcat:compressFormat "El formato de la distribución en el que los datos están en forma comprimida, e.g. para reducir el tamaño del archivo a bajar."@es)
AnnotationAssertion(rdfs:comment dcat:compressFormat "Formát komprese souboru, ve kterém jsou data poskytována v komprimované podobě, např. ke snížení velikosti souboru ke stažení."@cs)
AnnotationAssertion(rdfs:comment dcat:compressFormat "Il formato di compressione della distribuzione nel quale i dati sono in forma compressa, ad es. per ridurre le dimensioni del file da scaricare."@it)
AnnotationAssertion(rdfs:comment dcat:compressFormat "Kompressionsformatet for distributionen som indeholder data i et komprimeret format, fx for at reducere størrelsen af downloadfilen."@da)
AnnotationAssertion(rdfs:comment dcat:compressFormat "The compression format of the distribution in which the data is contained in a compressed form, e.g. to reduce the size of the downloadable file."@en)
AnnotationAssertion(rdfs:isDefinedBy dcat:compressFormat <https://www.w3.org/TR/vocab-dcat-2/>)
AnnotationAssertion(rdfs:label dcat:compressFormat "compression format"@en)
AnnotationAssertion(rdfs:label dcat:compressFormat "formato de compresión"@es)
AnnotationAssertion(rdfs:label dcat:compressFormat "formato di compressione"@it)
AnnotationAssertion(rdfs:label dcat:compressFormat "formát komprese"@cs)
AnnotationAssertion(rdfs:label dcat:compressFormat "kompressionsformat"@da)
AnnotationAssertion(skos:changeNote dcat:compressFormat "New property added in DCAT 2."@en)
AnnotationAssertion(skos:changeNote dcat:compressFormat "Nová vlastnost přidaná ve verzi DCAT 2."@cs)
AnnotationAssertion(skos:changeNote dcat:compressFormat "Nueva propiedad agregada en DCAT 2."@es)
AnnotationAssertion(skos:changeNote dcat:compressFormat "Nuova proprietà aggiunta in DCAT 2."@it)
AnnotationAssertion(skos:changeNote dcat:compressFormat "Ny egenskab tilføjet i DCAT 2."@da)
AnnotationAssertion(skos:definition dcat:compressFormat "El formato de la distribución en el que los datos están en forma comprimida, e.g. para reducir el tamaño del archivo a bajar."@es)
AnnotationAssertion(skos:definition dcat:compressFormat "Formát komprese souboru, ve kterém jsou data poskytována v komprimované podobě, např. ke snížení velikosti souboru ke stažení."@cs)
AnnotationAssertion(skos:definition dcat:compressFormat "Il formato di compressione della distribuzione nel quale i dati sono in forma compressa, ad es. per ridurre le dimensioni del file da scaricare."@it)
AnnotationAssertion(skos:definition dcat:compressFormat "Kompressionsformatet for distributionen som indeholder data i et komprimeret format, fx for at reducere størrelsen af downloadfilen."@da)
AnnotationAssertion(skos:definition dcat:compressFormat "The compression format of the distribution in which the data is contained in a compressed form, e.g. to reduce the size of the downloadable file."@en)
AnnotationAssertion(skos:scopeNote dcat:compressFormat "Denne egenskab kan anvendes når filerne i en distribution er blevet komprimeret, fx i en ZIP-fil. Formatet BØR udtrykkes ved en medietype som defineret i 'IANA media types registry', hvis der optræder en relevant medietype dér: https://www.iana.org/assignments/media-types/."@da)
AnnotationAssertion(skos:scopeNote dcat:compressFormat "Esta propiedad se debe usar cuando los archivos de la distribución están comprimidos, por ejemplo en un archivo ZIP. El formato DEBERÍA expresarse usando un 'media type', tales como los definidos en el registro IANA de 'media types' https://www.iana.org/assignments/media-types/, si está disponibles."@es)
AnnotationAssertion(skos:scopeNote dcat:compressFormat "Questa proprietà deve essere utilizzata quando i file nella distribuzione sono compressi, ad es. in un file ZIP. Il formato DOVREBBE essere espresso usando un tipo di media come definito dal registro dei tipi di media IANA https://www.iana.org/assignments/media-types/, se disponibile."@it)
AnnotationAssertion(skos:scopeNote dcat:compressFormat "Tato vlastnost se použije, když jsou soubory v distribuci komprimovány, např. v ZIP souboru. Formát BY MĚL být vyjádřen pomocí typu média definovaného v registru IANA https://www.iana.org/assignments/media-types/, pokud existuje."@cs)
AnnotationAssertion(skos:scopeNote dcat:compressFormat "This property is to be used when the files in the distribution are compressed, e.g. in a ZIP file. The format SHOULD be expressed using a media type as defined by IANA media types registry https://www.iana.org/assignments/media-types/, if available."@en)
SubObjectPropertyOf(dcat:compressFormat dcterms:format)
ObjectPropertyDomain(dcat:compressFormat dcat:Distribution)
ObjectPropertyRange(dcat:compressFormat dcterms:MediaType)

# Object Property: dcat:contactPoint (kontaktní bod)

AnnotationAssertion(rdfs:comment dcat:contactPoint "Información relevante de contacto para el recurso catalogado. Se recomienda el uso de vCard."@es)
AnnotationAssertion(rdfs:comment dcat:contactPoint "Informazioni di contatto rilevanti per la risorsa catalogata. Si raccomanda l'uso di vCard."@it)
AnnotationAssertion(rdfs:comment dcat:contactPoint "Relevant contact information for the catalogued resource. Use of vCard is recommended."@en)
AnnotationAssertion(rdfs:comment dcat:contactPoint "Relevante kontaktoplysninger for den katalogiserede ressource. Anvendelse af vCard anbefales."@da)
AnnotationAssertion(rdfs:comment dcat:contactPoint "Relevantní kontaktní informace pro katalogizovaný zdroj. Doporučuje se použít slovník VCard."@cs)
AnnotationAssertion(rdfs:comment dcat:contactPoint "Relie un jeu de données à une information de contact utile en utilisant VCard."@fr)
AnnotationAssertion(rdfs:comment dcat:contactPoint "Συνδέει ένα σύνολο δεδομένων με ένα σχετικό σημείο επικοινωνίας, μέσω VCard."@el)
AnnotationAssertion(rdfs:comment dcat:contactPoint "تربط قائمة البيانات بعنوان اتصال موصف  باستخدام VCard"@ar)
AnnotationAssertion(rdfs:comment dcat:contactPoint "データセットを、VCardを用いて提供されている適切な連絡先情報にリンクします。"@ja)
AnnotationAssertion(rdfs:isDefinedBy dcat:contactPoint <http://www.w3.org/TR/vocab-dcat/>)
AnnotationAssertion(rdfs:label dcat:contactPoint "Punto de contacto"@es)
AnnotationAssertion(rdfs:label dcat:contactPoint "contact point"@en)
AnnotationAssertion(rdfs:label dcat:contactPoint "kontaktní bod"@cs)
AnnotationAssertion(rdfs:label dcat:contactPoint "kontaktpunkt"@da)
AnnotationAssertion(rdfs:label dcat:contactPoint "point de contact"@fr)
AnnotationAssertion(rdfs:label dcat:contactPoint "punto di contatto"@it)
AnnotationAssertion(rdfs:label dcat:contactPoint "σημείο επικοινωνίας"@el)
AnnotationAssertion(rdfs:label dcat:contactPoint "عنوان اتصال"@ar)
AnnotationAssertion(rdfs:label dcat:contactPoint "窓口"@ja)
AnnotationAssertion(skos:definition dcat:contactPoint "Información relevante de contacto para el recurso catalogado. Se recomienda el uso de vCard."@es)
AnnotationAssertion(skos:definition dcat:contactPoint "Informazioni di contatto rilevanti per la risorsa catalogata. Si raccomanda l'uso di vCard."@it)
AnnotationAssertion(skos:definition dcat:contactPoint "Relevant contact information for the catalogued resource. Use of vCard is recommended."@en)
AnnotationAssertion(skos:definition dcat:contactPoint "Relevante kontaktoplysninger for den katalogiserede ressource. Anvendelse af vCard anbefales."@da)
AnnotationAssertion(skos:definition dcat:contactPoint "Relevantní kontaktní informace pro katalogizovaný zdroj. Doporučuje se použít slovník VCard."@cs)
AnnotationAssertion(skos:definition dcat:contactPoint "Relie un jeu de données à une information de contact utile en utilisant VCard."@fr)
AnnotationAssertion(skos:definition dcat:contactPoint "Συνδέει ένα σύνολο δεδομένων με ένα σχετικό σημείο επικοινωνίας, μέσω VCard."@el)
AnnotationAssertion(skos:definition dcat:contactPoint "تربط قائمة البيانات بعنوان اتصال موصف  باستخدام VCard"@ar)
AnnotationAssertion(skos:definition dcat:contactPoint "データセットを、VCardを用いて提供されている適切な連絡先情報にリンクします。"@ja)
AnnotationAssertion(skos:editorialNote dcat:contactPoint "Status: English Definition text modified by DCAT revision team, Italian, Spanish and Czech translations provided, other translations pending."@en)
ObjectPropertyRange(dcat:contactPoint vcard:Kind)

# Object Property: dcat:dataset (データセット)

AnnotationAssertion(rdfs:comment dcat:dataset "A dataset that is listed in the catalog."@en)
AnnotationAssertion(rdfs:comment dcat:dataset "En samling af data som er opført i kataloget."@da)
AnnotationAssertion(rdfs:comment dcat:dataset "Kolekce dat, která je katalogizována v katalogu."@cs)
AnnotationAssertion(rdfs:comment dcat:dataset "Relie un catalogue à un jeu de données faisant partie de ce catalogue."@fr)
AnnotationAssertion(rdfs:comment dcat:dataset "Un conjunto de datos que se lista en el catálogo."@es)
AnnotationAssertion(rdfs:comment dcat:dataset "Una raccolta di dati che è elencata nel catalogo."@it)
AnnotationAssertion(rdfs:comment dcat:dataset "Συνδέει έναν κατάλογο με ένα σύνολο δεδομένων το οποίο ανήκει στον εν λόγω κατάλογο."@el)
AnnotationAssertion(rdfs:comment dcat:dataset "تربط الفهرس بقائمة بيانات ضمنه"@ar)
AnnotationAssertion(rdfs:comment dcat:dataset "カタログの一部であるデータセット。"@ja)
AnnotationAssertion(rdfs:isDefinedBy dcat:dataset <http://www.w3.org/TR/vocab-dcat/>)
AnnotationAssertion(rdfs:label dcat:dataset "conjunto de datos"@es)
AnnotationAssertion(rdfs:label dcat:dataset "dataset"@en)
AnnotationAssertion(rdfs:label dcat:dataset "dataset"@it)
AnnotationAssertion(rdfs:label dcat:dataset "datasæt"@da)
AnnotationAssertion(rdfs:label dcat:dataset "datová sada"@cs)
AnnotationAssertion(rdfs:label dcat:dataset "jeu de données"@fr)
AnnotationAssertion(rdfs:label dcat:dataset "σύνολο δεδομένων"@el)
AnnotationAssertion(rdfs:label dcat:dataset "قائمة بيانات"@ar)
AnnotationAssertion(rdfs:label dcat:dataset "データセット"@ja)
AnnotationAssertion(skos:altLabel dcat:dataset "datasamling"@da)
AnnotationAssertion(skos:altLabel dcat:dataset "har datasæt"@da)
AnnotationAssertion(skos:altLabel dcat:dataset "has dataset"@en)
AnnotationAssertion(skos:definition dcat:dataset "A dataset that is listed in the catalog."@en)
AnnotationAssertion(skos:definition dcat:dataset "En samling af data som er opført i kataloget."@da)
AnnotationAssertion(skos:definition dcat:dataset "Kolekce dat, která je katalogizována v katalogu."@cs)
AnnotationAssertion(skos:definition dcat:dataset "Relie un catalogue à un jeu de données faisant partie de ce catalogue."@fr)
AnnotationAssertion(skos:definition dcat:dataset "Un conjunto de datos que se lista en el catálogo."@es)
AnnotationAssertion(skos:definition dcat:dataset "Una raccolta di dati che è elencata nel catalogo."@it)
AnnotationAssertion(skos:definition dcat:dataset "Συνδέει έναν κατάλογο με ένα σύνολο δεδομένων το οποίο ανήκει στον εν λόγω κατάλογο."@el)
AnnotationAssertion(skos:definition dcat:dataset "تربط الفهرس بقائمة بيانات ضمنه"@ar)
AnnotationAssertion(skos:definition dcat:dataset "カタログの一部であるデータセット。"@ja)
AnnotationAssertion(skos:editorialNote dcat:dataset "Status: English Definition text modified by DCAT 3 revision team, translations pending."@en)
SubObjectPropertyOf(dcat:dataset dcat:resource)
ObjectPropertyDomain(dcat:dataset dcat:Catalog)
ObjectPropertyRange(dcat:dataset dcat:Dataset)

# Object Property: dcat:distribution (distribution)

AnnotationAssertion(rdfs:comment dcat:distribution "An available distribution of the dataset."@en)
AnnotationAssertion(rdfs:comment dcat:distribution "Connecte un jeu de données à des distributions disponibles."@fr)
AnnotationAssertion(rdfs:comment dcat:distribution "Dostupná distribuce datové sady."@cs)
AnnotationAssertion(rdfs:comment dcat:distribution "En tilgængelig repræsentation af datasættet."@da)
AnnotationAssertion(rdfs:comment dcat:distribution "Una distribución disponible del conjunto de datos."@es)
AnnotationAssertion(rdfs:comment dcat:distribution "Una distribuzione disponibile per il set di dati."@it)
AnnotationAssertion(rdfs:comment dcat:distribution "Συνδέει ένα σύνολο δεδομένων με μία από τις διαθέσιμες διανομές του."@el)
AnnotationAssertion(rdfs:comment dcat:distribution "تربط قائمة البيانات بطريقة أو بشكل يسمح  الوصول الى البيانات"@ar)
AnnotationAssertion(rdfs:comment dcat:distribution "データセットを、その利用可能な配信に接続します。"@ja)
AnnotationAssertion(rdfs:isDefinedBy dcat:distribution <http://www.w3.org/TR/vocab-dcat/>)
AnnotationAssertion(rdfs:label dcat:distribution "distribuce"@cs)
AnnotationAssertion(rdfs:label dcat:distribution "distribución"@es)
AnnotationAssertion(rdfs:label dcat:distribution "distribution"@da)
AnnotationAssertion(rdfs:label dcat:distribution "distribution"@en)
AnnotationAssertion(rdfs:label dcat:distribution "distribution"@fr)
AnnotationAssertion(rdfs:label dcat:distribution "distribuzione"@it)
AnnotationAssertion(rdfs:label dcat:distribution "διανομή"@el)
AnnotationAssertion(rdfs:label dcat:distribution "توزيع"@ar)
AnnotationAssertion(rdfs:label dcat:distribution "データセット配信"@ja)
AnnotationAssertion(skos:altLabel dcat:distribution "har distribution"@da)
AnnotationAssertion(skos:altLabel dcat:distribution "has distribution"@en)
AnnotationAssertion(skos:definition dcat:distribution "An available distribution of the dataset."@en)
AnnotationAssertion(skos:definition dcat:distribution "Connecte un jeu de données à des distributions disponibles."@fr)
AnnotationAssertion(skos:definition dcat:distribution "Dostupná distribuce datové sady."@cs)
AnnotationAssertion(skos:definition dcat:distribution "En tilgængelig repræsentation af datasættet."@da)
AnnotationAssertion(skos:definition dcat:distribution "Una distribución disponible del conjunto de datos."@es)
AnnotationAssertion(skos:definition dcat:distribution "Una distribuzione disponibile per il set di dati."@it)
AnnotationAssertion(skos:definition dcat:distribution "Συνδέει ένα σύνολο δεδομένων με μία από τις διαθέσιμες διανομές του."@el)
AnnotationAssertion(skos:definition dcat:distribution "تربط قائمة البيانات بطريقة أو بشكل يسمح  الوصول الى البيانات"@ar)
AnnotationAssertion(skos:definition dcat:distribution "データセットを、その利用可能な配信に接続します。"@ja)
AnnotationAssertion(skos:editorialNote dcat:distribution "Status: English Definition text modified by DCAT revision team, translations pending (except for Italian, Spanish and Czech)."@en)
SubObjectPropertyOf(dcat:distribution dcterms:relation)
InverseObjectProperties(dcat:distribution dcat:isDistributionOf)
ObjectPropertyDomain(dcat:distribution dcat:Dataset)
ObjectPropertyRange(dcat:distribution dcat:Distribution)

# Object Property: dcat:downloadURL (رابط تحميل)

AnnotationAssertion(rdfs:comment dcat:downloadURL "Ceci est un lien direct à un fichier téléchargeable en un format donnée. Exple fichier CSV ou RDF. Le format est décrit par les propriétés de distribution dcterms:format et/ou dcat:mediaType."@fr)
AnnotationAssertion(rdfs:comment dcat:downloadURL "La URL de un archivo descargable en el formato dato. Por ejemplo, archivo CSV o archivo RDF. El formato se describe con las propiedades de la distribución dcterms:format y/o dcat:mediaType."@es)
AnnotationAssertion(rdfs:comment dcat:downloadURL "Questo è un link diretto al file scaricabile in un dato formato. E.g. un file CSV o un file RDF. Il formato è descritto dal dcterms:format e/o dal dcat:mediaType della distribuzione."@it)
AnnotationAssertion(rdfs:comment dcat:downloadURL "The URL of the downloadable file in a given format. E.g. CSV file or RDF file. The format is indicated by the distribution's dcterms:format and/or dcat:mediaType."@en)
AnnotationAssertion(rdfs:comment dcat:downloadURL "URL souboru ke stažení v daném formátu, například CSV nebo RDF soubor. Formát je popsán vlastností distribuce dcterms:format a/nebo dcat:mediaType."@cs)
AnnotationAssertion(rdfs:comment dcat:downloadURL "URL til fil der kan downloades i et bestemt format. Fx en CSV-fil eller en RDF-fil. Formatet for distributionen angives ved hjælp af egenskaberne dcterms:format og/eller dcat:mediaType."@da)
AnnotationAssertion(rdfs:comment dcat:downloadURL "dcat:downloadURLはdcat:accessURLの特定の形式です。しかし、DCATプロファイルが非ダウンロード・ロケーションに対してのみaccessURLを用いる場合には、より強い分離を課すことを望む可能性があるため、この含意を強化しないように、DCATは、dcat:downloadURLをdcat:accessURLのサブプロパティーであると定義しません。"@ja)
AnnotationAssertion(rdfs:comment dcat:downloadURL "Είναι ένας σύνδεσμος άμεσης μεταφόρτωσης ενός αρχείου σε μια δεδομένη μορφή. Π.χ. ένα αρχείο CSV ή RDF. Η μορφη αρχείου περιγράφεται από τις ιδιότητες dcterms:format ή/και dcat:mediaType της διανομής."@el)
AnnotationAssertion(rdfs:comment dcat:downloadURL "رابط مباشر لملف يمكن تحميله. نوع الملف يتم توصيفه باستخدام الخاصية dcterms:format dcat:mediaType "@ar)
AnnotationAssertion(rdfs:isDefinedBy dcat:downloadURL <http://www.w3.org/TR/vocab-dcat/>)
AnnotationAssertion(rdfs:label dcat:downloadURL "URL de descarga"@es)
AnnotationAssertion(rdfs:label dcat:downloadURL "URL de téléchargement"@fr)
AnnotationAssertion(rdfs:label dcat:downloadURL "URL di scarico"@it)
AnnotationAssertion(rdfs:label dcat:downloadURL "URL souboru ke stažení"@cs)
AnnotationAssertion(rdfs:label dcat:downloadURL "URL μεταφόρτωσης"@el)
AnnotationAssertion(rdfs:label dcat:downloadURL "download URL"@en)
AnnotationAssertion(rdfs:label dcat:downloadURL "downloadURL"@da)
AnnotationAssertion(rdfs:label dcat:downloadURL "رابط تحميل"@ar)
AnnotationAssertion(rdfs:label dcat:downloadURL "ダウンロードURL"@ja)
AnnotationAssertion(skos:definition dcat:downloadURL "Ceci est un lien direct à un fichier téléchargeable en un format donnée. Exple fichier CSV ou RDF. Le format est décrit par les propriétés de distribution dcterms:format et/ou dcat:mediaType."@fr)
AnnotationAssertion(skos:definition dcat:downloadURL "La URL de un archivo descargable en el formato dato. Por ejemplo, archivo CSV o archivo RDF. El formato se describe con las propiedades de la distribución dcterms:format y/o dcat:mediaType."@es)
AnnotationAssertion(skos:definition dcat:downloadURL "Questo è un link diretto al file scaricabile in un dato formato. E.g. un file CSV o un file RDF. Il formato è descritto dal dcterms:format e/o dal dcat:mediaType della distribuzione."@it)
AnnotationAssertion(skos:definition dcat:downloadURL "The URL of the downloadable file in a given format. E.g. CSV file or RDF file. The format is indicated by the distribution's dcterms:format and/or dcat:mediaType."@en)
AnnotationAssertion(skos:definition dcat:downloadURL "URL souboru ke stažení v daném formátu, například CSV nebo RDF soubor. Formát je popsán vlastností distribuce dcterms:format a/nebo dcat:mediaType."@cs)
AnnotationAssertion(skos:definition dcat:downloadURL "URL til fil der kan downloades i et bestemt format. Fx en CSV-fil eller en RDF-fil. Formatet for distributionen angives ved hjælp af egenskaberne dcterms:format og/eller dcat:mediaType."@da)
AnnotationAssertion(skos:definition dcat:downloadURL "dcat:downloadURLはdcat:accessURLの特定の形式です。しかし、DCATプロファイルが非ダウンロード・ロケーションに対してのみaccessURLを用いる場合には、より強い分離を課すことを望む可能性があるため、この含意を強化しないように、DCATは、dcat:downloadURLをdcat:accessURLのサブプロパティーであると定義しません。"@ja)
AnnotationAssertion(skos:definition dcat:downloadURL "Είναι ένας σύνδεσμος άμεσης μεταφόρτωσης ενός αρχείου σε μια δεδομένη μορφή. Π.χ. ένα αρχείο CSV ή RDF. Η μορφη αρχείου περιγράφεται από τις ιδιότητες dcterms:format ή/και dcat:mediaType της διανομής."@el)
AnnotationAssertion(skos:definition dcat:downloadURL "رابط مباشر لملف يمكن تحميله. نوع الملف يتم توصيفه باستخدام الخاصية dcterms:format dcat:mediaType "@ar)
AnnotationAssertion(skos:editorialNote dcat:downloadURL "Status: English  Definition text modified by DCAT revision team, Italian, Spanish and Czech translation updated, other translations pending."@en)
AnnotationAssertion(skos:editorialNote dcat:downloadURL "rdfs:label, rdfs:comment and/or skos:scopeNote have been modified. Non-english versions must be updated."@en)
AnnotationAssertion(skos:scopeNote dcat:downloadURL "El valor es una URL."@es)
AnnotationAssertion(skos:scopeNote dcat:downloadURL "La valeur est une URL."@fr)
AnnotationAssertion(skos:scopeNote dcat:downloadURL "dcat:downloadURL BY MĚLA být použita pro adresu, ze které je distribuce přímo přístupná, typicky skrze požadavek HTTP Get."@cs)
AnnotationAssertion(skos:scopeNote dcat:downloadURL "dcat:downloadURL BØR anvendes til angivelse af den adresse hvor distributionen er tilgængelig direkte, typisk gennem et HTTP Get request."@da)
AnnotationAssertion(skos:scopeNote dcat:downloadURL "dcat:downloadURL DOVREBBE essere utilizzato per l'indirizzo a cui questa distribuzione è disponibile direttamente, in genere attraverso una richiesta Get HTTP."@it)
AnnotationAssertion(skos:scopeNote dcat:downloadURL "dcat:downloadURL SHOULD be used for the address at which this distribution is available directly, typically through a HTTP Get request."@en)
AnnotationAssertion(skos:scopeNote dcat:downloadURL "Η τιμή είναι ένα URL."@el)
ObjectPropertyDomain(dcat:downloadURL dcat:Distribution)
ObjectPropertyRange(dcat:downloadURL rdfs:Resource)

# Object Property: dcat:endpointDescription (descripción del end-point del servicio)

AnnotationAssertion(rdfs:comment dcat:endpointDescription "A description of the service end-point, including its operations, parameters etc."@en)
AnnotationAssertion(rdfs:comment dcat:endpointDescription "En beskrivelse af det pågældende tjenesteendpoint, inklusiv dets operationer, parametre etc."@da)
AnnotationAssertion(rdfs:comment dcat:endpointDescription "Popis přístupového bodu služby včetně operací, parametrů apod."@cs)
AnnotationAssertion(rdfs:comment dcat:endpointDescription "Una descripción del end-point del servicio, incluyendo sus operaciones, parámetros, etc."@es)
AnnotationAssertion(rdfs:comment dcat:endpointDescription "Una descrizione dell'endpoint del servizio, incluse le sue operazioni, parametri, ecc."@it)
AnnotationAssertion(rdfs:isDefinedBy dcat:endpointDescription <https://www.w3.org/TR/vocab-dcat-2/>)
AnnotationAssertion(rdfs:label dcat:endpointDescription "descripción del end-point del servicio"@es)
AnnotationAssertion(rdfs:label dcat:endpointDescription "description of service end-point"@en)
AnnotationAssertion(rdfs:label dcat:endpointDescription "descrizione dell'endpoint del servizio"@it)
AnnotationAssertion(rdfs:label dcat:endpointDescription "endpointbeskrivelse"@da)
AnnotationAssertion(rdfs:label dcat:endpointDescription "popis přístupového bodu služby"@cs)
AnnotationAssertion(skos:changeNote dcat:endpointDescription "New property in DCAT 2."@en)
AnnotationAssertion(skos:changeNote dcat:endpointDescription "Nová vlastnost přidaná ve verzi DCAT 2."@cs)
AnnotationAssertion(skos:changeNote dcat:endpointDescription "Nueva propiedad agregada en DCAT 2."@en)
AnnotationAssertion(skos:changeNote dcat:endpointDescription "Nuova proprietà in DCAT 2."@it)
AnnotationAssertion(skos:changeNote dcat:endpointDescription "Ny egenskab i DCAT 2."@da)
AnnotationAssertion(skos:definition dcat:endpointDescription "A description of the service end-point, including its operations, parameters etc."@en)
AnnotationAssertion(skos:definition dcat:endpointDescription "En beskrivelse af det pågældende tjenesteendpoint, inklusiv dets operationer, parametre etc."@da)
AnnotationAssertion(skos:definition dcat:endpointDescription "Popis přístupového bodu služby včetně operací, parametrů apod."@cs)
AnnotationAssertion(skos:definition dcat:endpointDescription "Una descripción del end-point del servicio, incluyendo sus operaciones, parámetros, etc.."@es)
AnnotationAssertion(skos:definition dcat:endpointDescription "Una descrizione dell'endpoint del servizio, incluse le sue operazioni, parametri, ecc."@it)
AnnotationAssertion(skos:scopeNote dcat:endpointDescription "An endpoint description may be expressed in a machine-readable form, such as an OpenAPI (Swagger) description, an OGC GetCapabilities response, a SPARQL Service Description, an OpenSearch or WSDL document, a Hydra API description, else in text or some other informal mode if a formal representation is not possible."@en)
AnnotationAssertion(skos:scopeNote dcat:endpointDescription "En beskrivelse af et endpoint kan udtrykkes i et maskinlæsbart format, såsom OpenAPI (Swagger)-beskrivelser, et OGC GetCapabilities svar, en SPARQL tjenestebeskrivelse, en OpenSearch- eller et WSDL-dokument, en Hydra-API-beskrivelse, eller i tekstformat eller i et andet uformelt format, hvis en formel repræsentation ikke er mulig."@da)
AnnotationAssertion(skos:scopeNote dcat:endpointDescription "Endpointbeskrivelsen giver specifikke oplysninger om den konkrete endpointinstans, mens dcterms:conformsTo anvendes til at indikere den overordnede standard eller specifikation som endpointet er i overensstemmelse med."@da)
AnnotationAssertion(skos:scopeNote dcat:endpointDescription "La descripción del endpoint brinda detalles específicos de la instancia del endpoint, mientras que dcterms:conformsTo se usa para indicar el estándar general o especificación que implementa el endpoint."@es)
AnnotationAssertion(skos:scopeNote dcat:endpointDescription "La descrizione dell'endpoint fornisce dettagli specifici dell'istanza dell'endpoint reale, mentre dcterms:conformsTo viene utilizzato per indicare lo standard o le specifiche implementate dall'endpoint."@it)
AnnotationAssertion(skos:scopeNote dcat:endpointDescription "Popis přístupového bodu dává specifické detaily jeho konkrétní instance, zatímco dcterms:conformsTo indikuje obecný standard či specifikaci kterou přístupový bod implementuje."@cs)
AnnotationAssertion(skos:scopeNote dcat:endpointDescription "Popis přístupového bodu může být vyjádřen ve strojově čitelné formě, například jako popis OpenAPI (Swagger), odpověď služby OGC getCapabilities, pomocí slovníku SPARQL Service Description, jako OpenSearch či WSDL document, jako popis API dle slovníku Hydra, a nebo textově nebo jiným neformálním způsobem, pokud není možno použít formální reprezentaci."@cs)
AnnotationAssertion(skos:scopeNote dcat:endpointDescription "The endpoint description gives specific details of the actual endpoint instance, while dcterms:conformsTo is used to indicate the general standard or specification that the endpoint implements."@en)
AnnotationAssertion(skos:scopeNote dcat:endpointDescription "Una descripción del endpoint del servicio puede expresarse en un formato que la máquina puede interpretar, tal como una descripción basada en OpenAPI (Swagger), una respuesta OGC GetCapabilities, una descripción de un servicio SPARQL, un documento OpenSearch o WSDL, una descripción con la Hydra API, o en texto u otro modo informal si la representación formal no es posible."@es)
AnnotationAssertion(skos:scopeNote dcat:endpointDescription "Una descrizione dell'endpoint può essere espressa in un formato leggibile dalla macchina, come una descrizione OpenAPI (Swagger), una risposta GetCapabilities OGC, una descrizione del servizio SPARQL, un documento OpenSearch o WSDL, una descrizione API Hydra, o con del testo o qualche altra modalità informale se una rappresentazione formale non è possibile."@it)
ObjectPropertyDomain(dcat:endpointDescription dcat:DataService)

# Object Property: dcat:endpointURL (end-point del servicio)

AnnotationAssertion(rdfs:comment dcat:endpointURL "Kořenové umístění nebo hlavní přístupový bod služby (IRI přístupné přes Web)."@cs)
AnnotationAssertion(rdfs:comment dcat:endpointURL "La locazione principale o l'endpoint primario del servizio (un IRI risolvibile via web)."@it)
AnnotationAssertion(rdfs:comment dcat:endpointURL "La posición raíz o end-point principal del servicio (una IRI web)."@es)
AnnotationAssertion(rdfs:comment dcat:endpointURL "Rodplaceringen eller det primære endpoint for en tjeneste (en web-resolverbar IRI)."@da)
AnnotationAssertion(rdfs:comment dcat:endpointURL "The root location or primary endpoint of the service (a web-resolvable IRI)."@en)
AnnotationAssertion(rdfs:isDefinedBy dcat:endpointURL <https://www.w3.org/TR/vocab-dcat-2/>)
AnnotationAssertion(rdfs:label dcat:endpointURL "end-point del servicio"@es)
AnnotationAssertion(rdfs:label dcat:endpointURL "end-point del servizio"@it)
AnnotationAssertion(rdfs:label dcat:endpointURL "přístupový bod služby"@cs)
AnnotationAssertion(rdfs:label dcat:endpointURL "service end-point"@en)
AnnotationAssertion(rdfs:label dcat:endpointURL "tjenesteendpoint"@da)
AnnotationAssertion(skos:changeNote dcat:endpointURL "New property in DCAT 2."@en)
AnnotationAssertion(skos:changeNote dcat:endpointURL "Nová vlastnost přidaná ve verzi DCAT 2."@cs)
AnnotationAssertion(skos:changeNote dcat:endpointURL "Nueva propiedad agregada en DCAT 2."@es)
AnnotationAssertion(skos:changeNote dcat:endpointURL "Nuova proprietà in DCAT 2."@it)
AnnotationAssertion(skos:definition dcat:endpointURL "Kořenové umístění nebo hlavní přístupový bod služby (IRI přístupné přes Web)."@cs)
AnnotationAssertion(skos:definition dcat:endpointURL "La locazione principale o l'endpoint primario del servizio (un IRI risolvibile via web)."@it)
AnnotationAssertion(skos:definition dcat:endpointURL "La posición raíz o end-point principal del servicio (una IRI web)."@es)
AnnotationAssertion(skos:definition dcat:endpointURL "Rodplaceringen eller det primære endpoint for en tjeneste (en web-resolverbar IRI)."@da)
AnnotationAssertion(skos:definition dcat:endpointURL "The root location or primary endpoint of the service (a web-resolvable IRI)."@en)
ObjectPropertyDomain(dcat:endpointURL dcat:DataService)
ObjectPropertyRange(dcat:endpointURL rdfs:Resource)

# Object Property: dcat:first (primo)

AnnotationAssertion(rdfs:comment dcat:first "El primer recurso en una colección ordenada o serie de recursos, al que el recurso pertenece."@es)
AnnotationAssertion(rdfs:comment dcat:first "La prima risorsa in una collezione ordinata o in una serie di risorse, di cui la risorsa fa parte."@it)
AnnotationAssertion(rdfs:comment dcat:first "The first resource in an ordered collection or series of resources, to which the current resource belongs."@en)
AnnotationAssertion(rdfs:isDefinedBy dcat:first <https://www.w3.org/TR/vocab-dcat-3/>)
AnnotationAssertion(rdfs:label dcat:first "first"@en)
AnnotationAssertion(rdfs:label dcat:first "primero"@es)
AnnotationAssertion(rdfs:label dcat:first "primo"@it)
AnnotationAssertion(skos:changeNote dcat:first "New property added in DCAT 3."@en)
AnnotationAssertion(skos:changeNote dcat:first "Nová vlastnost přidaná ve verzi DCAT 3."@cs)
AnnotationAssertion(skos:changeNote dcat:first "Nueva propiedad agregada in DCAT 3."@es)
AnnotationAssertion(skos:changeNote dcat:first "Nuova proprietà aggiunta in DCAT 3."@it)
AnnotationAssertion(skos:changeNote dcat:first "Ny egenskab tilføjet i DCAT 3."@da)
AnnotationAssertion(skos:definition dcat:first "El primer recurso en una colección ordenada o serie de recursos, al que el recurso pertenece."@es)
AnnotationAssertion(skos:definition dcat:first "La prima risorsa in una collezione ordinata o in una serie di risorse, di cui la risorsa fa parte."@it)
AnnotationAssertion(skos:definition dcat:first "The first resource in an ordered collection or series of resources, to which the current resource belongs."@en)
AnnotationAssertion(skos:scopeNote dcat:first "En DCAT esta propiedad se usa para recursos que pertenecen a una dcat:DatasetSeries."@es)
AnnotationAssertion(skos:scopeNote dcat:first "In DCAT questa proprietà è usata per risorse che fanno parte di una dcat:DatasetSeries."@it)
AnnotationAssertion(skos:scopeNote dcat:first "In DCAT this property is used for resources belonging to a dcat:DatasetSeries."@en)
SubObjectPropertyOf(dcat:first xhv:first)

# Object Property: dcat:hadRole (tiene rol)

AnnotationAssertion(rdfs:comment dcat:hadRole "Den funktion en entitet eller aktør har i forhold til en anden ressource."@da)
AnnotationAssertion(rdfs:comment dcat:hadRole "Funkce entity či agenta ve vztahu k jiné entitě či zdroji."@cs)
AnnotationAssertion(rdfs:comment dcat:hadRole "La función de una entidad o agente con respecto a otra entidad o recurso."@es)
AnnotationAssertion(rdfs:comment dcat:hadRole "La funzione di un'entità o un agente rispetto ad un'altra entità o risorsa."@it)
AnnotationAssertion(rdfs:comment dcat:hadRole "The function of an entity or agent with respect to another entity or resource."@en)
AnnotationAssertion(rdfs:isDefinedBy dcat:hadRole <https://www.w3.org/TR/vocab-dcat-2/>)
AnnotationAssertion(rdfs:label dcat:hadRole "haRuolo"@it)
AnnotationAssertion(rdfs:label dcat:hadRole "hadRole"@en)
AnnotationAssertion(rdfs:label dcat:hadRole "havde rolle"@da)
AnnotationAssertion(rdfs:label dcat:hadRole "sehraná role"@cs)
AnnotationAssertion(rdfs:label dcat:hadRole "tiene rol"@it)
AnnotationAssertion(skos:changeNote dcat:hadRole "New property added in DCAT 2."@en)
AnnotationAssertion(skos:changeNote dcat:hadRole "Nová vlastnost přidaná ve verzi DCAT 2."@cs)
AnnotationAssertion(skos:changeNote dcat:hadRole "Nueva propiedad agregada en DCAT 2."@es)
AnnotationAssertion(skos:changeNote dcat:hadRole "Nuova proprietà aggiunta in DCAT 2."@it)
AnnotationAssertion(skos:definition dcat:hadRole "Den funktion en entitet eller aktør har i forhold til en anden ressource."@da)
AnnotationAssertion(skos:definition dcat:hadRole "Funkce entity či agenta ve vztahu k jiné entitě či zdroji."@cs)
AnnotationAssertion(skos:definition dcat:hadRole "La función de una entidad o agente con respecto a otra entidad o recurso."@es)
AnnotationAssertion(skos:definition dcat:hadRole "La funzione di un'entità o un agente rispetto ad un'altra entità o risorsa."@it)
AnnotationAssertion(skos:definition dcat:hadRole "The function of an entity or agent with respect to another entity or resource."@en)
AnnotationAssertion(skos:editorialNote dcat:hadRole "Agregada en DCAT para complementar prov:hadRole (cuyo uso está limitado a roles en el contexto de una actividad, con dominio prov:Association."@es)
AnnotationAssertion(skos:editorialNote dcat:hadRole "Introdotta in DCAT per completare prov:hadRole (il cui uso è limitato ai ruoli nel contesto di un'attività, con il dominio di prov:Association."@it)
AnnotationAssertion(skos:editorialNote dcat:hadRole "Introduced into DCAT to complement prov:hadRole (whose use is limited to roles in the context of an activity, with the domain of prov:Association."@en)
AnnotationAssertion(skos:editorialNote dcat:hadRole "Introduceret i DCAT for at supplere prov:hadRole (hvis anvendelse er begrænset til roller i forbindelse med en aktivitet med domænet prov:Association)."@da)
AnnotationAssertion(skos:editorialNote dcat:hadRole "Přidáno do DCAT pro doplnění vlastnosti prov:hadRole (jejíž užití je omezeno na role v kontextu aktivity, s definičním oborem prov:Association)."@cs)
AnnotationAssertion(skos:scopeNote dcat:hadRole "Kan vendes ved kvalificerede krediteringer til at angive en aktørs rolle i forhold en entitet. Det anbefales at værdierne styres som et kontrolleret udfaldsrum med aktørroller, såsom http://registry.it.csiro.au/def/isotc211/CI_RoleCode."@da)
AnnotationAssertion(skos:scopeNote dcat:hadRole "May be used in a qualified-attribution to specify the role of an Agent with respect to an Entity. It is recommended that the value be taken from a controlled vocabulary of agent roles, such as http://registry.it.csiro.au/def/isotc211/CI_RoleCode."@en)
AnnotationAssertion(skos:scopeNote dcat:hadRole "May be used in a qualified-relation to specify the role of an Entity with respect to another Entity.  It is recommended that the value be taken from a controlled vocabulary of entity roles such as: ISO 19115 DS_AssociationTypeCode http://registry.it.csiro.au/def/isotc211/DS_AssociationTypeCode; IANA Registry of Link Relations https://www.iana.org/assignments/link-relation; DataCite metadata schema; MARC relators https://id.loc.gov/vocabulary/relators."@en)
AnnotationAssertion(skos:scopeNote dcat:hadRole "Může být použito v kvalifikovaném přiřazení pro specifikaci role Agenta ve vztahu k Entitě. Je doporučeno hodnotu vybrat z řízeného slovníku rolí agentů, jako například http://registry.it.csiro.au/def/isotc211/CI_RoleCode."@cs)
AnnotationAssertion(skos:scopeNote dcat:hadRole "Může být použito v kvalifikovaném vztahu pro specifikaci role Entity ve vztahu k jiné Entitě. Je doporučeno použít hodnotu z řízeného slovníku rolí entit, jako například ISO 19115 DS_AssociationTypeCode http://registry.it.csiro.au/def/isotc211/DS_AssociationTypeCode, IANA Registry of Link Relations https://www.iana.org/assignments/link-relation, DataCite metadata schema, MARC relators https://id.loc.gov/vocabulary/relators."@cs)
AnnotationAssertion(skos:scopeNote dcat:hadRole "Puede usarse en una atribución cualificada para especificar el rol de un Agente con respecto a una Entidad. Se recomienda que el valor sea de un vocabulario controlado de roles de agentes, como por ejemplo http://registry.it.csiro.au/def/isotc211/CI_RoleCode."@es)
AnnotationAssertion(skos:scopeNote dcat:hadRole "Puede usarse en una atribución cualificada para especificar el rol de una Entidad con respecto a otra Entidad. Se recomienda que su valor se tome de un vocabulario controlado de roles de entidades como por ejemplo: ISO 19115 DS_AssociationTypeCode http://registry.it.csiro.au/def/isotc211/DS_AssociationTypeCode; IANA Registry of Link Relations https://www.iana.org/assignments/link-relation; esquema de metadatos de DataCite; MARC relators https://id.loc.gov/vocabulary/relators."@es)
AnnotationAssertion(skos:scopeNote dcat:hadRole "Può essere utilizzata in una relazione qualificata per specificare il ruolo di un'entità rispetto a un'altra entità. Si raccomanda che il valore sia preso da un vocabolario controllato di ruoli di entità come ISO 19115 DS_AssociationTypeCode http://registry.it.csiro.au/def/isotc211/DS_AssociationTypeCode, IANA Registry of Link Relations https://www.iana.org/assignments/link-relation, DataCite metadata schema, o MARC relators https://id.loc.gov/vocabulary/relators."@it)
AnnotationAssertion(skos:scopeNote dcat:hadRole "Può essere utilizzato in un'attribuzione qualificata per specificare il ruolo di un agente rispetto a un'entità. Si raccomanda che il valore sia preso da un vocabolario controllato di ruoli di agente, come ad esempio http://registry.it.csiro.au/def/isotc211/CI_RoleCode."@it)
ObjectPropertyDomain(dcat:hadRole ObjectUnionOf(dcat:Relationship prov:Attribution))
ObjectPropertyRange(dcat:hadRole dcat:Role)

# Object Property: dcat:hasCurrentVersion (tiene versión actual)

AnnotationAssertion(rdfs:comment dcat:hasCurrentVersion "Este recurso es más específico y versionado con contenido equivalente [PAV]."@es)
AnnotationAssertion(rdfs:comment dcat:hasCurrentVersion "Per questa risorsa esiste una risorsa più specifica e versionata, ma con lo stesso contenuto."@it)
AnnotationAssertion(rdfs:comment dcat:hasCurrentVersion "This resource has a more specific, versioned resource with equivalent content [PAV]."@en)
AnnotationAssertion(rdfs:isDefinedBy dcat:hasCurrentVersion <https://www.w3.org/TR/vocab-dcat-3/>)
AnnotationAssertion(rdfs:label dcat:hasCurrentVersion "ha versione attuale"@it)
AnnotationAssertion(rdfs:label dcat:hasCurrentVersion "has current version"@en)
AnnotationAssertion(rdfs:label dcat:hasCurrentVersion "tiene versión actual"@es)
AnnotationAssertion(skos:changeNote dcat:hasCurrentVersion "New property added in DCAT 3."@en)
AnnotationAssertion(skos:changeNote dcat:hasCurrentVersion "Nová vlastnost přidaná ve verzi DCAT 3."@cs)
AnnotationAssertion(skos:changeNote dcat:hasCurrentVersion "Nueva propiedad agregada in DCAT 3."@es)
AnnotationAssertion(skos:changeNote dcat:hasCurrentVersion "Nuova proprietà aggiunta in DCAT 3."@it)
AnnotationAssertion(skos:changeNote dcat:hasCurrentVersion "Ny egenskab tilføjet i DCAT 3."@da)
AnnotationAssertion(skos:definition dcat:hasCurrentVersion "Este recurso es más específico y versionado con contenido equivalente [PAV]."@es)
AnnotationAssertion(skos:definition dcat:hasCurrentVersion "Per questa risorsa esiste una risorsa più specifica e versionata, ma con lo stesso contenuto."@it)
AnnotationAssertion(skos:definition dcat:hasCurrentVersion "This resource has a more specific, versioned resource with equivalent content [PAV]."@en)
AnnotationAssertion(skos:scopeNote dcat:hasCurrentVersion "Esta propepiedad está destinada a relacionar un recurso no versionado o abstracto con una versión instantánea que puede usarse como un enlace permanente a la versión actual del recurso [PAV]."@es)
AnnotationAssertion(skos:scopeNote dcat:hasCurrentVersion "La noción de versión que se usa en esta propiedad está limitada a las versiones que resultan de revisiones de un recurso como parte de su ciclo de vida."@es)
AnnotationAssertion(skos:scopeNote dcat:hasCurrentVersion "La nozione di versione usata da questa proprietà è limitata a versioni risultanti da revisioni a cui una risorsa è soggetta nel suo ciclo di vita."@it)
AnnotationAssertion(skos:scopeNote dcat:hasCurrentVersion "Questa proprietà è usata per correlare una risorsa non versionata o astratta a un suo specifico snapshot che può essere usato come permalink per indicare la versione attuale del suo contenuto."@it)
AnnotationAssertion(skos:scopeNote dcat:hasCurrentVersion "The notion of version used by this property is limited to versions resulting from revisions occurring to a resource as part of its life-cycle."@en)
AnnotationAssertion(skos:scopeNote dcat:hasCurrentVersion "This property is intended for relating a non-versioned or abstract resource to a single snapshot that can be used as a permalink to indicate the current version of the content [PAV]."@en)
SubObjectPropertyOf(dcat:hasCurrentVersion pav:hasVersion)

# Object Property: dcat:hasVersion (has version)

AnnotationAssertion(rdfs:comment dcat:hasVersion "Este recurso tiene una versión específica."@es)
AnnotationAssertion(rdfs:comment dcat:hasVersion "Per questa risorsa esiste una risorsa più specifica e versionata."@it)
AnnotationAssertion(rdfs:comment dcat:hasVersion "This resource has a more specific, versioned resource [PAV]."@en)
AnnotationAssertion(rdfs:isDefinedBy dcat:hasVersion <https://www.w3.org/TR/vocab-dcat-3/>)
AnnotationAssertion(rdfs:label dcat:hasVersion "ha versione"@it)
AnnotationAssertion(rdfs:label dcat:hasVersion "has version"@en)
AnnotationAssertion(rdfs:label dcat:hasVersion "tiene versión"@es)
AnnotationAssertion(skos:changeNote dcat:hasVersion "New property added in DCAT 3."@en)
AnnotationAssertion(skos:changeNote dcat:hasVersion "Nová vlastnost přidaná ve verzi DCAT 3."@cs)
AnnotationAssertion(skos:changeNote dcat:hasVersion "Nueva propiedad agregada in DCAT 3."@es)
AnnotationAssertion(skos:changeNote dcat:hasVersion "Nuova proprietà aggiunta in DCAT 3."@it)
AnnotationAssertion(skos:changeNote dcat:hasVersion "Ny egenskab tilføjet i DCAT 3."@da)
AnnotationAssertion(skos:definition dcat:hasVersion "Este recurso tiene una versión específica."@es)
AnnotationAssertion(skos:definition dcat:hasVersion "Per questa risorsa esiste una risorsa più specifica e versionata."@it)
AnnotationAssertion(skos:definition dcat:hasVersion "This resource has a more specific, versioned resource [PAV]."@en)
AnnotationAssertion(skos:scopeNote dcat:hasVersion "Esta propiedad se utiliza para relacionar un recurso abstracto o no versionado de un recurso con varias versiones del recuros; por ejemplo, versiones intastáneas."@es)
AnnotationAssertion(skos:scopeNote dcat:hasVersion "La noción de versión que se usa en esta propiedad está limitada a las versiones que resultan de revisiones de un recurso como parte de su ciclo de vida. Por lo tanto, su semántica es más específica que su super-propiedad dcterns:hasVersion, la cuál hace uso de la noción más amplia de versión, incluyendo ediciones y adaptaciones."@es)
AnnotationAssertion(skos:scopeNote dcat:hasVersion "La nozione di versione usata da questa proprietà è limitata a versioni risultanti da revisioni a cui una risorsa è soggetta nel suo ciclo di vita. Quindi la sua semantica è più specifica di quella della sua super-proprietà dcterms:hasVersion, che utilizza una nozione di versione più ampia, e include, ad es., edizioni e adattamenti."@it)
AnnotationAssertion(skos:scopeNote dcat:hasVersion "Questa proprietà è usata per correlare una risorsa non versionata o astratta a differenti risorse versionate, ad es., i relativi snapshot."@it)
AnnotationAssertion(skos:scopeNote dcat:hasVersion "The notion of version used by this property is limited to versions resulting from revisions occurring to a resource as part of its life-cycle. Therefore, its semantics is more specific than its super-property dcterms:hasVersion, which makes use of a broader notion of version, including editions and adaptations."@en)
AnnotationAssertion(skos:scopeNote dcat:hasVersion "This property is intended for relating a non-versioned or abstract resource to several versioned resources, e.g., snapshots [PAV]."@en)
SubObjectPropertyOf(dcat:hasVersion dcterms:hasVersion)
SubObjectPropertyOf(dcat:hasVersion prov:generalizationOf)
InverseObjectProperties(dcat:hasVersion dcat:isVersionOf)

# Object Property: dcat:inCatalog (dcat:inCatalog)

AnnotationAssertion(rdfs:isDefinedBy dcat:inCatalog <https://www.w3.org/TR/vocab-dcat-3/>)
AnnotationAssertion(skos:changeNote dcat:inCatalog "New property added in DCAT 3."@en)
AnnotationAssertion(skos:changeNote dcat:inCatalog "Nová vlastnost přidaná ve verzi DCAT 3."@cs)
AnnotationAssertion(skos:changeNote dcat:inCatalog "Nueva propiedad agregada en DCAT 3."@es)
AnnotationAssertion(skos:changeNote dcat:inCatalog "Nuova proprietà aggiunta in DCAT 3."@it)
AnnotationAssertion(skos:scopeNote dcat:inCatalog "Esta propiedad inversa PUEDE usarse sólo en combinación con su inversa, y NO PUEDE utilizarse en su reemplazo."@es)
AnnotationAssertion(skos:scopeNote dcat:inCatalog "Questa proprietà PUÒ essere usata solo insieme alla sua inversa, e NON DEVE essere usata per sostituirla."@it)
AnnotationAssertion(skos:scopeNote dcat:inCatalog "This property MAY be used only in addition to its inverse, and it MUST NOT be used to replace it."@en)
InverseObjectProperties(dcat:inCatalog dcat:resource)

# Object Property: dcat:inSeries (in series)

AnnotationAssertion(rdfs:comment dcat:inSeries "A dataset series of which the dataset is part."@en)
AnnotationAssertion(rdfs:comment dcat:inSeries "Una serie de conjuntos de datos del cuál un conjunto de datos es parte."@es)
AnnotationAssertion(rdfs:comment dcat:inSeries "Una serie di dataset di cui questo dataset fa parte."@it)
AnnotationAssertion(rdfs:isDefinedBy dcat:inSeries <https://www.w3.org/TR/vocab-dcat-3/>)
AnnotationAssertion(rdfs:label dcat:inSeries "en serie"@es)
AnnotationAssertion(rdfs:label dcat:inSeries "in serie"@it)
AnnotationAssertion(rdfs:label dcat:inSeries "in series"@en)
AnnotationAssertion(skos:changeNote dcat:inSeries "New property added in DCAT 3."@en)
AnnotationAssertion(skos:changeNote dcat:inSeries "Nová vlastnost přidaná ve verzi DCAT 3."@cs)
AnnotationAssertion(skos:changeNote dcat:inSeries "Nueva propiedad agregada in DCAT 3."@es)
AnnotationAssertion(skos:changeNote dcat:inSeries "Nuova proprietà aggiunta in DCAT 3."@it)
AnnotationAssertion(skos:changeNote dcat:inSeries "Ny egenskab tilføjet i DCAT 3."@da)
AnnotationAssertion(skos:definition dcat:inSeries "A dataset series of which the dataset is part."@en)
AnnotationAssertion(skos:definition dcat:inSeries "Una serie de conjuntos de datos del cuál un conjunto de datos es parte."@es)
AnnotationAssertion(skos:definition dcat:inSeries "Una serie di dataset di cui questo dataset fa parte."@it)
SubObjectPropertyOf(dcat:inSeries dcterms:isPartOf)
InverseObjectProperties(dcat:inSeries dcat:seriesMember)

# Object Property: dcat:isDistributionOf (dcat:isDistributionOf)

AnnotationAssertion(rdfs:isDefinedBy dcat:isDistributionOf <https://www.w3.org/TR/vocab-dcat-3/>)
AnnotationAssertion(skos:changeNote dcat:isDistributionOf "New property added in DCAT 3."@en)
AnnotationAssertion(skos:changeNote dcat:isDistributionOf "Nová vlastnost přidaná ve verzi DCAT 3."@cs)
AnnotationAssertion(skos:changeNote dcat:isDistributionOf "Nueva propiedad agregada en DCAT 3."@es)
AnnotationAssertion(skos:changeNote dcat:isDistributionOf "Nuova proprietà aggiunta in DCAT 3."@it)
AnnotationAssertion(skos:scopeNote dcat:isDistributionOf "Esta propiedad inversa PUEDE usarse sólo en combinación con su inversa, y NO PUEDE utilizarse en su reemplazo."@es)
AnnotationAssertion(skos:scopeNote dcat:isDistributionOf "Questa proprietà PUÒ essere usata solo insieme alla sua inversa, e NON DEVE essere usata per sostituirla."@it)
AnnotationAssertion(skos:scopeNote dcat:isDistributionOf "This property MAY be used only in addition to its inverse, and it MUST NOT be used to replace it."@en)

# Object Property: dcat:isVersionOf (dcat:isVersionOf)

AnnotationAssertion(rdfs:isDefinedBy dcat:isVersionOf <https://www.w3.org/TR/vocab-dcat-3/>)
AnnotationAssertion(skos:changeNote dcat:isVersionOf "New property added in DCAT 3."@en)
AnnotationAssertion(skos:changeNote dcat:isVersionOf "Nová vlastnost přidaná ve verzi DCAT 3."@cs)
AnnotationAssertion(skos:changeNote dcat:isVersionOf "Nueva propiedad agregada en DCAT 3."@es)
AnnotationAssertion(skos:changeNote dcat:isVersionOf "Nuova proprietà aggiunta in DCAT 3."@it)
AnnotationAssertion(skos:scopeNote dcat:isVersionOf "Esta propiedad inversa PUEDE usarse sólo en combinación con su inversa, y NO PUEDE utilizarse en su reemplazo."@es)
AnnotationAssertion(skos:scopeNote dcat:isVersionOf "Questa proprietà PUÒ essere usata solo insieme alla sua inversa, e NON DEVE essere usata per sostituirla."@it)
AnnotationAssertion(skos:scopeNote dcat:isVersionOf "This property MAY be used only in addition to its inverse, and it MUST NOT be used to replace it."@en)

# Object Property: dcat:landingPage (page d'atterrissage)

AnnotationAssertion(rdfs:comment dcat:landingPage "A Web page that can be navigated to in a Web browser to gain access to the catalog, a dataset, its distributions and/or additional information."@en)
AnnotationAssertion(rdfs:comment dcat:landingPage "En webside som der kan navigeres til i en webbrowser for at få adgang til kataloget, et datasæt, dets distributioner og/eller yderligere information."@da)
AnnotationAssertion(rdfs:comment dcat:landingPage "Una pagina web che può essere navigata per ottenere l'accesso al catalogo, ad un dataset, alle distribuzioni del dataset e/o ad informazioni addizionali."@it)
AnnotationAssertion(rdfs:comment dcat:landingPage "Una página web que puede ser visitada en un explorador Web para tener acceso el catálogo, un conjunto de datos, sus distribuciones y/o información adicional."@es)
AnnotationAssertion(rdfs:comment dcat:landingPage "Une page Web accessible par un navigateur Web donnant accès au catalogue, un jeu de données, ses distributions et/ou des informations additionnelles."@fr)
AnnotationAssertion(rdfs:comment dcat:landingPage "Webová stránka, na kterou lze pro získání přístupu ke katalogu, datové sadě, jejím distribucím a/nebo dalším informacím přistoupit webovým prohlížečem."@cs)
AnnotationAssertion(rdfs:comment dcat:landingPage "Μία ιστοσελίδα πλοηγίσιμη μέσω ενός φυλλομετρητή (Web browser) που δίνει πρόσβαση στο σύνολο δεδομένων, τις διανομές αυτού ή/και επιπρόσθετες πληροφορίες."@el)
AnnotationAssertion(rdfs:comment dcat:landingPage "صفحة وب يمكن من خلالها الوصول الى قائمة البيانات أو إلى معلومات إضافية متعلقة بها "@ar)
AnnotationAssertion(rdfs:comment dcat:landingPage "データセット、その配信および（または）追加情報にアクセスするためにウエブ・ブラウザでナビゲートできるウェブページ。"@ja)
AnnotationAssertion(rdfs:isDefinedBy dcat:landingPage <http://www.w3.org/TR/vocab-dcat/>)
AnnotationAssertion(rdfs:label dcat:landingPage "destinationsside"@da)
AnnotationAssertion(rdfs:label dcat:landingPage "landing page"@en)
AnnotationAssertion(rdfs:label dcat:landingPage "page d'atterrissage"@fr)
AnnotationAssertion(rdfs:label dcat:landingPage "pagina di destinazione"@it)
AnnotationAssertion(rdfs:label dcat:landingPage "página de destino"@es)
AnnotationAssertion(rdfs:label dcat:landingPage "vstupní stránka"@cs)
AnnotationAssertion(rdfs:label dcat:landingPage "ιστοσελίδα αρχικής πρόσβασης"@el)
AnnotationAssertion(rdfs:label dcat:landingPage "صفحة وصول"@ar)
AnnotationAssertion(rdfs:label dcat:landingPage "ランディング・ページ"@ja)
AnnotationAssertion(skos:definition dcat:landingPage "A Web page that can be navigated to in a Web browser to gain access to the catalog, a dataset, its distributions and/or additional information."@en)
AnnotationAssertion(skos:definition dcat:landingPage "En webside som en webbrowser kan navigeres til for at få adgang til kataloget, et datasæt, dets distritbutioner og/eller yderligere information."@da)
AnnotationAssertion(skos:definition dcat:landingPage "Una pagina web che può essere navigata per ottenere l'accesso al catalogo, ad un dataset, alle distribuzioni del dataset e/o ad informazioni addizionali."@it)
AnnotationAssertion(skos:definition dcat:landingPage "Una página web que puede ser visitada en un explorador Web para tener acceso el catálogo, un conjunto de datos, sus distribuciones y/o información adicional."@es)
AnnotationAssertion(skos:definition dcat:landingPage "Une page Web accessible par un navigateur Web donnant accès au catalogue, un jeu de données, ses distributions et/ou des informations additionnelles."@fr)
AnnotationAssertion(skos:definition dcat:landingPage "Webová stránka, na kterou lze pro získání přístupu ke katalogu, datové sadě, jejím distribucím a/nebo dalším informacím přistoupit webovým prohlížečem."@cs)
AnnotationAssertion(skos:definition dcat:landingPage "Μία ιστοσελίδα πλοηγίσιμη μέσω ενός φυλλομετρητή (Web browser) που δίνει πρόσβαση στο σύνολο δεδομένων, τις διανομές αυτού ή/και επιπρόσθετες πληροφορίες."@el)
AnnotationAssertion(skos:definition dcat:landingPage "صفحة وب يمكن من خلالها الوصول الى قائمة البيانات أو إلى معلومات إضافية متعلقة بها "@ar)
AnnotationAssertion(skos:definition dcat:landingPage "データセット、その配信および（または）追加情報にアクセスするためにウエブ・ブラウザでナビゲートできるウェブページ。"@ja)
AnnotationAssertion(skos:scopeNote dcat:landingPage "Hvis en eller flere distributioner kun er tilgængelige via en destinationsside (dvs. en URL til direkte download er ikke kendt), så bør destinationssidelinket gentages som adgangsadresse for en distribution."@da)
AnnotationAssertion(skos:scopeNote dcat:landingPage "If the distribution(s) are accessible only through a landing page (i.e. direct download URLs are not known), then the landing page link should be duplicated as accessURL on a distribution."@en)
AnnotationAssertion(skos:scopeNote dcat:landingPage "Pokud je distribuce dostupná pouze přes vstupní stránku, t.j. přímý URL odkaz ke stažení není znám, URL přístupové stránky by mělo být duplikováno ve vlastnosti distribuce accessURL."@cs)
AnnotationAssertion(skos:scopeNote dcat:landingPage "Se la distribuzione è accessibile solo attraverso una pagina di destinazione (cioè, un URL di download diretto non è noto), il link alla pagina di destinazione deve essere duplicato come accessURL sulla distribuzione."@it)
AnnotationAssertion(skos:scopeNote dcat:landingPage "Si la distribución es accesible solamente través de una página de aterrizaje (i.e., no se conoce una URL de descarga directa), entonces el enlance a la página de aterrizaje debe ser duplicado como accessURL sobre la distribución."@es)
AnnotationAssertion(skos:scopeNote dcat:landingPage "Si la distribution est seulement accessible à travers une page d'atterrissage (exple. pas de connaissance d'URLS de téléchargement direct ), alors le lien de la page d'atterrissage doit être dupliqué comme accessURL sur la distribution."@fr)
AnnotationAssertion(skos:scopeNote dcat:landingPage "Αν η/οι διανομή/ές είναι προσβάσιμη/ες μόνο μέσω μίας ιστοσελίδας αρχικής πρόσβασης (δηλαδή αν δεν υπάρχουν γνωστές διευθύνσεις άμεσης μεταφόρτωσης), τότε ο σύνδεσμος της ιστοσελίδας αρχικής πρόσβασης πρέπει να αναπαραχθεί ως accessURL σε μία διανομή."@el)
AnnotationAssertion(skos:scopeNote dcat:landingPage "ランディング・ページを通じてしか配信にアクセスできない場合（つまり、直接的なダウンロードURLが不明）には、配信におけるaccessURLとしてランディング・ページのリンクをコピーすべきです（SHOULD）。"@ja)
SubObjectPropertyOf(dcat:landingPage foaf:page)
ObjectPropertyRange(dcat:landingPage foaf:Document)

# Object Property: dcat:last (last)

AnnotationAssertion(rdfs:comment dcat:last "El último recurso en una colección ordenada o serie de recursos, al que el recurso pertenece."@es)
AnnotationAssertion(rdfs:comment dcat:last "L'ultima risorsa in una collezione ordinata o in una serie di risorse, di cui la risorsa fa parte."@it)
AnnotationAssertion(rdfs:comment dcat:last "The last resource in an ordered collection or series of resources, to which the current resource belongs."@en)
AnnotationAssertion(rdfs:isDefinedBy dcat:last <https://www.w3.org/TR/vocab-dcat-3/>)
AnnotationAssertion(rdfs:label dcat:last "last"@en)
AnnotationAssertion(rdfs:label dcat:last "ultimo"@it)
AnnotationAssertion(rdfs:label dcat:last "último"@es)
AnnotationAssertion(skos:changeNote dcat:last "New property added in DCAT 3."@en)
AnnotationAssertion(skos:changeNote dcat:last "Nová vlastnost přidaná ve verzi DCAT 3."@cs)
AnnotationAssertion(skos:changeNote dcat:last "Nueva propiedad agregada in DCAT 3."@es)
AnnotationAssertion(skos:changeNote dcat:last "Nuova proprietà aggiunta in DCAT 3."@it)
AnnotationAssertion(skos:changeNote dcat:last "Ny egenskab tilføjet i DCAT 3."@da)
AnnotationAssertion(skos:definition dcat:last "El último recurso en una colección ordenada o serie de recursos, al que el recurso pertenece."@es)
AnnotationAssertion(skos:definition dcat:last "L'ultima risorsa in una collezione ordinata o in una serie di risorse, di cui la risorsa fa parte."@it)
AnnotationAssertion(skos:definition dcat:last "The last resource in an ordered collection or series of resources, to which the current resource belongs."@en)
AnnotationAssertion(skos:scopeNote dcat:last "En DCAT esta propiedad se usa para recursos que pertenecen a una dcat:DatasetSeries."@es)
AnnotationAssertion(skos:scopeNote dcat:last "In DCAT questa proprietà è usata per risorse che fanno parte di una dcat:DatasetSeries."@it)
AnnotationAssertion(skos:scopeNote dcat:last "In DCAT this property is used for resources belonging to a dcat:DatasetSeries."@en)
SubObjectPropertyOf(dcat:last xhv:last)

# Object Property: dcat:mediaType (typ média)

AnnotationAssertion(rdfs:comment dcat:mediaType "Cette propriété doit être utilisée quand c'est définit le type de média de la distribution en IANA, sinon dcterms:format DOIT être utilisé avec différentes valeurs."@fr)
AnnotationAssertion(rdfs:comment dcat:mediaType "Esta propiedad debe ser usada cuando está definido el tipo de media de la distribución en IANA, de otra manera dcterms:format puede ser utilizado con diferentes valores"@es)
AnnotationAssertion(rdfs:comment dcat:mediaType "Il tipo di media della distribuzione come definito da IANA"@it)
AnnotationAssertion(rdfs:comment dcat:mediaType "Medietypen for distributionen som den er defineret af IANA."@da)
AnnotationAssertion(rdfs:comment dcat:mediaType "The media type of the distribution as defined by IANA"@en)
AnnotationAssertion(rdfs:comment dcat:mediaType "Typ média distribuce definovaný v IANA."@cs)
AnnotationAssertion(rdfs:comment dcat:mediaType "Η ιδιότητα αυτή ΘΑ ΠΡΕΠΕΙ να χρησιμοποιείται όταν ο τύπος μέσου μίας διανομής είναι ορισμένος στο IANA, αλλιώς η ιδιότητα dcterms:format ΔΥΝΑΤΑΙ να χρησιμοποιηθεί με διαφορετικές τιμές."@el)
AnnotationAssertion(rdfs:comment dcat:mediaType "يجب استخدام هذه الخاصية إذا كان نوع الملف معرف ضمن IANA"@ar)
AnnotationAssertion(rdfs:comment dcat:mediaType "このプロパティーは、配信のメディア・タイプがIANAで定義されているときに使用すべきで（SHOULD）、そうでない場合には、dcterms:formatを様々な値と共に使用できます（MAY）。"@ja)
AnnotationAssertion(rdfs:isDefinedBy dcat:mediaType <http://www.w3.org/TR/vocab-dcat/>)
AnnotationAssertion(rdfs:label dcat:mediaType "media type"@en)
AnnotationAssertion(rdfs:label dcat:mediaType "medietype"@da)
AnnotationAssertion(rdfs:label dcat:mediaType "tipo de media"@es)
AnnotationAssertion(rdfs:label dcat:mediaType "tipo di media"@it)
AnnotationAssertion(rdfs:label dcat:mediaType "typ média"@cs)
AnnotationAssertion(rdfs:label dcat:mediaType "type de média"@fr)
AnnotationAssertion(rdfs:label dcat:mediaType "τύπος μέσου"@el)
AnnotationAssertion(rdfs:label dcat:mediaType "نوع الميديا"@ar)
AnnotationAssertion(rdfs:label dcat:mediaType "メディア・タイプ"@ja)
AnnotationAssertion(skos:changeNote dcat:mediaType "Il range di dcat:mediaType è stato ristretto  come parte della revisione di DCAT."@it)
AnnotationAssertion(skos:changeNote dcat:mediaType "Obor hodnot dcat:mediaType byl zúžen v této revizi DCAT."@cs)
AnnotationAssertion(skos:changeNote dcat:mediaType "The range of dcat:mediaType has been tightened as part of the revision of DCAT."@en)
AnnotationAssertion(skos:definition dcat:mediaType "Cette propriété doit être utilisée quand c'est définit le type de média de la distribution en IANA, sinon dcterms:format DOIT être utilisé avec différentes valeurs."@fr)
AnnotationAssertion(skos:definition dcat:mediaType "Esta propiedad debe ser usada cuando está definido el tipo de media de la distribución en IANA, de otra manera dcterms:format puede ser utilizado con diferentes valores."@es)
AnnotationAssertion(skos:definition dcat:mediaType "Il tipo di media della distribuzione come definito da IANA."@it)
AnnotationAssertion(skos:definition dcat:mediaType "Medietypen for distributionen som den er defineret af IANA."@da)
AnnotationAssertion(skos:definition dcat:mediaType "The media type of the distribution as defined by IANA."@en)
AnnotationAssertion(skos:definition dcat:mediaType "Typ média distribuce definovaný v IANA."@cs)
AnnotationAssertion(skos:definition dcat:mediaType "Η ιδιότητα αυτή ΘΑ ΠΡΕΠΕΙ να χρησιμοποιείται όταν ο τύπος μέσου μίας διανομής είναι ορισμένος στο IANA, αλλιώς η ιδιότητα dcterms:format ΔΥΝΑΤΑΙ να χρησιμοποιηθεί με διαφορετικές τιμές."@el)
AnnotationAssertion(skos:definition dcat:mediaType "يجب استخدام هذه الخاصية إذا كان نوع الملف معرف ضمن IANA"@ar)
AnnotationAssertion(skos:definition dcat:mediaType "このプロパティーは、配信のメディア・タイプがIANAで定義されているときに使用すべきで（SHOULD）、そうでない場合には、dcterms:formatを様々な値と共に使用できます（MAY）。"@ja)
AnnotationAssertion(skos:editorialNote dcat:mediaType "Status: English Definition text modified by DCAT revision team, Italian and Czech translation provided, other translations pending. Note some inconsistency on def vs. usage."@en)
AnnotationAssertion(skos:scopeNote dcat:mediaType "Denne egenskab BØR anvendes hvis distributionens medietype optræder i 'IANA media types registry' https://www.iana.org/assignments/media-types/, ellers KAN egenskaben dcterms:format anvendes med et andet udfaldsrum."@da)
AnnotationAssertion(skos:scopeNote dcat:mediaType "Esta propiedad DEBERÍA usarse cuando el 'media type' de la distribución está definido en el registro IANA de 'media types' https://www.iana.org/assignments/media-types/, de lo contrario, dcterms:format PUEDE usarse con distintos valores."@es)
AnnotationAssertion(skos:scopeNote dcat:mediaType "Questa proprietà DEVE essere usata quando il tipo di media della distribuzione è definito nel registro dei tipi di media IANA https://www.iana.org/assignments/media-types/, altrimenti dcterms:format PUO 'essere usato con differenti valori."@it)
AnnotationAssertion(skos:scopeNote dcat:mediaType "Tato vlastnost BY MĚLA být použita, je-li typ média distribuce definován v registru IANA https://www.iana.org/assignments/media-types/. V ostatních případech MŮŽE být použita vlastnost dcterms:format s jinými hodnotami."@cs)
AnnotationAssertion(skos:scopeNote dcat:mediaType "This property SHOULD be used when the media type of the distribution is defined in the IANA media types registry https://www.iana.org/assignments/media-types/, otherwise dcterms:format MAY be used with different values."@en)
SubObjectPropertyOf(dcat:mediaType dcterms:format)
ObjectPropertyDomain(dcat:mediaType dcat:Distribution)
ObjectPropertyRange(dcat:mediaType dcterms:MediaType)

# Object Property: dcat:next (dcat:next)

AnnotationAssertion(rdfs:isDefinedBy dcat:next <https://www.w3.org/TR/vocab-dcat-3/>)
AnnotationAssertion(skos:changeNote dcat:next "New property added in DCAT 3."@en)
AnnotationAssertion(skos:changeNote dcat:next "Nová vlastnost přidaná ve verzi DCAT 3."@cs)
AnnotationAssertion(skos:changeNote dcat:next "Nueva propiedad agregada en DCAT 3."@es)
AnnotationAssertion(skos:changeNote dcat:next "Nuova proprietà aggiunta in DCAT 3."@it)
AnnotationAssertion(skos:scopeNote dcat:next "Esta propiedad inversa PUEDE usarse sólo en combinación con su inversa, y NO PUEDE utilizarse en su reemplazo."@es)
AnnotationAssertion(skos:scopeNote dcat:next "Questa proprietà PUÒ essere usata solo insieme alla sua inversa, e NON DEVE essere usata per sostituirla."@it)
AnnotationAssertion(skos:scopeNote dcat:next "This property MAY be used only in addition to its inverse, and it MUST NOT be used to replace it."@en)
InverseObjectProperties(dcat:next dcat:prev)

# Object Property: dcat:nextVersion (dcat:nextVersion)

AnnotationAssertion(rdfs:isDefinedBy dcat:nextVersion <https://www.w3.org/TR/vocab-dcat-3/>)
AnnotationAssertion(skos:changeNote dcat:nextVersion "New property added in DCAT 3."@en)
AnnotationAssertion(skos:changeNote dcat:nextVersion "Nová vlastnost přidaná ve verzi DCAT 3."@cs)
AnnotationAssertion(skos:changeNote dcat:nextVersion "Nueva propiedad agregada en DCAT 3."@es)
AnnotationAssertion(skos:changeNote dcat:nextVersion "Nuova proprietà aggiunta in DCAT 3."@it)
AnnotationAssertion(skos:scopeNote dcat:nextVersion "Esta propiedad inversa PUEDE usarse sólo en combinación con su inversa, y NO PUEDE utilizarse en su reemplazo."@es)
AnnotationAssertion(skos:scopeNote dcat:nextVersion "Questa proprietà PUÒ essere usata solo insieme alla sua inversa, e NON DEVE essere usata per sostituirla."@it)
AnnotationAssertion(skos:scopeNote dcat:nextVersion "This property MAY be used only in addition to its inverse, and it MUST NOT be used to replace it."@en)
InverseObjectProperties(dcat:nextVersion dcat:previousVersion)

# Object Property: dcat:packageFormat (packaging format)

AnnotationAssertion(rdfs:comment dcat:packageFormat "Balíčkový formát souboru, ve kterém je jeden či více souborů seskupeno dohromady, např. aby bylo možné stáhnout sadu souvisejících souborů naráz."@cs)
AnnotationAssertion(rdfs:comment dcat:packageFormat "El formato del archivo en que se agrupan uno o más archivos de datos, e.g. para permitir que un conjunto de archivos relacionados se bajen juntos."@es)
AnnotationAssertion(rdfs:comment dcat:packageFormat "Format til pakning af data med henblik på distribution af en eller flere relaterede datafiler der samles til en enhed med henblik på samlet distribution. "@da)
AnnotationAssertion(rdfs:comment dcat:packageFormat "Il formato di impacchettamento della distribuzione in cui uno o più file di dati sono raggruppati insieme, ad es. per abilitare un insieme di file correlati da scaricare insieme."@it)
AnnotationAssertion(rdfs:comment dcat:packageFormat "The package format of the distribution in which one or more data files are grouped together, e.g. to enable a set of related files to be downloaded together."@en)
AnnotationAssertion(rdfs:isDefinedBy dcat:packageFormat <https://www.w3.org/TR/vocab-dcat-2/>)
AnnotationAssertion(rdfs:label dcat:packageFormat "formato de empaquetado"@es)
AnnotationAssertion(rdfs:label dcat:packageFormat "formato di impacchettamento"@it)
AnnotationAssertion(rdfs:label dcat:packageFormat "formát balíčku"@cs)
AnnotationAssertion(rdfs:label dcat:packageFormat "packaging format"@en)
AnnotationAssertion(rdfs:label dcat:packageFormat "pakkeformat"@da)
AnnotationAssertion(skos:changeNote dcat:packageFormat "New property added in DCAT 2."@en)
AnnotationAssertion(skos:changeNote dcat:packageFormat "Nová vlastnost přidaná ve verzi DCAT 2."@cs)
AnnotationAssertion(skos:changeNote dcat:packageFormat "Nueva propiedad agregada en DCAT 2."@es)
AnnotationAssertion(skos:changeNote dcat:packageFormat "Nuova proprietà aggiunta in DCAT 2."@it)
AnnotationAssertion(skos:changeNote dcat:packageFormat "Ny egenskab tilføjet i DCAT 2."@da)
AnnotationAssertion(skos:definition dcat:packageFormat "Balíčkový formát souboru, ve kterém je jeden či více souborů seskupeno dohromady, např. aby bylo možné stáhnout sadu souvisejících souborů naráz."@cs)
AnnotationAssertion(skos:definition dcat:packageFormat "El formato del archivo en que se agrupan uno o más archivos de datos, e.g. para permitir que un conjunto de archivos relacionados se bajen juntos."@es)
AnnotationAssertion(skos:definition dcat:packageFormat "Il formato di impacchettamento della distribuzione in cui uno o più file di dati sono raggruppati insieme, ad es. per abilitare un insieme di file correlati da scaricare insieme."@it)
AnnotationAssertion(skos:definition dcat:packageFormat "The package format of the distribution in which one or more data files are grouped together, e.g. to enable a set of related files to be downloaded together."@en)
AnnotationAssertion(skos:scopeNote dcat:packageFormat "Denne egenskab kan anvendes hvis filerne i en distribution er pakket, fx i en TAR-fil, en Frictionless Data Package eller en Bagit-fil. Formatet BØR udtrykkes ved en medietype som defineret i 'IANA media types registry', hvis der optræder en relevant medietype dér: https://www.iana.org/assignments/media-types/."@da)
AnnotationAssertion(skos:scopeNote dcat:packageFormat "Esta propiedad se debe usar cuando los archivos de la distribución están empaquetados, por ejemplo en un archivo TAR, Frictionless Data Package o Bagit. El formato DEBERÍA expresarse usando un 'media type', tales como los definidos en el registro IANA de 'media types' https://www.iana.org/assignments/media-types/, si está disponibles."@es)
AnnotationAssertion(skos:scopeNote dcat:packageFormat "Questa proprietà deve essere utilizzata quando i file nella distribuzione sono impacchettati, ad esempio in un file TAR, Frictionless Data Package o Bagit. Il formato DOVREBBE essere espresso utilizzando un tipo di supporto come definito dal registro dei tipi di media IANA https://www.iana.org/assignments/media-types/, se disponibili."@it)
AnnotationAssertion(skos:scopeNote dcat:packageFormat "Tato vlastnost se použije, když jsou soubory v distribuci zabaleny, např. v souboru TAR, v balíčku Frictionless Data Package nebo v souboru Bagit. Formát BY MĚL být vyjádřen pomocí typu média definovaného v registru IANA https://www.iana.org/assignments/media-types/, pokud existuje."@cs)
AnnotationAssertion(skos:scopeNote dcat:packageFormat "This property to be used when the files in the distribution are packaged, e.g. in a TAR file, a Frictionless Data Package or a Bagit file. The format SHOULD be expressed using a media type as defined by IANA media types registry https://www.iana.org/assignments/media-types/, if available."@en)
SubObjectPropertyOf(dcat:packageFormat dcterms:format)
ObjectPropertyDomain(dcat:packageFormat dcat:Distribution)
ObjectPropertyRange(dcat:packageFormat dcterms:MediaType)

# Object Property: dcat:prev (previous)

AnnotationAssertion(rdfs:comment dcat:prev "La risorsa precedente a quella attuale in una collezione ordinata o in una serie di risorse."@it)
AnnotationAssertion(rdfs:comment dcat:prev "The previous resource (before the current one) in an ordered collection or series of resources."@en)
AnnotationAssertion(rdfs:isDefinedBy dcat:prev <https://www.w3.org/TR/vocab-dcat-3/>)
AnnotationAssertion(rdfs:label dcat:prev "precedente"@it)
AnnotationAssertion(rdfs:label dcat:prev "previo"@es)
AnnotationAssertion(rdfs:label dcat:prev "previous"@en)
AnnotationAssertion(skos:changeNote dcat:prev "New property added in DCAT 3."@en)
AnnotationAssertion(skos:changeNote dcat:prev "Nová vlastnost přidaná ve verzi DCAT 3."@cs)
AnnotationAssertion(skos:changeNote dcat:prev "Nueva propiedad agregada in DCAT 3."@es)
AnnotationAssertion(skos:changeNote dcat:prev "Nuova proprietà aggiunta in DCAT 3."@it)
AnnotationAssertion(skos:changeNote dcat:prev "Ny egenskab tilføjet i DCAT 3."@da)
AnnotationAssertion(skos:definition dcat:prev "La risorsa precedente a quella attuale in una collezione ordinata o in una serie di risorse."@it)
AnnotationAssertion(skos:definition dcat:prev "The previous resource (before the current one) in an ordered collection or series of resources."@en)
AnnotationAssertion(skos:scopeNote dcat:prev "En DCAT esta propiedad se usa para recursos que pertenecen a una dcat:DatasetSeries."@es)
AnnotationAssertion(skos:scopeNote dcat:prev "In DCAT questa proprietà è usata per risorse che fanno parte di una dcat:DatasetSeries."@it)
AnnotationAssertion(skos:scopeNote dcat:prev "In DCAT this property is used for resources belonging to a dcat:DatasetSeries."@en)
AnnotationAssertion(skos:scopeNote dcat:prev "It is important to note that this property is different from dcat:previousVersion, as it does not denote a previous version of the same resource, but a distinct resource immediately preceding the current one in an ordered collection of resources."@en)
AnnotationAssertion(skos:scopeNote dcat:prev "È importante notare che questa proprietà è diversa da dcat:previousVersion, dato che non indica una versione precedente della stessa risorsa, ma una risorsa distinta che precede immediatamente quella attuale in una collezione ordinata di risorse."@it)
SubObjectPropertyOf(dcat:prev xhv:prev)

# Object Property: dcat:previousVersion (previous version)

AnnotationAssertion(rdfs:comment dcat:previousVersion "La versione precedente di una risorsa."@it)
AnnotationAssertion(rdfs:comment dcat:previousVersion "The previous version of a resource in a lineage [PAV]."@en)
AnnotationAssertion(rdfs:isDefinedBy dcat:previousVersion <https://www.w3.org/TR/vocab-dcat-3/>)
AnnotationAssertion(rdfs:label dcat:previousVersion "previous version"@en)
AnnotationAssertion(rdfs:label dcat:previousVersion "versione precedente"@it)
AnnotationAssertion(rdfs:label dcat:previousVersion "versión anterior"@es)
AnnotationAssertion(skos:changeNote dcat:previousVersion "New property added in DCAT 3."@en)
AnnotationAssertion(skos:changeNote dcat:previousVersion "Nová vlastnost přidaná ve verzi DCAT 3."@cs)
AnnotationAssertion(skos:changeNote dcat:previousVersion "Nueva propiedad agregada in DCAT 3."@es)
AnnotationAssertion(skos:changeNote dcat:previousVersion "Nuova proprietà aggiunta in DCAT 3."@it)
AnnotationAssertion(skos:changeNote dcat:previousVersion "Ny egenskab tilføjet i DCAT 3."@da)
AnnotationAssertion(skos:definition dcat:previousVersion "La versione precedente di una risorsa."@it)
AnnotationAssertion(skos:definition dcat:previousVersion "The previous version of a resource in a lineage [PAV]."@en)
AnnotationAssertion(skos:scopeNote dcat:previousVersion "La nozione di versione usata da questa proprietà è limitata a versioni risultanti da revisioni a cui una risorsa è soggetta nel suo ciclo di vita. Uno dei casi tipici è la rappresentazione della storia delle versioni di un dataset, che sono state pubblicate nel corso del tempo."@it)
AnnotationAssertion(skos:scopeNote dcat:previousVersion "Questa proprietà è usata per specificare una catena di versioni, costituita da snapshot di una risorsa."@it)
AnnotationAssertion(skos:scopeNote dcat:previousVersion "The notion of version used by this property is limited to versions resulting from revisions occurring to a resource as part of its life-cycle. One of the typical cases here is representing the history of the versions of a dataset that have been released over time."@en)
AnnotationAssertion(skos:scopeNote dcat:previousVersion "This property is meant to be used to specify a version chain, consisting of snapshots of a resource."@en)
SubObjectPropertyOf(dcat:previousVersion prov:wasRevisionOf)

# Object Property: dcat:qualifiedRelation (Kvalificeret relation)

AnnotationAssertion(rdfs:comment dcat:qualifiedRelation "Enlace a una descripción de la relación con otro recurso."@es)
AnnotationAssertion(rdfs:comment dcat:qualifiedRelation "Link a una descrizione di una relazione con un'altra risorsa."@it)
AnnotationAssertion(rdfs:comment dcat:qualifiedRelation "Link to a description of a relationship with another resource."@en)
AnnotationAssertion(rdfs:comment dcat:qualifiedRelation "Odkaz na popis vztahu s jiným zdrojem."@cs)
AnnotationAssertion(rdfs:comment dcat:qualifiedRelation "Reference til en beskrivelse af en relation til en anden ressource."@da)
AnnotationAssertion(rdfs:isDefinedBy dcat:qualifiedRelation <https://www.w3.org/TR/vocab-dcat-2/>)
AnnotationAssertion(rdfs:label dcat:qualifiedRelation "Kvalificeret relation"@da)
AnnotationAssertion(rdfs:label dcat:qualifiedRelation "kvalifikovaný vztah"@cs)
AnnotationAssertion(rdfs:label dcat:qualifiedRelation "qualified relation"@en)
AnnotationAssertion(rdfs:label dcat:qualifiedRelation "relación calificada"@es)
AnnotationAssertion(rdfs:label dcat:qualifiedRelation "relazione qualificata"@it)
AnnotationAssertion(skos:changeNote dcat:qualifiedRelation "New property added in DCAT 2."@en)
AnnotationAssertion(skos:changeNote dcat:qualifiedRelation "Nová vlastnost přidaná ve verzi DCAT 2."@cs)
AnnotationAssertion(skos:changeNote dcat:qualifiedRelation "Nuova proprietà aggiunta in DCAT 2."@it)
AnnotationAssertion(skos:changeNote dcat:qualifiedRelation "Ny egenskab tilføjet i DCAT 2."@da)
AnnotationAssertion(skos:changeNote dcat:qualifiedRelation "Propiedad nueva añadida en DCAT 2."@es)
AnnotationAssertion(skos:definition dcat:qualifiedRelation "Enlace a una descripción de la relación con otro recurso."@es)
AnnotationAssertion(skos:definition dcat:qualifiedRelation "Link a una descrizione di una relazione con un'altra risorsa."@it)
AnnotationAssertion(skos:definition dcat:qualifiedRelation "Link to a description of a relationship with another resource."@en)
AnnotationAssertion(skos:definition dcat:qualifiedRelation "Odkaz na popis vztahu s jiným zdrojem."@cs)
AnnotationAssertion(skos:definition dcat:qualifiedRelation "Reference til en beskrivelse af en relation til en anden ressource."@da)
AnnotationAssertion(skos:editorialNote dcat:qualifiedRelation "Introdotta in DCAT per integrare le altre relazioni qualificate di PROV."@it)
AnnotationAssertion(skos:editorialNote dcat:qualifiedRelation "Introduced into DCAT to complement the other PROV qualified relations. "@en)
AnnotationAssertion(skos:editorialNote dcat:qualifiedRelation "Introduceret i DCAT med henblik på at supplere de øvrige kvalificerede relationer fra PROV. "@da)
AnnotationAssertion(skos:editorialNote dcat:qualifiedRelation "Přidáno do DCAT k doplnění jiných kvalifikovaných vztahů ze slovníku PROV."@cs)
AnnotationAssertion(skos:editorialNote dcat:qualifiedRelation "Se incluyó en DCAT para complementar las relaciones calificadas disponibles en PROV."@es)
AnnotationAssertion(skos:scopeNote dcat:qualifiedRelation "Anvendes til at referere til en anden ressource hvor relationens betydning er kendt men ikke matcher en af de standardiserede egenskaber fra Dublin Core (dcterms:hasPart, dcterms:isPartOf, dcterms:conformsTo, dcterms:isFormatOf, dcterms:hasFormat, dcterms:isVersionOf, dcterms:hasVersion, dcterms:replaces, dcterms:isReplacedBy, dcterms:references, dcterms:isReferencedBy, dcterms:requires, dcterms:isRequiredBy) eller PROV-O-egenskaber (prov:wasDerivedFrom, prov:wasInfluencedBy, prov:wasQuotedFrom, prov:wasRevisionOf, prov:hadPrimarySource, prov:alternateOf, prov:specializationOf)."@da)
AnnotationAssertion(skos:scopeNote dcat:qualifiedRelation "Použito pro odkazování na jiný zdroj, kde druh vztahu je znám, ale neodpovídá standardním vlastnostem ze slovníku Dublin Core (dcterms:hasPart, dcterms:isPartOf, dcterms:conformsTo, dcterms:isFormatOf, dcterms:hasFormat, dcterms:isVersionOf, dcterms:hasVersion, dcterms:replaces, dcterms:isReplacedBy, dcterms:references, dcterms:isReferencedBy, dcterms:requires, dcterms:isRequiredBy) či slovníku PROV-O (prov:wasDerivedFrom, prov:wasInfluencedBy, prov:wasQuotedFrom, prov:wasRevisionOf, prov:hadPrimarySource, prov:alternateOf, prov:specializationOf)."@cs)
AnnotationAssertion(skos:scopeNote dcat:qualifiedRelation "Se usa para asociar con otro recurso para el cuál la naturaleza de la relación es conocida pero no es ninguna de las propiedades que provee el estándar Dublin Core (dcterms:hasPart, dcterms:isPartOf, dcterms:conformsTo, dcterms:isFormatOf, dcterms:hasFormat, dcterms:isVersionOf, dcterms:hasVersion, dcterms:replaces, dcterms:isReplacedBy, dcterms:references, dcterms:isReferencedBy, dcterms:requires, dcterms:isRequiredBy) or PROV-O properties (prov:wasDerivedFrom, prov:wasInfluencedBy, prov:wasQuotedFrom, prov:wasRevisionOf, prov:hadPrimarySource, prov:alternateOf, prov:specializationOf)."@es)
AnnotationAssertion(skos:scopeNote dcat:qualifiedRelation "Used to link to another resource where the nature of the relationship is known but does not match one of the standard Dublin Core properties (dcterms:hasPart, dcterms:isPartOf, dcterms:conformsTo, dcterms:isFormatOf, dcterms:hasFormat, dcterms:isVersionOf, dcterms:hasVersion, dcterms:replaces, dcterms:isReplacedBy, dcterms:references, dcterms:isReferencedBy, dcterms:requires, dcterms:isRequiredBy) or PROV-O properties (prov:wasDerivedFrom, prov:wasInfluencedBy, prov:wasQuotedFrom, prov:wasRevisionOf, prov:hadPrimarySource, prov:alternateOf, prov:specializationOf)."@en)
AnnotationAssertion(skos:scopeNote dcat:qualifiedRelation "Viene utilizzato per associarsi a un'altra risorsa nei casi per i quali la natura della relazione è nota ma non è alcuna delle proprietà fornite dallo standard Dublin Core (dcterms:hasPart, dcterms:isPartOf, dcterms:conformsTo, dcterms:isFormatOf, dcterms:hasFormat , dcterms:isVersionOf, dcterms:hasVersion, dcterms:replaces, dcterms:isReplacedBy, dcterms:references, dcterms:isReferencedBy, dcterms:require, dcterms:isRequiredBy) o dalle proprietà fornite da PROV-O (prov:wasDerivedFrom, prov:wasInfluencedBy, prov:wasQuotedFrom , prov:wasRevisionOf, prov:hadPrimarySource, prov:alternateOf, prov:specializationOf)."@it)
ObjectPropertyDomain(dcat:qualifiedRelation dcat:Resource)
ObjectPropertyRange(dcat:qualifiedRelation dcat:Relationship)

# Object Property: dcat:record (záznam)

AnnotationAssertion(rdfs:comment dcat:record "A record describing the registration of a single dataset or data service that is part of the catalog."@en)
AnnotationAssertion(rdfs:comment dcat:record "Describe la registración de un conjunto de datos o un servicio de datos en el catálogo."@es)
AnnotationAssertion(rdfs:comment dcat:record "En post der beskriver registreringen af et enkelt datasæt eller en datatjeneste som er opført i kataloget."@da)
AnnotationAssertion(rdfs:comment dcat:record "Propojuje katalog a jeho záznamy."@cs)
AnnotationAssertion(rdfs:comment dcat:record "Relie un catalogue à ses registres."@fr)
AnnotationAssertion(rdfs:comment dcat:record "Un record che descrive la registrazione di un singolo set di dati o di un servizio dati che fa parte del catalogo."@it)
AnnotationAssertion(rdfs:comment dcat:record "Záznam popisující registraci jedné datové sady či datové služby jakožto součásti katalogu."@cs)
AnnotationAssertion(rdfs:comment dcat:record "Συνδέει έναν κατάλογο με τις καταγραφές του."@el)
AnnotationAssertion(rdfs:comment dcat:record "تربط الفهرس بسجل ضمنه"@ar)
AnnotationAssertion(rdfs:comment dcat:record "カタログの一部であるカタログ・レコード。"@ja)
AnnotationAssertion(rdfs:isDefinedBy dcat:record <http://www.w3.org/TR/vocab-dcat/>)
AnnotationAssertion(rdfs:label dcat:record "post"@da)
AnnotationAssertion(rdfs:label dcat:record "record"@en)
AnnotationAssertion(rdfs:label dcat:record "record"@it)
AnnotationAssertion(rdfs:label dcat:record "registre"@fr)
AnnotationAssertion(rdfs:label dcat:record "registro"@es)
AnnotationAssertion(rdfs:label dcat:record "záznam"@cs)
AnnotationAssertion(rdfs:label dcat:record "καταγραφή"@el)
AnnotationAssertion(rdfs:label dcat:record "سجل"@ar)
AnnotationAssertion(rdfs:label dcat:record "カタログ・レコード"@ja)
AnnotationAssertion(skos:altLabel dcat:record "har post"@da)
AnnotationAssertion(skos:definition dcat:record "A record describing the registration of a single dataset or data service that is part of the catalog."@en)
AnnotationAssertion(skos:definition dcat:record "Describe la registración de un conjunto de datos o un servicio de datos en el catálogo."@es)
AnnotationAssertion(skos:definition dcat:record "En post der beskriver registreringen af et enkelt datasæt eller en datatjeneste som er opført i kataloget."@da)
AnnotationAssertion(skos:definition dcat:record "Propojuje katalog a jeho záznamy."@cs)
AnnotationAssertion(skos:definition dcat:record "Relie un catalogue à ses registres."@fr)
AnnotationAssertion(skos:definition dcat:record "Un record che descrive la registrazione di un singolo set di dati o di un servizio dati che fa parte del catalogo."@it)
AnnotationAssertion(skos:definition dcat:record "Záznam popisující registraci jedné datové sady či datové služby jakožto součásti katalogu."@cs)
AnnotationAssertion(skos:definition dcat:record "Συνδέει έναν κατάλογο με τις καταγραφές του."@el)
AnnotationAssertion(skos:definition dcat:record "تربط الفهرس بسجل ضمنه"@ar)
AnnotationAssertion(skos:definition dcat:record "カタログの一部であるカタログ・レコード。"@ja)
AnnotationAssertion(skos:editorialNote dcat:record "Status: English, Italian, Spanish and Czech Definitions modified by DCAT revision team, other translations pending."@en)
ObjectPropertyDomain(dcat:record dcat:Catalog)
ObjectPropertyRange(dcat:record dcat:CatalogRecord)

# Object Property: dcat:resource (resource)

AnnotationAssertion(rdfs:comment dcat:resource "A resource that is listed in the catalog."@en)
AnnotationAssertion(rdfs:comment dcat:resource "Una risorsa elencata nel catalogo."@it)
AnnotationAssertion(rdfs:isDefinedBy dcat:resource <https://www.w3.org/TR/vocab-dcat-3/>)
AnnotationAssertion(rdfs:label dcat:resource "resource"@en)
AnnotationAssertion(rdfs:label dcat:resource "risorsa"@it)
AnnotationAssertion(skos:changeNote dcat:resource "New property added in DCAT 3."@en)
AnnotationAssertion(skos:changeNote dcat:resource "Nová vlastnost přidaná ve verzi DCAT 3."@cs)
AnnotationAssertion(skos:changeNote dcat:resource "Nueva propiedad agregada en DCAT 3."@es)
AnnotationAssertion(skos:changeNote dcat:resource "Nuova proprietà aggiunta in DCAT 3."@it)
AnnotationAssertion(skos:definition dcat:resource "A resource that is listed in the catalog."@en)
AnnotationAssertion(skos:definition dcat:resource "Una risorsa elencata nel catalogo."@it)
AnnotationAssertion(skos:editorialNote dcat:resource "Status: English Definition text modified by DCAT 3 revision team, translations pending."@en)
AnnotationAssertion(skos:scopeNote dcat:resource "Questo è il predicate più generale per indicare l'appartenenza di una risorsa a un catalogo. Si raccomanda l'uso di una proprietà più specifica, quando disponibile."@it)
AnnotationAssertion(skos:scopeNote dcat:resource "See also:	Sub-properties of dcat:resource in particular dcat:dataset, dcat:catalog, dcat:service."@en)
AnnotationAssertion(skos:scopeNote dcat:resource "This is the most general predicate for membership of a catalog. Use of a more specific sub-property is recommended when available."@en)
AnnotationAssertion(skos:scopeNote dcat:resource "Vd. anche: Le sottoproprietà di dcat:resource, in particolare: dcat:dataset, dcat:catalog, dcat:service."@it)
SubObjectPropertyOf(dcat:resource dcterms:hasPart)
ObjectPropertyDomain(dcat:resource dcat:Catalog)
ObjectPropertyRange(dcat:resource dcat:Resource)

# Object Property: dcat:seriesMember (dcat:seriesMember)

AnnotationAssertion(rdfs:isDefinedBy dcat:seriesMember <https://www.w3.org/TR/vocab-dcat-3/>)
AnnotationAssertion(skos:changeNote dcat:seriesMember "New property added in DCAT 3."@en)
AnnotationAssertion(skos:changeNote dcat:seriesMember "Nová vlastnost přidaná ve verzi DCAT 3."@cs)
AnnotationAssertion(skos:changeNote dcat:seriesMember "Nueva propiedad agregada en DCAT 3."@es)
AnnotationAssertion(skos:changeNote dcat:seriesMember "Nuova proprietà aggiunta in DCAT 3."@it)
AnnotationAssertion(skos:scopeNote dcat:seriesMember "Esta propiedad inversa PUEDE usarse sólo en combinación con su inversa, y NO PUEDE utilizarse en su reemplazo."@es)
AnnotationAssertion(skos:scopeNote dcat:seriesMember "Questa proprietà PUÒ essere usata solo insieme alla sua inversa, e NON DEVE essere usata per sostituirla."@it)
AnnotationAssertion(skos:scopeNote dcat:seriesMember "This property MAY be used only in addition to its inverse, and it MUST NOT be used to replace it."@en)

# Object Property: dcat:servesDataset (provee conjunto de datos)

AnnotationAssertion(rdfs:comment dcat:servesDataset "A collection of data that this DataService can distribute."@en)
AnnotationAssertion(rdfs:comment dcat:servesDataset "En samling af data som denne datatjeneste kan distribuere."@da)
AnnotationAssertion(rdfs:comment dcat:servesDataset "Kolekce dat, kterou je tato Datová služba schopna poskytnout."@cs)
AnnotationAssertion(rdfs:comment dcat:servesDataset "Una colección de datos que este Servicio de Datos puede distribuir."@es)
AnnotationAssertion(rdfs:comment dcat:servesDataset "Una raccolta di dati che questo DataService può distribuire."@it)
AnnotationAssertion(rdfs:isDefinedBy dcat:servesDataset <https://www.w3.org/TR/vocab-dcat-2/>)
AnnotationAssertion(rdfs:label dcat:servesDataset "datatjeneste for datasæt"@da)
AnnotationAssertion(rdfs:label dcat:servesDataset "poskytuje datovou sadu"@cs)
AnnotationAssertion(rdfs:label dcat:servesDataset "provee conjunto de datos"@es)
AnnotationAssertion(rdfs:label dcat:servesDataset "serve set di dati"@it)
AnnotationAssertion(rdfs:label dcat:servesDataset "serves dataset"@en)
AnnotationAssertion(skos:altLabel dcat:servesDataset "distribuerer"@da)
AnnotationAssertion(skos:altLabel dcat:servesDataset "ekspederer"@da)
AnnotationAssertion(skos:altLabel dcat:servesDataset "udstiller"@da)
AnnotationAssertion(skos:changeNote dcat:servesDataset "New property in DCAT 2."@en)
AnnotationAssertion(skos:changeNote dcat:servesDataset "Nová vlastnost přidaná ve verzi DCAT 2."@cs)
AnnotationAssertion(skos:changeNote dcat:servesDataset "Nueva propiedad agregada en DCAT 2."@es)
AnnotationAssertion(skos:changeNote dcat:servesDataset "Nuova proprietà in DCAT 2."@it)
AnnotationAssertion(skos:definition dcat:servesDataset "A collection of data that this DataService can distribute."@en)
AnnotationAssertion(skos:definition dcat:servesDataset "En samling af data som denne datatjeneste kan distribuere."@da)
AnnotationAssertion(skos:definition dcat:servesDataset "Kolekce dat, kterou je tato Datová služba schopna poskytnout."@cs)
AnnotationAssertion(skos:definition dcat:servesDataset "Una colección de datos que este Servicio de Datos puede distribuir."@es)
AnnotationAssertion(skos:definition dcat:servesDataset "Una raccolta di dati che questo DataService può distribuire."@it)
ObjectPropertyDomain(dcat:servesDataset dcat:DataService)
ObjectPropertyRange(dcat:servesDataset dcat:Dataset)

# Object Property: dcat:service (datatjeneste)

AnnotationAssertion(rdfs:comment dcat:service "A service that is listed in the catalog."@en)
AnnotationAssertion(rdfs:comment dcat:service "Et websted eller et endpoint som er opført i kataloget."@da)
AnnotationAssertion(rdfs:comment dcat:service "Umístění či přístupový bod registrovaný v katalogu."@cs)
AnnotationAssertion(rdfs:comment dcat:service "Un sitio o 'endpoint' que está listado en el catálogo."@es)
AnnotationAssertion(rdfs:comment dcat:service "Un sito o endpoint elencato nel catalogo."@it)
AnnotationAssertion(rdfs:isDefinedBy dcat:service <https://www.w3.org/TR/vocab-dcat-2/>)
AnnotationAssertion(rdfs:label dcat:service "datatjeneste"@da)
AnnotationAssertion(rdfs:label dcat:service "service"@en)
AnnotationAssertion(rdfs:label dcat:service "servicio"@es)
AnnotationAssertion(rdfs:label dcat:service "servizio"@it)
AnnotationAssertion(rdfs:label dcat:service "služba"@cs)
AnnotationAssertion(skos:altLabel dcat:service "har datatjeneste"@da)
AnnotationAssertion(skos:altLabel dcat:service "has service"@en)
AnnotationAssertion(skos:changeNote dcat:service "New property added in DCAT 2."@en)
AnnotationAssertion(skos:changeNote dcat:service "Nová vlastnost přidaná ve verzi DCAT 2."@cs)
AnnotationAssertion(skos:changeNote dcat:service "Nueva propiedad añadida en DCAT 2."@es)
AnnotationAssertion(skos:changeNote dcat:service "Nuova proprietà aggiunta in DCAT 2."@it)
AnnotationAssertion(skos:definition dcat:service "A service that is listed in the catalog."@en)
AnnotationAssertion(skos:definition dcat:service "Et websted eller et endpoint som er opført i kataloget."@da)
AnnotationAssertion(skos:definition dcat:service "Umístění či přístupový bod registrovaný v katalogu."@cs)
AnnotationAssertion(skos:definition dcat:service "Un sitio o 'endpoint' que está listado en el catálogo."@es)
AnnotationAssertion(skos:definition dcat:service "Un sito o endpoint elencato nel catalogo."@it)
AnnotationAssertion(skos:editorialNote dcat:service "Status: English Definition text modified by DCAT 3 revision team, translations pending."@en)
SubObjectPropertyOf(dcat:service dcat:resource)
ObjectPropertyDomain(dcat:service dcat:Catalog)
ObjectPropertyRange(dcat:service dcat:DataService)

# Object Property: dcat:theme (tema)

AnnotationAssertion(rdfs:comment dcat:theme "A main category of the resource. A resource can have multiple themes."@en)
AnnotationAssertion(rdfs:comment dcat:theme "Et centralt emne for ressourcen. En ressource kan have flere centrale emner."@da)
AnnotationAssertion(rdfs:comment dcat:theme "Hlavní téma zdroje. Zdroj může mít více témat."@cs)
AnnotationAssertion(rdfs:comment dcat:theme "La categoria principale della risorsa. Una risorsa può avere più temi."@it)
AnnotationAssertion(rdfs:comment dcat:theme "La categoría principal del recurso. Un recurso puede tener varios temas."@es)
AnnotationAssertion(rdfs:comment dcat:theme "La catégorie principale de la ressource. Une ressource peut avoir plusieurs thèmes."@fr)
AnnotationAssertion(rdfs:comment dcat:theme "Η κύρια κατηγορία του συνόλου δεδομένων. Ένα σύνολο δεδομένων δύναται να έχει πολλαπλά θέματα."@el)
AnnotationAssertion(rdfs:comment dcat:theme "التصنيف الرئيسي لقائمة البيانات. قائمة البيانات يمكن أن تملك أكثر من تصنيف رئيسي واحد."@ar)
AnnotationAssertion(rdfs:comment dcat:theme "データセットの主要カテゴリー。データセットは複数のテーマを持つことができます。"@ja)
AnnotationAssertion(rdfs:isDefinedBy dcat:theme <http://www.w3.org/TR/vocab-dcat/>)
AnnotationAssertion(rdfs:label dcat:theme "emne"@da)
AnnotationAssertion(rdfs:label dcat:theme "tema"@es)
AnnotationAssertion(rdfs:label dcat:theme "tema"@it)
AnnotationAssertion(rdfs:label dcat:theme "theme"@en)
AnnotationAssertion(rdfs:label dcat:theme "thème"@fr)
AnnotationAssertion(rdfs:label dcat:theme "téma"@cs)
AnnotationAssertion(rdfs:label dcat:theme "Θέμα"@el)
AnnotationAssertion(rdfs:label dcat:theme "التصنيف"@ar)
AnnotationAssertion(rdfs:label dcat:theme "テーマ/カテゴリー"@ja)
AnnotationAssertion(skos:altLabel dcat:theme "tema"@da)
AnnotationAssertion(skos:definition dcat:theme "A main category of the resource. A resource can have multiple themes."@en)
AnnotationAssertion(skos:definition dcat:theme "Et centralt emne for ressourcen. En ressource kan have flere centrale emner."@da)
AnnotationAssertion(skos:definition dcat:theme "Hlavní téma zdroje. Zdroj může mít více témat."@cs)
AnnotationAssertion(skos:definition dcat:theme "La categoria principale della risorsa. Una risorsa può avere più temi."@it)
AnnotationAssertion(skos:definition dcat:theme "La categoría principal del recurso. Un recurso puede tener varios temas."@es)
AnnotationAssertion(skos:definition dcat:theme "La catégorie principale de la ressource. Une ressource peut avoir plusieurs thèmes."@fr)
AnnotationAssertion(skos:definition dcat:theme "Η κύρια κατηγορία του συνόλου δεδομένων. Ένα σύνολο δεδομένων δύναται να έχει πολλαπλά θέματα."@el)
AnnotationAssertion(skos:definition dcat:theme "التصنيف الرئيسي لقائمة البيانات. قائمة البيانات يمكن أن تملك أكثر من تصنيف رئيسي واحد."@ar)
AnnotationAssertion(skos:definition dcat:theme "データセットの主要カテゴリー。データセットは複数のテーマを持つことができます。"@ja)
AnnotationAssertion(skos:editorialNote dcat:theme "Status: English Definition text  modified by DCAT revision team, all except for Italian and Czech translations are pending. Scope note has changed and its translations should be updated"@en)
AnnotationAssertion(skos:scopeNote dcat:theme "El conjunto de skos:Concepts utilizados para categorizar los recursos están organizados en un skos:ConceptScheme que describe todas las categorías y sus relaciones en el catálogo."@es)
AnnotationAssertion(skos:scopeNote dcat:theme "Il set di concetti skos usati per categorizzare le risorse sono organizzati in skos:ConceptScheme che descrive tutte le categorie e le loro relazioni nel catalogo."@it)
AnnotationAssertion(skos:scopeNote dcat:theme "Sada instancí třídy skos:Concept použitá pro kategorizaci zdrojů je organizována do schématu konceptů skos:ConceptScheme, které popisuje všechny kategorie v katalogu a jejich vztahy."@cs)
AnnotationAssertion(skos:scopeNote dcat:theme "Samlingen af begreber (skos:Concept) der anvendes til at emneinddele ressourcer organiseres i et begrebssystem (skos:ConceptScheme) som beskriver alle emnerne og deres relationer i kataloget."@da)
AnnotationAssertion(skos:scopeNote dcat:theme "The set of themes used to categorize the resources are organized in a skos:ConceptScheme, skos:Collection, owl:Ontology or similar, describing all the categories and their relations in the catalog."@en)
AnnotationAssertion(skos:scopeNote dcat:theme "Un ensemble de skos:Concepts utilisés pour catégoriser les ressources sont organisés en un skos:ConceptScheme décrivant toutes les catégories et ses relations dans le catalogue."@fr)
AnnotationAssertion(skos:scopeNote dcat:theme "Το σετ των skos:Concepts που χρησιμοποιείται για να κατηγοριοποιήσει τα σύνολα δεδομένων είναι οργανωμένο εντός ενός skos:ConceptScheme που περιγράφει όλες τις κατηγορίες και τις σχέσεις αυτών στον κατάλογο."@el)
AnnotationAssertion(skos:scopeNote dcat:theme "データセットを分類するために用いられるskos:Conceptの集合は、カタログのすべてのカテゴリーとそれらの関係を記述しているskos:ConceptSchemeで組織化されます。"@ja)
SubObjectPropertyOf(dcat:theme dcterms:subject)

# Object Property: dcat:themeTaxonomy (قائمة التصنيفات)

AnnotationAssertion(sdo:rangeIncludes dcat:themeTaxonomy owl:Ontology)
AnnotationAssertion(sdo:rangeIncludes dcat:themeTaxonomy skos:Collection)
AnnotationAssertion(sdo:rangeIncludes dcat:themeTaxonomy skos:ConceptScheme)
AnnotationAssertion(rdfs:comment dcat:themeTaxonomy "El sistema de organización del conocimiento utilizado para clasificar conjuntos de datos de catálogos."@es)
AnnotationAssertion(rdfs:comment dcat:themeTaxonomy "Il sistema di organizzazione della conoscenza (KOS) usato per classificare i dataset del catalogo."@it)
AnnotationAssertion(rdfs:comment dcat:themeTaxonomy "Le systhème d'ogranisation de connaissances utilisé pour classifier les jeux de données du catalogue."@fr)
AnnotationAssertion(rdfs:comment dcat:themeTaxonomy "Systém organizace znalostí (KOS) použitý pro klasifikaci datových sad v katalogu."@cs)
AnnotationAssertion(rdfs:comment dcat:themeTaxonomy "The knowledge organization system (KOS) used to classify catalog's datasets."@en)
AnnotationAssertion(rdfs:comment dcat:themeTaxonomy "Vidensorganiseringssystem (KOS) som anvendes til at klassificere datasæt i kataloget."@da)
AnnotationAssertion(rdfs:comment dcat:themeTaxonomy "Το σύστημα οργάνωσης γνώσης που χρησιμοποιείται για την κατηγοριοποίηση των συνόλων δεδομένων του καταλόγου."@el)
AnnotationAssertion(rdfs:comment dcat:themeTaxonomy "لائحة التصنيفات المستخدمه لتصنيف قوائم البيانات ضمن الفهرس"@ar)
AnnotationAssertion(rdfs:comment dcat:themeTaxonomy "カタログのデータセットを分類するために用いられる知識組織化体系（KOS；knowledge organization system）。"@ja)
AnnotationAssertion(rdfs:isDefinedBy dcat:themeTaxonomy <http://www.w3.org/TR/vocab-dcat/>)
AnnotationAssertion(rdfs:label dcat:themeTaxonomy "emnetaksonomi"@da)
AnnotationAssertion(rdfs:label dcat:themeTaxonomy "tassonomia dei temi"@it)
AnnotationAssertion(rdfs:label dcat:themeTaxonomy "taxonomie de thèmes"@fr)
AnnotationAssertion(rdfs:label dcat:themeTaxonomy "taxonomie témat"@cs)
AnnotationAssertion(rdfs:label dcat:themeTaxonomy "taxonomía de temas"@es)
AnnotationAssertion(rdfs:label dcat:themeTaxonomy "theme taxonomy"@en)
AnnotationAssertion(rdfs:label dcat:themeTaxonomy "Ταξινομία θεματικών κατηγοριών."@el)
AnnotationAssertion(rdfs:label dcat:themeTaxonomy "قائمة التصنيفات"@ar)
AnnotationAssertion(rdfs:label dcat:themeTaxonomy "テーマ"@ja)
AnnotationAssertion(skos:altLabel dcat:themeTaxonomy "temataksonomi"@da)
AnnotationAssertion(skos:definition dcat:themeTaxonomy "El sistema de organización del conocimiento utilizado para clasificar conjuntos de datos de catálogos."@es)
AnnotationAssertion(skos:definition dcat:themeTaxonomy "Il sistema di organizzazione della conoscenza (KOS) usato per classificare i dataset del catalogo."@it)
AnnotationAssertion(skos:definition dcat:themeTaxonomy "Le systhème d'ogranisation de connaissances utilisé pour classifier les jeux de données du catalogue."@fr)
AnnotationAssertion(skos:definition dcat:themeTaxonomy "Systém organizace znalostí (KOS) použitý pro klasifikaci datových sad v katalogu."@cs)
AnnotationAssertion(skos:definition dcat:themeTaxonomy "The knowledge organization system (KOS) used to classify catalog's datasets."@en)
AnnotationAssertion(skos:definition dcat:themeTaxonomy "Vidensorganiseringssystem (KOS) som anvendes til at klassificere datasæt i kataloget."@da)
AnnotationAssertion(skos:definition dcat:themeTaxonomy "Το σύστημα οργάνωσης γνώσης που χρησιμοποιείται για την κατηγοριοποίηση των συνόλων δεδομένων του καταλόγου."@el)
AnnotationAssertion(skos:definition dcat:themeTaxonomy "لائحة التصنيفات المستخدمه لتصنيف قوائم البيانات ضمن الفهرس"@ar)
AnnotationAssertion(skos:definition dcat:themeTaxonomy "カタログのデータセットを分類するために用いられる知識組織化体系（KOS；knowledge organization system）。"@ja)
AnnotationAssertion(skos:scopeNote dcat:themeTaxonomy "Det anbefales at taksonomien organiseres i et skos:ConceptScheme, skos:Collection, owl:Ontology eller lignende, som giver mulighed for at ethvert medlem af taksonomien kan forsynes med en IRI og udgives som linked-data."@da)
AnnotationAssertion(skos:scopeNote dcat:themeTaxonomy "It is recommended that the taxonomy is organized in a skos:ConceptScheme, skos:Collection, owl:Ontology or similar, which allows each member to be denoted by an IRI and published as linked-data."@en)
AnnotationAssertion(skos:scopeNote dcat:themeTaxonomy "Je doporučeno, aby byla taxonomie vyjádřena jako skos:ConceptScheme, skos:Collection, owl:Ontology nebo podobné, aby mohla být každá položka identifikována pomocí IRI a publikována jako propojená data."@cs)
AnnotationAssertion(skos:scopeNote dcat:themeTaxonomy "Se recomienda que la taxonomía se organice como un skos:ConceptScheme, skos:Collection, owl:Ontology o similar, los cuáles permiten que cada miembro se denote con una IRI y se publique como datos enlazados."@es)
AnnotationAssertion(skos:scopeNote dcat:themeTaxonomy "Si raccomanda che la tassonomia sia organizzata in uno skos:ConceptScheme, skos:Collection, owl:Ontology o simili, che permette ad ogni membro di essere indicato da un IRI e pubblicato come linked-data."@it)
ObjectPropertyDomain(dcat:themeTaxonomy dcat:Catalog)
ObjectPropertyRange(dcat:themeTaxonomy rdfs:Resource)

# Object Property: foaf:homepage (foaf:homepage)

AnnotationAssertion(rdfs:comment foaf:homepage "Este axioma se necesita de manera que Protege cargue DCAT3 sin problemas."@es)
AnnotationAssertion(rdfs:comment foaf:homepage "This axiom needed so that Protege loads DCAT 3 without errors."@en)

# Object Property: foaf:primaryTopic (foaf:primaryTopic)

AnnotationAssertion(rdfs:comment foaf:primaryTopic "Este axioma se necesita de manera que Protege cargue DCAT 3 sin problemas."@es)
AnnotationAssertion(rdfs:comment foaf:primaryTopic "This axiom needed so that Protege loads DCAT 3 without errors."@en)


############################
#   Data Properties
############################

# Data Property: dcterms:alternative (Alternative Title)

SubDataPropertyOf(dcterms:alternative dcterms:title)
DataPropertyRange(dcterms:alternative rdfs:Literal)

# Data Property: dcterms:available (Date Available)

SubDataPropertyOf(dcterms:available dcterms:date)
DataPropertyRange(dcterms:available rdfs:Literal)

# Data Property: dcterms:bibliographicCitation (Bibliographic Citation)

SubDataPropertyOf(dcterms:bibliographicCitation dcterms:identifier)
DataPropertyRange(dcterms:bibliographicCitation rdfs:Literal)

# Data Property: dcterms:created (Date Created)

SubDataPropertyOf(dcterms:created dcterms:date)
DataPropertyRange(dcterms:created rdfs:Literal)

# Data Property: dcterms:date (Date)

DataPropertyRange(dcterms:date rdfs:Literal)

# Data Property: dcterms:dateAccepted (Date Accepted)

SubDataPropertyOf(dcterms:dateAccepted dcterms:date)
DataPropertyRange(dcterms:dateAccepted rdfs:Literal)

# Data Property: dcterms:dateCopyrighted (Date Copyrighted)

SubDataPropertyOf(dcterms:dateCopyrighted dcterms:date)
DataPropertyRange(dcterms:dateCopyrighted rdfs:Literal)

# Data Property: dcterms:dateSubmitted (Date Submitted)

SubDataPropertyOf(dcterms:dateSubmitted dcterms:date)
DataPropertyRange(dcterms:dateSubmitted rdfs:Literal)

# Data Property: dcterms:identifier (Identifier)

DataPropertyRange(dcterms:identifier rdfs:Literal)

# Data Property: dcterms:issued (Date Issued)

SubDataPropertyOf(dcterms:issued dcterms:date)
DataPropertyRange(dcterms:issued rdfs:Literal)

# Data Property: dcterms:modified (Date Modified)

SubDataPropertyOf(dcterms:modified dcterms:date)
DataPropertyRange(dcterms:modified rdfs:Literal)

# Data Property: dcterms:title (Title)

DataPropertyRange(dcterms:title rdfs:Literal)

# Data Property: dcterms:valid (Date Valid)

SubDataPropertyOf(dcterms:valid dcterms:date)
DataPropertyRange(dcterms:valid rdfs:Literal)

# Data Property: dcat:bbox (bounding box)

AnnotationAssertion(rdfs:comment dcat:bbox "Den geografiske omskrevne firkant af en ressource."@da)
AnnotationAssertion(rdfs:comment dcat:bbox "El cuadro delimitador geográfico para un recurso."@es)
AnnotationAssertion(rdfs:comment dcat:bbox "Il riquadro di delimitazione geografica di una risorsa."@it)
AnnotationAssertion(rdfs:comment dcat:bbox "Ohraničení geografické oblasti zdroje."@cs)
AnnotationAssertion(rdfs:comment dcat:bbox "The geographic bounding box of a spatial thing [SDW-BP]."@en)
AnnotationAssertion(rdfs:isDefinedBy dcat:bbox <https://www.w3.org/TR/vocab-dcat-2/>)
AnnotationAssertion(rdfs:label dcat:bbox "bounding box"@da)
AnnotationAssertion(rdfs:label dcat:bbox "bounding box"@en)
AnnotationAssertion(rdfs:label dcat:bbox "cuadro delimitador"@es)
AnnotationAssertion(rdfs:label dcat:bbox "ohraničení oblasti"@cs)
AnnotationAssertion(rdfs:label dcat:bbox "quadro di delimitazione"@it)
AnnotationAssertion(skos:changeNote dcat:bbox "New property added in DCAT 2."@en)
AnnotationAssertion(skos:changeNote dcat:bbox "Nová vlastnost přidaná ve verzi DCAT 2."@cs)
AnnotationAssertion(skos:changeNote dcat:bbox "Nuova proprietà aggiunta in DCAT 2."@it)
AnnotationAssertion(skos:changeNote dcat:bbox "Ny egenskab tilføjet i DCAT 2."@da)
AnnotationAssertion(skos:changeNote dcat:bbox "Propiedad nueva agregada en DCAT 2."@es)
AnnotationAssertion(skos:definition dcat:bbox "Den geografiske omskrevne firkant af en ressource."@da)
AnnotationAssertion(skos:definition dcat:bbox "El cuadro delimitador geográfico para un recurso."@es)
AnnotationAssertion(skos:definition dcat:bbox "Il riquadro di delimitazione geografica di una risorsa."@it)
AnnotationAssertion(skos:definition dcat:bbox "Ohraničení geografické oblasti zdroje."@cs)
AnnotationAssertion(skos:definition dcat:bbox "The geographic bounding box of a spatial thing [SDW-BP]."@en)
AnnotationAssertion(skos:editorialNote dcat:bbox "English language definitions and comments updated in this revision in line with ED. Multilingual text unevenly updated."@en)
AnnotationAssertion(skos:scopeNote dcat:bbox "El rango de esta propiedad es intencionalmente genérico con el propósito de permitir distintas codificaciones geométricas. Por ejemplo, la geometría puede ser codificada como WKT (geosparql:wktLiteral [GeoSPARQL]) o [GML] (geosparql:asGML [GeoSPARQL])."@es)
AnnotationAssertion(skos:scopeNote dcat:bbox "Il range di questa proprietà (rdfs:Literal) è volutamente generica, con lo scopo di consentire diverse codifiche geometriche letterali. Ad esempio, la geometria potrebbe essere codificata con un letterale WKT (geosparql:wktLiteral [GeoSPARQL]) o [GML] (geosparql:asGML [GeoSPARQL])."@it)
AnnotationAssertion(skos:scopeNote dcat:bbox "Obor hodnot této vlastnosti je úmyslně obecný, aby umožnil různé kódování geometrií. Geometrie by kupříkladu mohla být kódována jako WKT (geosparql:wktLiteral [GeoSPARQL]) či [GML] (geosparql:asGML [GeoSPARQL])."@cs)
AnnotationAssertion(skos:scopeNote dcat:bbox "Rækkevidden for denne egenskab er bevidst generisk defineret med det formål at tillade forskellige kodninger af geometrier. Geometrien kan eksempelvis repræsenteres som WKT (geosparql:asWKT [GeoSPARQL]) eller [GML] (geosparql:asGML [GeoSPARQL])."@da)
AnnotationAssertion(skos:scopeNote dcat:bbox "The range of this property (rdfs:Literal) is intentionally generic, with the purpose of allowing different geometry literal encodings. E.g., the geometry could be encoded as a WKT literal (geosparql:wktLiteral [GeoSPARQL])."@en)
DataPropertyDomain(dcat:bbox dcterms:Location)
DataPropertyRange(dcat:bbox rdfs:Literal)

# Data Property: dcat:byteSize (taille en octects)

AnnotationAssertion(rdfs:comment dcat:byteSize "El tamaño de una distribución en bytes."@es)
AnnotationAssertion(rdfs:comment dcat:byteSize "La dimensione di una distribuzione in byte."@it)
AnnotationAssertion(rdfs:comment dcat:byteSize "La taille de la distribution en octects"@fr)
AnnotationAssertion(rdfs:comment dcat:byteSize "Størrelsen af en distributionen angivet i bytes."@da)
AnnotationAssertion(rdfs:comment dcat:byteSize "The size of a distribution in bytes."@en)
AnnotationAssertion(rdfs:comment dcat:byteSize "Velikost distribuce v bajtech."@cs)
AnnotationAssertion(rdfs:comment dcat:byteSize "Το μέγεθος μιας διανομής σε bytes."@el)
AnnotationAssertion(rdfs:comment dcat:byteSize "الحجم بالبايتات "@ar)
AnnotationAssertion(rdfs:comment dcat:byteSize "バイトによる配信のサイズ。"@ja)
AnnotationAssertion(rdfs:isDefinedBy dcat:byteSize <http://www.w3.org/TR/vocab-dcat/>)
AnnotationAssertion(rdfs:label dcat:byteSize "byte size"@en)
AnnotationAssertion(rdfs:label dcat:byteSize "bytestørrelse"@da)
AnnotationAssertion(rdfs:label dcat:byteSize "dimensione in byte"@it)
AnnotationAssertion(rdfs:label dcat:byteSize "taille en octects"@fr)
AnnotationAssertion(rdfs:label dcat:byteSize "tamaño en bytes"@es)
AnnotationAssertion(rdfs:label dcat:byteSize "velikost v bajtech"@cs)
AnnotationAssertion(rdfs:label dcat:byteSize "μέγεθος σε bytes"@el)
AnnotationAssertion(rdfs:label dcat:byteSize "الحجم بالبايت"@ar)
AnnotationAssertion(rdfs:label dcat:byteSize "バイト・サイズ"@ja)
AnnotationAssertion(skos:definition dcat:byteSize "El tamaño de una distribución en bytes."@es)
AnnotationAssertion(skos:definition dcat:byteSize "La dimensione di una distribuzione in byte."@it)
AnnotationAssertion(skos:definition dcat:byteSize "La taille de la distribution en octects."@fr)
AnnotationAssertion(skos:definition dcat:byteSize "Størrelsen af en distribution angivet i bytes."@da)
AnnotationAssertion(skos:definition dcat:byteSize "The size of a distribution in bytes."@en)
AnnotationAssertion(skos:definition dcat:byteSize "Velikost distribuce v bajtech."@cs)
AnnotationAssertion(skos:definition dcat:byteSize "Το μέγεθος μιας διανομής σε bytes."@el)
AnnotationAssertion(skos:definition dcat:byteSize "الحجم بالبايتات "@ar)
AnnotationAssertion(skos:definition dcat:byteSize "バイトによる配信のサイズ。"@ja)
AnnotationAssertion(skos:scopeNote dcat:byteSize "Bytestørrelsen kan approximeres hvis den præcise størrelse ikke er kendt. Værdien af dcat:byteSize bør angives som xsd:decimal."@da)
AnnotationAssertion(skos:scopeNote dcat:byteSize "El tamaño en bytes puede ser aproximado cuando se desconoce el tamaño exacto. El valor literal de dcat:byteSize debe tener tipo 'xsd:decimal'."@es)
AnnotationAssertion(skos:scopeNote dcat:byteSize "La dimensione in byte può essere approssimata quando non si conosce la dimensione precisa. Il valore di dcat:byteSize dovrebbe essere espresso come un xsd:decimal."@it)
AnnotationAssertion(skos:scopeNote dcat:byteSize "La taille en octects peut être approximative lorsque l'on ignore la taille réelle. La valeur littérale de dcat:byteSize doit être de type xsd:decimal."@fr)
AnnotationAssertion(skos:scopeNote dcat:byteSize "The size in bytes can be approximated when the precise size is not known. The literal value of dcat:byteSize should by typed as xsd:decimal."@en)
AnnotationAssertion(skos:scopeNote dcat:byteSize "Velikost v bajtech může být přibližná, pokud její přesná hodnota není známa. Literál s hodnotou dcat:byteSize by měl mít datový typ xsd:decimal."@cs)
AnnotationAssertion(skos:scopeNote dcat:byteSize "Το μέγεθος σε bytes μπορεί να προσεγγιστεί όταν η ακριβής τιμή δεν είναι γνωστή. Η τιμή της dcat:byteSize θα πρέπει να δίνεται με τύπο δεδομένων xsd:decimal."@el)
AnnotationAssertion(skos:scopeNote dcat:byteSize "الحجم يمكن أن يكون تقريبي إذا كان الحجم الدقيق غير معروف"@ar)
AnnotationAssertion(skos:scopeNote dcat:byteSize "正確なサイズが不明である場合、サイズは、バイトによる近似値を示すことができます。"@ja)
DataPropertyDomain(dcat:byteSize dcat:Distribution)
DataPropertyRange(dcat:byteSize rdfs:Literal)

# Data Property: dcat:centroid (centroide)

AnnotationAssertion(rdfs:comment dcat:centroid "Det geometrisk tyngdepunkt (centroid) for en ressource."@da)
AnnotationAssertion(rdfs:comment dcat:centroid "El centro geográfico (centroide) de un recurso."@es)
AnnotationAssertion(rdfs:comment dcat:centroid "Geografický střed (centroid) zdroje."@cs)
AnnotationAssertion(rdfs:comment dcat:centroid "Il centro geografico (centroide) di una risorsa."@it)
AnnotationAssertion(rdfs:comment dcat:centroid "The geographic center (centroid) of a spatial thing [SDW-BP]."@en)
AnnotationAssertion(rdfs:isDefinedBy dcat:centroid <https://www.w3.org/TR/vocab-dcat-2/>)
AnnotationAssertion(rdfs:label dcat:centroid "centroid"@cs)
AnnotationAssertion(rdfs:label dcat:centroid "centroid"@en)
AnnotationAssertion(rdfs:label dcat:centroid "centroide"@es)
AnnotationAssertion(rdfs:label dcat:centroid "centroide"@it)
AnnotationAssertion(rdfs:label dcat:centroid "geometrisk tyngdepunkt"@da)
AnnotationAssertion(skos:altLabel dcat:centroid "centroide"@da)
AnnotationAssertion(skos:changeNote dcat:centroid "New property added in DCAT 2."@en)
AnnotationAssertion(skos:changeNote dcat:centroid "Nová vlastnost přidaná ve verzi DCAT 2."@cs)
AnnotationAssertion(skos:changeNote dcat:centroid "Nueva propiedad agregada en DCAT 2."@es)
AnnotationAssertion(skos:changeNote dcat:centroid "Nuova proprietà aggiunta in DCAT 2."@it)
AnnotationAssertion(skos:changeNote dcat:centroid "Ny egenskab tilføjet i DCAT 2."@da)
AnnotationAssertion(skos:definition dcat:centroid "Det geometrisk tyngdepunkt (centroid) for en ressource."@da)
AnnotationAssertion(skos:definition dcat:centroid "El centro geográfico (centroide) de un recurso."@es)
AnnotationAssertion(skos:definition dcat:centroid "Geografický střed (centroid) zdroje."@cs)
AnnotationAssertion(skos:definition dcat:centroid "Il centro geografico (centroide) di una risorsa."@it)
AnnotationAssertion(skos:definition dcat:centroid "The geographic center (centroid) of a spatial thing [SDW-BP]."@en)
AnnotationAssertion(skos:editorialNote dcat:centroid "English language definitions and comments updated in this revision in line with ED. Multilingual text unevenly updated."@en)
AnnotationAssertion(skos:scopeNote dcat:centroid "El rango de esta propiedad es intencionalmente genérico con el objetivo de permitir distintas codificaciones geométricas. Por ejemplo, la geometría puede codificarse como WKT (geosparql:wktLiteral [GeoSPARQL]) o [GML] (geosparql:asGML [GeoSPARQL])."@es)
AnnotationAssertion(skos:scopeNote dcat:centroid "Il range di questa proprietà (rdfs:Literal) è volutamente generica, con lo scopo di consentire diverse codifiche geometriche letterali. Ad esempio, la geometria potrebbe essere codificata con un letterale WKT (geosparql:wktLiteral [GeoSPARQL]) o [GML] (geosparql:asGML [GeoSPARQL])."@it)
AnnotationAssertion(skos:scopeNote dcat:centroid "Obor hodnot této vlastnosti je úmyslně obecný, aby umožnil různé kódování geometrií. Geometrie by kupříkladu mohla být kódována jako WKT (geosparql:wktLiteral [GeoSPARQL]) či [GML] (geosparql:asGML [GeoSPARQL])."@cs)
AnnotationAssertion(skos:scopeNote dcat:centroid "Rækkevidden for denne egenskab er bevidst generisk definere med det formål at tillade forskellige geokodninger. Geometrien kan eksempelvis repræsenteres som WKT (geosparql:asWKT [GeoSPARQL]) eller [GML] (geosparql:asGML [GeoSPARQL])."@da)
AnnotationAssertion(skos:scopeNote dcat:centroid "The range of this property (rdfs:Literal) is intentionally generic, with the purpose of allowing different geometry literal encodings. E.g., the geometry could be encoded as a WKT literal (geosparql:wktLiteral [GeoSPARQL])."@en)
DataPropertyDomain(dcat:centroid dcterms:Location)
DataPropertyRange(dcat:centroid rdfs:Literal)

# Data Property: dcat:endDate (fecha final)

AnnotationAssertion(rdfs:comment dcat:endDate "El fin del período."@es)
AnnotationAssertion(rdfs:comment dcat:endDate "Konec doby trvání."@cs)
AnnotationAssertion(rdfs:comment dcat:endDate "La fine del periodo."@it)
AnnotationAssertion(rdfs:comment dcat:endDate "Slutningen på perioden."@da)
AnnotationAssertion(rdfs:comment dcat:endDate "The end of the period."@en)
AnnotationAssertion(rdfs:isDefinedBy dcat:endDate <https://www.w3.org/TR/vocab-dcat-2/>)
AnnotationAssertion(rdfs:label dcat:endDate "data di fine"@it)
AnnotationAssertion(rdfs:label dcat:endDate "datum konce"@cs)
AnnotationAssertion(rdfs:label dcat:endDate "end date"@en)
AnnotationAssertion(rdfs:label dcat:endDate "fecha final"@es)
AnnotationAssertion(rdfs:label dcat:endDate "slutdato"@da)
AnnotationAssertion(skos:altLabel dcat:endDate "sluttidspunkt"@da)
AnnotationAssertion(skos:changeNote dcat:endDate "New property added in DCAT 2."@en)
AnnotationAssertion(skos:changeNote dcat:endDate "Nová vlastnost přidaná ve verzi DCAT 2."@cs)
AnnotationAssertion(skos:changeNote dcat:endDate "Nueva propiedad agregada en DCAT 2."@es)
AnnotationAssertion(skos:changeNote dcat:endDate "Nuova proprietà aggiunta in DCAT 2."@it)
AnnotationAssertion(skos:changeNote dcat:endDate "Ny egenskab i DCAT 2."@da)
AnnotationAssertion(skos:definition dcat:endDate "El fin del período."@es)
AnnotationAssertion(skos:definition dcat:endDate "Konec doby trvání."@cs)
AnnotationAssertion(skos:definition dcat:endDate "La fine del periodo."@it)
AnnotationAssertion(skos:definition dcat:endDate "Slutningen på perioden."@da)
AnnotationAssertion(skos:definition dcat:endDate "The end of the period."@en)
AnnotationAssertion(skos:scopeNote dcat:endDate "El rango de esta propiedad es intencionalmente genérico con el propósito de permitir distintos niveles de precisión temporal para especificar el fin del período. Por ejemplo, puede expresarse como una fecha (xsd:date), una fecha y un tiempo (xsd:dateTime), o un año (xsd:gYear)."@es)
AnnotationAssertion(skos:scopeNote dcat:endDate "La range di questa proprietà è volutamente generico, con lo scopo di consentire diversi livelli di precisione temporale per specificare la fine di un periodo. Ad esempio, può essere espresso con una data (xsd:date), una data e un'ora (xsd:dateTime), o un anno (xsd:gYear)."@it)
AnnotationAssertion(skos:scopeNote dcat:endDate "Obor hodnot této vlastnosti je úmyslně obecný, aby umožnil různé úrovně časového rozlišení pro specifikaci konce doby trvání. Ten může být kupříkladu vyjádřen datumem (xsd:date), datumem a časem (xsd:dateTime) či rokem (xsd:gYear)."@cs)
AnnotationAssertion(skos:scopeNote dcat:endDate "Rækkeviden for denne egenskab er bevidst generisk defineret med det formål at tillade forskellige niveauer af tidslig præcision ifm. angivelse af slutdatoen for en periode. Den kan eksempelvis udtrykkes som en dato (xsd:date), en dato og et tidspunkt (xsd:dateTime), eller et årstal (xsd:gYear)."@da)
AnnotationAssertion(skos:scopeNote dcat:endDate "The range of this property is intentionally generic, with the purpose of allowing different level of temporal precision for specifying the end of a period. E.g., it can be expressed with a date (xsd:date), a date and time (xsd:dateTime), or a year (xsd:gYear)."@en)
DataPropertyDomain(dcat:endDate dcterms:PeriodOfTime)
DataPropertyRange(dcat:endDate rdfs:Literal)

# Data Property: dcat:keyword (nøgleord)

AnnotationAssertion(rdfs:comment dcat:keyword "A keyword or tag describing a resource."@en)
AnnotationAssertion(rdfs:comment dcat:keyword "Et nøgleord eller tag til beskrivelse af en ressource."@da)
AnnotationAssertion(rdfs:comment dcat:keyword "Klíčové slovo nebo značka popisující zdroj."@cs)
AnnotationAssertion(rdfs:comment dcat:keyword "Un mot-clé ou étiquette décrivant une ressource."@fr)
AnnotationAssertion(rdfs:comment dcat:keyword "Una palabra clave o etiqueta que describe un recurso."@es)
AnnotationAssertion(rdfs:comment dcat:keyword "Una parola chiave o un'etichetta per descrivere la risorsa."@it)
AnnotationAssertion(rdfs:comment dcat:keyword "Μία λέξη-κλειδί ή μία ετικέτα που περιγράφει το σύνολο δεδομένων."@el)
AnnotationAssertion(rdfs:comment dcat:keyword "كلمة  مفتاحيه توصف قائمة البيانات"@ar)
AnnotationAssertion(rdfs:comment dcat:keyword "データセットを記述しているキーワードまたはタグ。"@ja)
AnnotationAssertion(rdfs:isDefinedBy dcat:keyword <http://www.w3.org/TR/vocab-dcat/>)
AnnotationAssertion(rdfs:label dcat:keyword "keyword"@en)
AnnotationAssertion(rdfs:label dcat:keyword "klíčové slovo"@cs)
AnnotationAssertion(rdfs:label dcat:keyword "mot-clés "@fr)
AnnotationAssertion(rdfs:label dcat:keyword "nøgleord"@da)
AnnotationAssertion(rdfs:label dcat:keyword "palabra clave"@es)
AnnotationAssertion(rdfs:label dcat:keyword "parola chiave"@it)
AnnotationAssertion(rdfs:label dcat:keyword "λέξη-κλειδί"@el)
AnnotationAssertion(rdfs:label dcat:keyword "كلمة  مفتاحية "@ar)
AnnotationAssertion(rdfs:label dcat:keyword "キーワード/タグ"@ja)
AnnotationAssertion(skos:definition dcat:keyword "A keyword or tag describing a resource."@en)
AnnotationAssertion(skos:definition dcat:keyword "Et nøgleord eller tag til beskrivelse af en ressource."@da)
AnnotationAssertion(skos:definition dcat:keyword "Klíčové slovo nebo značka popisující zdroj."@cs)
AnnotationAssertion(skos:definition dcat:keyword "Un mot-clé ou étiquette décrivant une ressource."@fr)
AnnotationAssertion(skos:definition dcat:keyword "Una palabra clave o etiqueta que describe un recurso."@es)
AnnotationAssertion(skos:definition dcat:keyword "Una parola chiave o un'etichetta per descrivere la risorsa."@it)
AnnotationAssertion(skos:definition dcat:keyword "Μία λέξη-κλειδί ή μία ετικέτα που περιγράφει το σύνολο δεδομένων."@el)
AnnotationAssertion(skos:definition dcat:keyword "كلمة  مفتاحيه توصف قائمة البيانات"@ar)
AnnotationAssertion(skos:definition dcat:keyword "データセットを記述しているキーワードまたはタグ。"@ja)
DataPropertyRange(dcat:keyword rdfs:Literal)

# Data Property: dcat:spatialResolutionInMeters (geografisk opløsning (meter))

AnnotationAssertion(rdfs:comment dcat:spatialResolutionInMeters "mindste geografiske afstand som kan erkendes i et datasæt, målt i meter."@da)
AnnotationAssertion(rdfs:comment dcat:spatialResolutionInMeters "minimum spatial separation resolvable in a dataset, measured in meters."@en-us)
AnnotationAssertion(rdfs:comment dcat:spatialResolutionInMeters "minimum spatial separation resolvable in a dataset, measured in metres."@en-gb)
AnnotationAssertion(rdfs:comment dcat:spatialResolutionInMeters "minimální prostorový rozestup rozeznatelný v datové sadě, měřeno v metrech."@cs)
AnnotationAssertion(rdfs:comment dcat:spatialResolutionInMeters "mínima separacíon espacial disponible en un conjunto de datos, medida en metros."@es)
AnnotationAssertion(rdfs:comment dcat:spatialResolutionInMeters "separazione spaziale minima risolvibile in un set di dati, misurata in metri."@it)
AnnotationAssertion(rdfs:isDefinedBy dcat:spatialResolutionInMeters <https://www.w3.org/TR/vocab-dcat-2/>)
AnnotationAssertion(rdfs:label dcat:spatialResolutionInMeters "geografisk opløsning (meter)"@da)
AnnotationAssertion(rdfs:label dcat:spatialResolutionInMeters "prostorové rozlišení (metry)"@cs)
AnnotationAssertion(rdfs:label dcat:spatialResolutionInMeters "resolución espacial (metros)"@es)
AnnotationAssertion(rdfs:label dcat:spatialResolutionInMeters "risoluzione spaziale (metri)"@it)
AnnotationAssertion(rdfs:label dcat:spatialResolutionInMeters "spatial resolution (meters)"@en-us)
AnnotationAssertion(rdfs:label dcat:spatialResolutionInMeters "spatial resolution (metres)"@en-gb)
AnnotationAssertion(skos:changeNote dcat:spatialResolutionInMeters "New property added in DCAT 2."@en)
AnnotationAssertion(skos:changeNote dcat:spatialResolutionInMeters "Nová vlastnost přidaná ve verzi DCAT 2."@cs)
AnnotationAssertion(skos:changeNote dcat:spatialResolutionInMeters "Nueva propiedad añadida en DCAT 2."@es)
AnnotationAssertion(skos:changeNote dcat:spatialResolutionInMeters "Nuova proprietà aggiunta in DCAT 2."@it)
AnnotationAssertion(skos:changeNote dcat:spatialResolutionInMeters "Ny genskab tilføjet i DCAT 2."@da)
AnnotationAssertion(skos:definition dcat:spatialResolutionInMeters "mindste geografiske afstand som kan resolveres i et datasæt, målt i meter."@da)
AnnotationAssertion(skos:definition dcat:spatialResolutionInMeters "minimum spatial separation resolvable in a dataset, measured in meters."@en-us)
AnnotationAssertion(skos:definition dcat:spatialResolutionInMeters "minimum spatial separation resolvable in a dataset, measured in metres."@en-gb)
AnnotationAssertion(skos:definition dcat:spatialResolutionInMeters "minimální prostorový rozestup rozeznatelný v datové sadě, měřeno v metrech."@cs)
AnnotationAssertion(skos:definition dcat:spatialResolutionInMeters "mínima separacíon espacial disponible en un conjunto de datos, medida en metros."@es)
AnnotationAssertion(skos:definition dcat:spatialResolutionInMeters "separazione spaziale minima risolvibile in un set di dati, misurata in metri."@it)
AnnotationAssertion(skos:editorialNote dcat:spatialResolutionInMeters "Kan optræde i forbindelse med beskrivelse af datasættet eller datasætditributionen, så der er ikke angivet et domæne for egenskaben."@da)
AnnotationAssertion(skos:editorialNote dcat:spatialResolutionInMeters "Might appear in the description of a Dataset or a Distribution, so no domain is specified."@en)
AnnotationAssertion(skos:editorialNote dcat:spatialResolutionInMeters "Může se vyskytnout v popisu Datové sady nebo Distribuce, takže nebyl specifikován definiční obor."@cs)
AnnotationAssertion(skos:scopeNote dcat:spatialResolutionInMeters "Alternative geografiske opløsninger kan leveres som forskellige datasætdistributioner."@da)
AnnotationAssertion(skos:scopeNote dcat:spatialResolutionInMeters "Alternative spatial resolutions might be provided as different dataset distributions."@en)
AnnotationAssertion(skos:scopeNote dcat:spatialResolutionInMeters "Distintas distribuciones de un conjunto de datos pueden tener resoluciones espaciales diferentes."@es)
AnnotationAssertion(skos:scopeNote dcat:spatialResolutionInMeters "Hvis datasættet udgøres af et billede eller et grid, så bør dette svare til afstanden mellem elementerne. For andre typer af spatiale datasæt, vil denne egenskab typisk indikere den mindste afstand mellem elementerne i datasættet."@da)
AnnotationAssertion(skos:scopeNote dcat:spatialResolutionInMeters "If the dataset is an image or grid this should correspond to the spacing of items. For other kinds of spatial dataset, this property will usually indicate the smallest distance between items in the dataset."@en)
AnnotationAssertion(skos:scopeNote dcat:spatialResolutionInMeters "Pokud je datová sada obraz či mřížka, měla by tato vlastnost odpovídat rozestupu položek. Pro ostatní druhy prostorových datových sad bude tato vlastnost obvykle indikovat nejmenší vzdálenost mezi položkami této datové sady."@cs)
AnnotationAssertion(skos:scopeNote dcat:spatialResolutionInMeters "Risoluzioni spaziali alternative possono essere fornite come diverse distribuzioni di set di dati."@it)
AnnotationAssertion(skos:scopeNote dcat:spatialResolutionInMeters "Různá prostorová rozlišení mohou být poskytována jako různé distribuce datové sady."@cs)
AnnotationAssertion(skos:scopeNote dcat:spatialResolutionInMeters "Se il set di dati è un'immagine o una griglia, questo dovrebbe corrispondere alla spaziatura degli elementi. Per altri tipi di set di dati spaziali, questa proprietà di solito indica la distanza minima tra gli elementi nel set di dati."@it)
AnnotationAssertion(skos:scopeNote dcat:spatialResolutionInMeters "Si el conjunto de datos es una imágen o grilla, esta propiedad corresponde al espaciado de los elementos. Para otro tipo de conjunto de datos espaciales, esta propieda usualmente indica la menor distancia entre los elementos de dichos datos."@es)
DataPropertyRange(dcat:spatialResolutionInMeters xsd:decimal)

# Data Property: dcat:startDate (data di inizio)

AnnotationAssertion(rdfs:isDefinedBy dcat:startDate <https://www.w3.org/TR/vocab-dcat-2/>)
AnnotationAssertion(rdfs:label dcat:startDate "data di inizio"@it)
AnnotationAssertion(rdfs:label dcat:startDate "datum začátku"@cs)
AnnotationAssertion(rdfs:label dcat:startDate "start date"@en)
AnnotationAssertion(rdfs:label dcat:startDate "startdato"@da)
AnnotationAssertion(skos:altLabel dcat:startDate "starttidspunkt"@da)
AnnotationAssertion(skos:changeNote dcat:startDate "New property added in DCAT 2."@en)
AnnotationAssertion(skos:changeNote dcat:startDate "Nová vlastnost přidaná ve verzi DCAT 2."@cs)
AnnotationAssertion(skos:changeNote dcat:startDate "Nueva propiedad agregada en DCAT 2."@es)
AnnotationAssertion(skos:changeNote dcat:startDate "Nuova proprietà aggiunta in DCAT 2."@it)
AnnotationAssertion(skos:changeNote dcat:startDate "Ny egenskab tilføjet i DCAT 2."@da)
AnnotationAssertion(skos:definition dcat:startDate "El comienzo del período"@es)
AnnotationAssertion(skos:definition dcat:startDate "L'inizio del periodo"@it)
AnnotationAssertion(skos:definition dcat:startDate "Start på perioden."@da)
AnnotationAssertion(skos:definition dcat:startDate "The start of the period"@en)
AnnotationAssertion(skos:definition dcat:startDate "Začátek doby trvání"@cs)
AnnotationAssertion(skos:scopeNote dcat:startDate "El rango de esta propiedad es intencionalmente genérico con el propósito de permitir distintos niveles de precisión temporal para especificar el comienzo de un período. Por ejemplo, puede expresarse como una fecha (xsd:date), una fecha y un tiempo (xsd:dateTime), o un año (xsd:gYear)."@es)
AnnotationAssertion(skos:scopeNote dcat:startDate "Il range di questa proprietà è volutamente generico, con lo scopo di consentire diversi livelli di precisione temporale per specificare l'inizio di un periodo. Ad esempio, può essere espresso con una data (xsd:date), una data e un'ora (xsd:dateTime), o un anno (xsd:gYear)."@it)
AnnotationAssertion(skos:scopeNote dcat:startDate "Obor hodnot této vlastnosti je úmyslně obecný, aby umožnil různé úrovně časového rozlišení pro specifikaci začátku doby trvání. Ten může být kupříkladu vyjádřen datumem (xsd:date), datumem a časem (xsd:dateTime) či rokem (xsd:gYear)."@cs)
AnnotationAssertion(skos:scopeNote dcat:startDate "Rækkeviden for denne egenskab er bevidst generisk defineret med det formål at tillade forskellige niveauer af tidslig præcision ifm. angivelse af startdatoen for en periode. Den kan eksempelvis udtrykkes som en dato (xsd:date), en dato og et tidspunkt (xsd:dateTime), eller et årstal (xsd:gYear)."@da)
AnnotationAssertion(skos:scopeNote dcat:startDate "The range of this property is intentionally generic, with the purpose of allowing different level of temporal precision for specifying the start of a period. E.g., it can be expressed with a date (xsd:date), a date and time (xsd:dateTime), or a year (xsd:gYear)."@en)
DataPropertyDomain(dcat:startDate dcterms:PeriodOfTime)
DataPropertyRange(dcat:startDate rdfs:Literal)

# Data Property: dcat:temporalResolution (temporal resolution)

AnnotationAssertion(rdfs:comment dcat:temporalResolution "mindste tidsperiode der kan resolveres i datasættet."@da)
AnnotationAssertion(rdfs:comment dcat:temporalResolution "minimum time period resolvable in a dataset."@en)
AnnotationAssertion(rdfs:comment dcat:temporalResolution "minimální doba trvání rozlišitelná v datové sadě."@cs)
AnnotationAssertion(rdfs:comment dcat:temporalResolution "periodo di tempo minimo risolvibile in un set di dati."@it)
AnnotationAssertion(rdfs:comment dcat:temporalResolution "período de tiempo mínimo en el conjunto de datos."@es)
AnnotationAssertion(rdfs:isDefinedBy dcat:temporalResolution <https://www.w3.org/TR/vocab-dcat-2/>)
AnnotationAssertion(rdfs:label dcat:temporalResolution "resolución temporal"@es)
AnnotationAssertion(rdfs:label dcat:temporalResolution "risoluzione temporale"@it)
AnnotationAssertion(rdfs:label dcat:temporalResolution "temporal resolution"@en)
AnnotationAssertion(rdfs:label dcat:temporalResolution "tidslig opløsning"@da)
AnnotationAssertion(rdfs:label dcat:temporalResolution "časové rozlišení"@cs)
AnnotationAssertion(skos:changeNote dcat:temporalResolution "New property added in DCAT 2."@en)
AnnotationAssertion(skos:changeNote dcat:temporalResolution "Nová vlastnost přidaná ve verzi DCAT 2."@cs)
AnnotationAssertion(skos:changeNote dcat:temporalResolution "Nueva propiedad añadida en DCAT 2."@es)
AnnotationAssertion(skos:changeNote dcat:temporalResolution "Nuova proprietà aggiunta in DCAT 2."@it)
AnnotationAssertion(skos:definition dcat:temporalResolution "mindste tidsperiode der kan resolveres i datasættet."@da)
AnnotationAssertion(skos:definition dcat:temporalResolution "minimum time period resolvable in a dataset."@en)
AnnotationAssertion(skos:definition dcat:temporalResolution "minimální doba trvání rozlišitelná v datové sadě."@cs)
AnnotationAssertion(skos:definition dcat:temporalResolution "periodo di tempo minimo risolvibile in un set di dati."@it)
AnnotationAssertion(skos:definition dcat:temporalResolution "período de tiempo mínimo en el conjunto de datos."@es)
AnnotationAssertion(skos:editorialNote dcat:temporalResolution "Kan optræde i forbindelse med beskrivelse af datasættet eller datasætditributionen, så der er ikke angivet et domæne for egenskaben."@da)
AnnotationAssertion(skos:editorialNote dcat:temporalResolution "Might appear in the description of a Dataset or a Distribution, so no domain is specified."@en)
AnnotationAssertion(skos:editorialNote dcat:temporalResolution "Může se vyskytnout v popisu Datové sady nebo Distribuce, takže nebyl specifikován definiční obor."@cs)
AnnotationAssertion(skos:scopeNote dcat:temporalResolution "Alternative temporal resolutions might be provided as different dataset distributions."@en)
AnnotationAssertion(skos:scopeNote dcat:temporalResolution "Alternative tidslige opløsninger kan leveres som forskellige datasætdistributioner."@da)
AnnotationAssertion(skos:scopeNote dcat:temporalResolution "Distintas distribuciones del conjunto de datos pueden tener resoluciones temporales diferentes."@es)
AnnotationAssertion(skos:scopeNote dcat:temporalResolution "Hvis datasættet er en tidsserie, så bør denne egenskab svare til afstanden mellem elementerne i tidsserien. For andre typer af datasæt indikerer denne egenskab den mindste tidsforskel mellem elementer i datasættet."@da)
AnnotationAssertion(skos:scopeNote dcat:temporalResolution "If the dataset is a time-series this should correspond to the spacing of items in the series. For other kinds of dataset, this property will usually indicate the smallest time difference between items in the dataset."@en)
AnnotationAssertion(skos:scopeNote dcat:temporalResolution "Pokud je datová sada časovou řadou, měla by tato vlastnost odpovídat rozestupu položek v řadě. Pro ostatní druhy datových sad bude tato vlastnost obvykle indikovat nejmenší časovou vzdálenost mezi položkami této datové sady."@cs)
AnnotationAssertion(skos:scopeNote dcat:temporalResolution "Risoluzioni temporali alternative potrebbero essere fornite come diverse distribuzioni di set di dati."@it)
AnnotationAssertion(skos:scopeNote dcat:temporalResolution "Různá časová rozlišení mohou být poskytována jako různé distribuce datové sady."@cs)
AnnotationAssertion(skos:scopeNote dcat:temporalResolution "Se il set di dati è una serie temporale, questo dovrebbe corrispondere alla spaziatura degli elementi della serie. Per altri tipi di set di dati, questa proprietà di solito indica la più piccola differenza di tempo tra gli elementi nel set di dati."@it)
AnnotationAssertion(skos:scopeNote dcat:temporalResolution "Si el conjunto de datos es una serie temporal, debe corresponder al espaciado de los elementos de la serie. Para otro tipo de conjuntos de datos, esta propiedad indicará usualmente la menor diferencia de tiempo entre elementos en el dataset."@es)
DataPropertyRange(dcat:temporalResolution xsd:duration)

# Data Property: dcat:version (versión)

AnnotationAssertion(rdfs:comment dcat:version "El indicador de versión (nombre o identificador) del recurso."@es)
AnnotationAssertion(rdfs:comment dcat:version "L'indicatore di versione (un nome o un identificatore) di una risorsa."@it)
AnnotationAssertion(rdfs:comment dcat:version "The version indicator (name or identifier) of a resource."@en)
AnnotationAssertion(rdfs:isDefinedBy dcat:version <https://www.w3.org/TR/vocab-dcat-3/>)
AnnotationAssertion(rdfs:label dcat:version "version"@en)
AnnotationAssertion(rdfs:label dcat:version "versione"@it)
AnnotationAssertion(rdfs:label dcat:version "versión"@es)
AnnotationAssertion(skos:changeNote dcat:version "New property added in DCAT 3."@en)
AnnotationAssertion(skos:changeNote dcat:version "Nová vlastnost přidaná ve verzi DCAT 3."@cs)
AnnotationAssertion(skos:changeNote dcat:version "Nueva propiedad agregada in DCAT 3."@es)
AnnotationAssertion(skos:changeNote dcat:version "Nuova proprietà aggiunta in DCAT 3."@it)
AnnotationAssertion(skos:changeNote dcat:version "Ny egenskab tilføjet i DCAT 3."@da)
AnnotationAssertion(skos:definition dcat:version "El indicador de versión (nombre o identificador) del recurso."@es)
AnnotationAssertion(skos:definition dcat:version "L'indicatore di versione (un nome o un identificatore) di una risorsa"@it)
AnnotationAssertion(skos:definition dcat:version "The version indicator (name or identifier) of a resource."@en)
AnnotationAssertion(skos:scopeNote dcat:version "DCAT does not prescribe how a version name / identifier should be specified, and refers for guidance to [DWBP]'s Best Practice 7: Provide a version indicator."@en)
AnnotationAssertion(skos:scopeNote dcat:version "DCAT no prescribe cómo especificar el nombre or identificador de una versión, y como guía sugiere leer las práctica 7 en [DWBP] sobre cómo proveer un indicador de versión"@es)
AnnotationAssertion(skos:scopeNote dcat:version "DCAT non prescrive come un nome o identificatore di versione dovrebbe essere specificato, e fa riferimento alle linee guida indicate in [DWBP] Best Practice 7: Provide a version indicator."@it)


############################
#   Datatypes
############################

# Datatype: dcterms:Box (DCMI Box)

AnnotationAssertion(rdfs:comment dcterms:Box "The set of regions in space defined by their geographic coordinates according to the DCMI Box Encoding Scheme."@en)
AnnotationAssertion(rdfs:isDefinedBy dcterms:Box <http://purl.org/dc/terms/>)
AnnotationAssertion(rdfs:label dcterms:Box "DCMI Box"@en)
AnnotationAssertion(rdfs:seeAlso dcterms:Box <https://www.dublincore.org/specifications/dublin-core/dcmi-box/>)

# Datatype: dcterms:ISO3166 (ISO 3166)

AnnotationAssertion(rdfs:comment dcterms:ISO3166 "The set of codes listed in ISO 3166-1 for the representation of names of countries."@en)
AnnotationAssertion(rdfs:isDefinedBy dcterms:ISO3166 <http://purl.org/dc/terms/>)
AnnotationAssertion(rdfs:label dcterms:ISO3166 "ISO 3166"@en)
AnnotationAssertion(rdfs:seeAlso dcterms:ISO3166 <https://www.iso.org/obp/ui/#search>)

# Datatype: dcterms:ISO639-2 (ISO 639-2)

AnnotationAssertion(rdfs:comment dcterms:ISO639-2 "The three-letter alphabetic codes listed in ISO639-2 for the representation of names of languages."@en)
AnnotationAssertion(rdfs:isDefinedBy dcterms:ISO639-2 <http://purl.org/dc/terms/>)
AnnotationAssertion(rdfs:label dcterms:ISO639-2 "ISO 639-2"@en)
AnnotationAssertion(rdfs:seeAlso dcterms:ISO639-2 <http://lcweb.loc.gov/standards/iso639-2/langhome.html>)

# Datatype: dcterms:ISO639-3 (ISO 639-3)

AnnotationAssertion(rdfs:comment dcterms:ISO639-3 "The set of three-letter codes listed in ISO 639-3 for the representation of names of languages."@en)
AnnotationAssertion(rdfs:isDefinedBy dcterms:ISO639-3 <http://purl.org/dc/terms/>)
AnnotationAssertion(rdfs:label dcterms:ISO639-3 "ISO 639-3"@en)
AnnotationAssertion(rdfs:seeAlso dcterms:ISO639-3 <http://www.sil.org/iso639-3/>)

# Datatype: dcterms:Period (DCMI Period)

AnnotationAssertion(rdfs:comment dcterms:Period "The set of time intervals defined by their limits according to the DCMI Period Encoding Scheme."@en)
AnnotationAssertion(rdfs:isDefinedBy dcterms:Period <http://purl.org/dc/terms/>)
AnnotationAssertion(rdfs:label dcterms:Period "DCMI Period"@en)
AnnotationAssertion(rdfs:seeAlso dcterms:Period <https://www.dublincore.org/specifications/dublin-core/dcmi-period/>)

# Datatype: dcterms:Point (DCMI Point)

AnnotationAssertion(rdfs:comment dcterms:Point "The set of points in space defined by their geographic coordinates according to the DCMI Point Encoding Scheme."@en)
AnnotationAssertion(rdfs:isDefinedBy dcterms:Point <http://purl.org/dc/terms/>)
AnnotationAssertion(rdfs:label dcterms:Point "DCMI Point"@en)
AnnotationAssertion(rdfs:seeAlso dcterms:Point <https://www.dublincore.org/specifications/dublin-core/dcmi-point/>)

# Datatype: dcterms:RFC1766 (RFC 1766)

AnnotationAssertion(rdfs:comment dcterms:RFC1766 "The set of tags, constructed according to RFC 1766, for the identification of languages."@en)
AnnotationAssertion(rdfs:isDefinedBy dcterms:RFC1766 <http://purl.org/dc/terms/>)
AnnotationAssertion(rdfs:label dcterms:RFC1766 "RFC 1766"@en)
AnnotationAssertion(rdfs:seeAlso dcterms:RFC1766 <http://www.ietf.org/rfc/rfc1766.txt>)

# Datatype: dcterms:RFC3066 (RFC 3066)

AnnotationAssertion(dcterms:description dcterms:RFC3066 "RFC 3066 has been obsoleted by RFC 4646."@en)
AnnotationAssertion(rdfs:comment dcterms:RFC3066 "The set of tags constructed according to RFC 3066 for the identification of languages."@en)
AnnotationAssertion(rdfs:isDefinedBy dcterms:RFC3066 <http://purl.org/dc/terms/>)
AnnotationAssertion(rdfs:label dcterms:RFC3066 "RFC 3066"@en)
AnnotationAssertion(rdfs:seeAlso dcterms:RFC3066 <http://www.ietf.org/rfc/rfc3066.txt>)

# Datatype: dcterms:RFC4646 (RFC 4646)

AnnotationAssertion(dcterms:description dcterms:RFC4646 "RFC 4646 obsoletes RFC 3066."@en)
AnnotationAssertion(rdfs:comment dcterms:RFC4646 "The set of tags constructed according to RFC 4646 for the identification of languages."@en)
AnnotationAssertion(rdfs:isDefinedBy dcterms:RFC4646 <http://purl.org/dc/terms/>)
AnnotationAssertion(rdfs:label dcterms:RFC4646 "RFC 4646"@en)
AnnotationAssertion(rdfs:seeAlso dcterms:RFC4646 <http://www.ietf.org/rfc/rfc4646.txt>)

# Datatype: dcterms:RFC5646 (RFC 5646)

AnnotationAssertion(dcterms:description dcterms:RFC5646 "RFC 5646 obsoletes RFC 4646."@en)
AnnotationAssertion(rdfs:comment dcterms:RFC5646 "The set of tags constructed according to RFC 5646 for the identification of languages."@en)
AnnotationAssertion(rdfs:isDefinedBy dcterms:RFC5646 <http://purl.org/dc/terms/>)
AnnotationAssertion(rdfs:label dcterms:RFC5646 "RFC 5646"@en)
AnnotationAssertion(rdfs:seeAlso dcterms:RFC5646 <http://www.ietf.org/rfc/rfc5646.txt>)

# Datatype: dcterms:URI (URI)

AnnotationAssertion(rdfs:comment dcterms:URI "The set of identifiers constructed according to the generic syntax for Uniform Resource Identifiers as specified by the Internet Engineering Task Force."@en)
AnnotationAssertion(rdfs:isDefinedBy dcterms:URI <http://purl.org/dc/terms/>)
AnnotationAssertion(rdfs:label dcterms:URI "URI"@en)
AnnotationAssertion(rdfs:seeAlso dcterms:URI <http://www.ietf.org/rfc/rfc3986.txt>)

# Datatype: dcterms:W3CDTF (W3C-DTF)

AnnotationAssertion(rdfs:comment dcterms:W3CDTF "The set of dates and times constructed according to the W3C Date and Time Formats Specification."@en)
AnnotationAssertion(rdfs:isDefinedBy dcterms:W3CDTF <http://purl.org/dc/terms/>)
AnnotationAssertion(rdfs:label dcterms:W3CDTF "W3C-DTF"@en)
AnnotationAssertion(rdfs:seeAlso dcterms:W3CDTF <http://www.w3.org/TR/NOTE-datetime>)


############################
#   Classes
############################

# Class: dcterms:Agent (Agent)

AnnotationAssertion(rdfs:comment dcterms:Agent "A resource that acts or has the power to act."@en)
AnnotationAssertion(rdfs:isDefinedBy dcterms:Agent <http://purl.org/dc/terms/>)
AnnotationAssertion(rdfs:label dcterms:Agent "Agent"@en)

# Class: dcterms:AgentClass (Agent Class)

AnnotationAssertion(rdfs:comment dcterms:AgentClass "A group of agents."@en)
AnnotationAssertion(rdfs:isDefinedBy dcterms:AgentClass <http://purl.org/dc/terms/>)
AnnotationAssertion(rdfs:label dcterms:AgentClass "Agent Class"@en)
SubClassOf(dcterms:AgentClass rdfs:Class)

# Class: dcterms:BibliographicResource (Bibliographic Resource)

AnnotationAssertion(rdfs:comment dcterms:BibliographicResource "A book, article, or other documentary resource."@en)
AnnotationAssertion(rdfs:isDefinedBy dcterms:BibliographicResource <http://purl.org/dc/terms/>)
AnnotationAssertion(rdfs:label dcterms:BibliographicResource "Bibliographic Resource"@en)

# Class: dcterms:FileFormat (File Format)

AnnotationAssertion(rdfs:comment dcterms:FileFormat "A digital resource format."@en)
AnnotationAssertion(rdfs:isDefinedBy dcterms:FileFormat <http://purl.org/dc/terms/>)
AnnotationAssertion(rdfs:label dcterms:FileFormat "File Format"@en)
SubClassOf(dcterms:FileFormat dcterms:MediaType)

# Class: dcterms:Frequency (Frequency)

AnnotationAssertion(rdfs:comment dcterms:Frequency "A rate at which something recurs."@en)
AnnotationAssertion(rdfs:isDefinedBy dcterms:Frequency <http://purl.org/dc/terms/>)
AnnotationAssertion(rdfs:label dcterms:Frequency "Frequency"@en)

# Class: dcterms:Jurisdiction (Jurisdiction)

AnnotationAssertion(rdfs:comment dcterms:Jurisdiction "The extent or range of judicial, law enforcement, or other authority."@en)
AnnotationAssertion(rdfs:isDefinedBy dcterms:Jurisdiction <http://purl.org/dc/terms/>)
AnnotationAssertion(rdfs:label dcterms:Jurisdiction "Jurisdiction"@en)
SubClassOf(dcterms:Jurisdiction dcterms:LocationPeriodOrJurisdiction)

# Class: dcterms:LicenseDocument (License Document)

AnnotationAssertion(rdfs:comment dcterms:LicenseDocument "A legal document giving official permission to do something with a resource."@en)
AnnotationAssertion(rdfs:isDefinedBy dcterms:LicenseDocument <http://purl.org/dc/terms/>)
AnnotationAssertion(rdfs:label dcterms:LicenseDocument "License Document"@en)
SubClassOf(dcterms:LicenseDocument dcterms:RightsStatement)

# Class: dcterms:LinguisticSystem (Linguistic System)

AnnotationAssertion(dcterms:description dcterms:LinguisticSystem "Written, spoken, sign, and computer languages are linguistic systems."@en)
AnnotationAssertion(rdfs:comment dcterms:LinguisticSystem "A system of signs, symbols, sounds, gestures, or rules used in communication."@en)
AnnotationAssertion(rdfs:isDefinedBy dcterms:LinguisticSystem <http://purl.org/dc/terms/>)
AnnotationAssertion(rdfs:label dcterms:LinguisticSystem "Linguistic System"@en)

# Class: dcterms:Location (Location)

AnnotationAssertion(rdfs:comment dcterms:Location "A spatial region or named place."@en)
AnnotationAssertion(rdfs:isDefinedBy dcterms:Location <http://purl.org/dc/terms/>)
AnnotationAssertion(rdfs:label dcterms:Location "Location"@en)
SubClassOf(dcterms:Location dcterms:LocationPeriodOrJurisdiction)

# Class: dcterms:LocationPeriodOrJurisdiction (Location, Period, or Jurisdiction)

AnnotationAssertion(rdfs:comment dcterms:LocationPeriodOrJurisdiction "A location, period of time, or jurisdiction."@en)
AnnotationAssertion(rdfs:isDefinedBy dcterms:LocationPeriodOrJurisdiction <http://purl.org/dc/terms/>)
AnnotationAssertion(rdfs:label dcterms:LocationPeriodOrJurisdiction "Location, Period, or Jurisdiction"@en)

# Class: dcterms:MediaType (Media Type)

AnnotationAssertion(rdfs:comment dcterms:MediaType "A file format or physical medium."@en)
AnnotationAssertion(rdfs:isDefinedBy dcterms:MediaType <http://purl.org/dc/terms/>)
AnnotationAssertion(rdfs:label dcterms:MediaType "Media Type"@en)
SubClassOf(dcterms:MediaType dcterms:MediaTypeOrExtent)

# Class: dcterms:MediaTypeOrExtent (Media Type or Extent)

AnnotationAssertion(rdfs:comment dcterms:MediaTypeOrExtent "A media type or extent."@en)
AnnotationAssertion(rdfs:isDefinedBy dcterms:MediaTypeOrExtent <http://purl.org/dc/terms/>)
AnnotationAssertion(rdfs:label dcterms:MediaTypeOrExtent "Media Type or Extent"@en)

# Class: dcterms:MethodOfAccrual (Method of Accrual)

AnnotationAssertion(rdfs:comment dcterms:MethodOfAccrual "A method by which resources are added to a collection."@en)
AnnotationAssertion(rdfs:isDefinedBy dcterms:MethodOfAccrual <http://purl.org/dc/terms/>)
AnnotationAssertion(rdfs:label dcterms:MethodOfAccrual "Method of Accrual"@en)

# Class: dcterms:MethodOfInstruction (Method of Instruction)

AnnotationAssertion(rdfs:comment dcterms:MethodOfInstruction "A process that is used to engender knowledge, attitudes, and skills."@en)
AnnotationAssertion(rdfs:isDefinedBy dcterms:MethodOfInstruction <http://purl.org/dc/terms/>)
AnnotationAssertion(rdfs:label dcterms:MethodOfInstruction "Method of Instruction"@en)

# Class: dcterms:PeriodOfTime (Period of Time)

AnnotationAssertion(rdfs:comment dcterms:PeriodOfTime "An interval of time that is named or defined by its start and end dates."@en)
AnnotationAssertion(rdfs:isDefinedBy dcterms:PeriodOfTime <http://purl.org/dc/terms/>)
AnnotationAssertion(rdfs:label dcterms:PeriodOfTime "Period of Time"@en)
SubClassOf(dcterms:PeriodOfTime dcterms:LocationPeriodOrJurisdiction)

# Class: dcterms:PhysicalMedium (Physical Medium)

AnnotationAssertion(dcterms:description dcterms:PhysicalMedium "Examples include paper, canvas, or DVD."@en)
AnnotationAssertion(rdfs:comment dcterms:PhysicalMedium "A physical material or carrier."@en)
AnnotationAssertion(rdfs:isDefinedBy dcterms:PhysicalMedium <http://purl.org/dc/terms/>)
AnnotationAssertion(rdfs:label dcterms:PhysicalMedium "Physical Medium"@en)
SubClassOf(dcterms:PhysicalMedium dcterms:MediaType)

# Class: dcterms:PhysicalResource (Physical Resource)

AnnotationAssertion(rdfs:comment dcterms:PhysicalResource "A material thing."@en)
AnnotationAssertion(rdfs:isDefinedBy dcterms:PhysicalResource <http://purl.org/dc/terms/>)
AnnotationAssertion(rdfs:label dcterms:PhysicalResource "Physical Resource"@en)

# Class: dcterms:Policy (Policy)

AnnotationAssertion(rdfs:comment dcterms:Policy "A plan or course of action by an authority, intended to influence and determine decisions, actions, and other matters."@en)
AnnotationAssertion(rdfs:isDefinedBy dcterms:Policy <http://purl.org/dc/terms/>)
AnnotationAssertion(rdfs:label dcterms:Policy "Policy"@en)

# Class: dcterms:ProvenanceStatement (Provenance Statement)

AnnotationAssertion(rdfs:comment dcterms:ProvenanceStatement "Any changes in ownership and custody of a resource since its creation that are significant for its authenticity, integrity, and interpretation."@en)
AnnotationAssertion(rdfs:isDefinedBy dcterms:ProvenanceStatement <http://purl.org/dc/terms/>)
AnnotationAssertion(rdfs:label dcterms:ProvenanceStatement "Provenance Statement"@en)

# Class: dcterms:RightsStatement (Rights Statement)

AnnotationAssertion(rdfs:comment dcterms:RightsStatement "A statement about the intellectual property rights (IPR) held in or over a resource, a legal document giving official permission to do something with a resource, or a statement about access rights."@en)
AnnotationAssertion(rdfs:isDefinedBy dcterms:RightsStatement <http://purl.org/dc/terms/>)
AnnotationAssertion(rdfs:label dcterms:RightsStatement "Rights Statement"@en)

# Class: dcterms:SizeOrDuration (Size or Duration)

AnnotationAssertion(dcterms:description dcterms:SizeOrDuration "Examples include a number of pages, a specification of length, width, and breadth, or a period in hours, minutes, and seconds."@en)
AnnotationAssertion(rdfs:comment dcterms:SizeOrDuration "A dimension or extent, or a time taken to play or execute."@en)
AnnotationAssertion(rdfs:isDefinedBy dcterms:SizeOrDuration <http://purl.org/dc/terms/>)
AnnotationAssertion(rdfs:label dcterms:SizeOrDuration "Size or Duration"@en)
SubClassOf(dcterms:SizeOrDuration dcterms:MediaTypeOrExtent)

# Class: dcterms:Standard (Standard)

AnnotationAssertion(rdfs:comment dcterms:Standard "A reference point against which other things can be evaluated or compared."@en)
AnnotationAssertion(rdfs:isDefinedBy dcterms:Standard <http://purl.org/dc/terms/>)
AnnotationAssertion(rdfs:label dcterms:Standard "Standard"@en)

# Class: dcat:Catalog (Katalog)

AnnotationAssertion(rdfs:comment dcat:Catalog "A curated collection of metadata about resources (e.g., datasets and data services in the context of a data catalog)."@en)
AnnotationAssertion(rdfs:comment dcat:Catalog "En udvalgt og arrangeret samling af metadata om ressourcer (fx datasæt og datatjenester i kontekst af et datakatalog). "@da)
AnnotationAssertion(rdfs:comment dcat:Catalog "Una colección curada de metadatos sobre recursos (por ejemplo, conjuntos de datos y servicios de datos en el contexto de un catálogo de datos)."@es)
AnnotationAssertion(rdfs:comment dcat:Catalog "Una raccolta curata di metadati sulle risorse (ad es. sui dataset e relativi servizi nel contesto di cataloghi di dati)."@it)
AnnotationAssertion(rdfs:comment dcat:Catalog "Une collection élaborée de métadonnées sur les jeux de données"@fr)
AnnotationAssertion(rdfs:comment dcat:Catalog "Řízená kolekce metadat o datových sadách a datových službách"@cs)
AnnotationAssertion(rdfs:comment dcat:Catalog "Μια επιμελημένη συλλογή μεταδεδομένων περί συνόλων δεδομένων"@el)
AnnotationAssertion(rdfs:comment dcat:Catalog "مجموعة من توصيفات قوائم البيانات"@ar)
AnnotationAssertion(rdfs:comment dcat:Catalog "データ・カタログは、データセットに関するキュレートされたメタデータの集合です。"@ja)
AnnotationAssertion(rdfs:isDefinedBy dcat:Catalog <http://www.w3.org/TR/vocab-dcat/>)
AnnotationAssertion(rdfs:label dcat:Catalog "Catalog"@en)
AnnotationAssertion(rdfs:label dcat:Catalog "Catalogo"@it)
AnnotationAssertion(rdfs:label dcat:Catalog "Catalogue"@fr)
AnnotationAssertion(rdfs:label dcat:Catalog "Catálogo"@es)
AnnotationAssertion(rdfs:label dcat:Catalog "Katalog"@cs)
AnnotationAssertion(rdfs:label dcat:Catalog "Katalog"@da)
AnnotationAssertion(rdfs:label dcat:Catalog "Κατάλογος"@el)
AnnotationAssertion(rdfs:label dcat:Catalog "فهرس قوائم البيانات"@ar)
AnnotationAssertion(rdfs:label dcat:Catalog "カタログ"@ja)
AnnotationAssertion(skos:definition dcat:Catalog "A curated collection of metadata about resources."@en)
AnnotationAssertion(skos:definition dcat:Catalog "En samling af metadata om ressourcer."@da)
AnnotationAssertion(skos:definition dcat:Catalog "Una colección curada de metadatos sobre recursos."@es)
AnnotationAssertion(skos:definition dcat:Catalog "Una raccolta curata di metadati sulle risorse."@it)
AnnotationAssertion(skos:definition dcat:Catalog "Une collection élaborée de métadonnées sur les jeux de données."@fr)
AnnotationAssertion(skos:definition dcat:Catalog "Řízená kolekce metadat o datových sadách a datových službách."@cs)
AnnotationAssertion(skos:definition dcat:Catalog "Μια επιμελημένη συλλογή μεταδεδομένων περί συνόλων δεδομένων."@el)
AnnotationAssertion(skos:definition dcat:Catalog "مجموعة من توصيفات قوائم البيانات"@ar)
AnnotationAssertion(skos:definition dcat:Catalog "データ・カタログは、データセットに関するキュレートされたメタデータの集合です。"@ja)
AnnotationAssertion(skos:editorialNote dcat:Catalog "Multilingual text not completelly updated. Translations for skos:scopeNote and definitions to doublecheck."@en)
AnnotationAssertion(skos:scopeNote dcat:Catalog "A web-based data catalog is typically represented as a single instance of this class."@en)
AnnotationAssertion(skos:scopeNote dcat:Catalog "Datasets and data services are examples of resources in the context of a data catalog."@en)
AnnotationAssertion(skos:scopeNote dcat:Catalog "Et webbaseret datakatalog repræsenteres typisk ved en enkelt instans af denne klasse."@da)
AnnotationAssertion(skos:scopeNote dcat:Catalog "Normalmente, un catalogo di dati nel web viene rappresentato come una singola istanza di questa classe."@it)
AnnotationAssertion(skos:scopeNote dcat:Catalog "Normalmente, un catálogo de datos disponible en la web se representa como una única instancia de esta clase."@es)
AnnotationAssertion(skos:scopeNote dcat:Catalog "Webový datový katalog je typicky reprezentován jako jedna instance této třídy."@cs)
AnnotationAssertion(skos:scopeNote dcat:Catalog "Συνήθως, ένας κατάλογος δεδομένων στον Παγκόσμιο Ιστό αναπαρίσταται ως ένα στιγμιότυπο αυτής της κλάσης."@el)
AnnotationAssertion(skos:scopeNote dcat:Catalog "通常、ウェブ・ベースのデータ・カタログは、このクラスの1つのインスタンスとして表わされます。"@ja)
SubClassOf(dcat:Catalog dcat:Dataset)

# Class: dcat:CatalogRecord (Record di catalogo)

AnnotationAssertion(rdfs:comment dcat:CatalogRecord "1つのデータセットを記述したデータ・カタログ内のレコード。"@ja)
AnnotationAssertion(rdfs:comment dcat:CatalogRecord "A record in a data catalog, describing the registration of a single dataset or data service."@en)
AnnotationAssertion(rdfs:comment dcat:CatalogRecord "En post i et datakatalog der beskriver registreringen af et enkelt datasæt eller en datatjeneste."@da)
AnnotationAssertion(rdfs:comment dcat:CatalogRecord "Un record in un catalogo di dati che descrive un singolo dataset o servizio di dati."@it)
AnnotationAssertion(rdfs:comment dcat:CatalogRecord "Un registre du catalogue ou une entrée du catalogue, décrivant un seul jeu de données."@fr)
AnnotationAssertion(rdfs:comment dcat:CatalogRecord "Un registro en un catálogo de datos que describe un solo conjunto de datos o un servicio de datos."@es)
AnnotationAssertion(rdfs:comment dcat:CatalogRecord "Záznam v datovém katalogu popisující jednu datovou sadu či datovou službu."@cs)
AnnotationAssertion(rdfs:comment dcat:CatalogRecord "Μία καταγραφή ενός καταλόγου, η οποία περιγράφει ένα συγκεκριμένο σύνολο δεδομένων."@el)
AnnotationAssertion(rdfs:isDefinedBy dcat:CatalogRecord <http://www.w3.org/TR/vocab-dcat/>)
AnnotationAssertion(rdfs:label dcat:CatalogRecord "Catalog Record"@en)
AnnotationAssertion(rdfs:label dcat:CatalogRecord "Katalogizační záznam"@cs)
AnnotationAssertion(rdfs:label dcat:CatalogRecord "Katalogpost"@da)
AnnotationAssertion(rdfs:label dcat:CatalogRecord "Record di catalogo"@it)
AnnotationAssertion(rdfs:label dcat:CatalogRecord "Registre du catalogue"@fr)
AnnotationAssertion(rdfs:label dcat:CatalogRecord "Registro del catálogo"@es)
AnnotationAssertion(rdfs:label dcat:CatalogRecord "Καταγραφή καταλόγου"@el)
AnnotationAssertion(rdfs:label dcat:CatalogRecord "سجل"@ar)
AnnotationAssertion(rdfs:label dcat:CatalogRecord "カタログ・レコード"@ja)
AnnotationAssertion(skos:definition dcat:CatalogRecord "1つのデータセットを記述したデータ・カタログ内のレコード。"@ja)
AnnotationAssertion(skos:definition dcat:CatalogRecord "A record in a data catalog, describing the registration of a single dataset or data service."@en)
AnnotationAssertion(skos:definition dcat:CatalogRecord "En post i et datakatalog der beskriver registreringen af et enkelt datasæt eller en datatjeneste."@da)
AnnotationAssertion(skos:definition dcat:CatalogRecord "Un record in un catalogo di dati che descrive un singolo dataset o servizio di dati."@it)
AnnotationAssertion(skos:definition dcat:CatalogRecord "Un registre du catalogue ou une entrée du catalogue, décrivant un seul jeu de données."@fr)
AnnotationAssertion(skos:definition dcat:CatalogRecord "Un registro en un catálogo de datos que describe un solo conjunto de datos o un servicio de datos."@es)
AnnotationAssertion(skos:definition dcat:CatalogRecord "Záznam v datovém katalogu popisující jednu datovou sadu či datovou službu."@cs)
AnnotationAssertion(skos:definition dcat:CatalogRecord "Μία καταγραφή ενός καταλόγου, η οποία περιγράφει ένα συγκεκριμένο σύνολο δεδομένων."@el)
AnnotationAssertion(skos:editorialNote dcat:CatalogRecord "English definition updated in this revision. Multilingual text not yet updated except the Spanish one and the Czech one and Italian one."@en)
AnnotationAssertion(skos:scopeNote dcat:CatalogRecord "C'est une classe facultative et tous les catalogues ne l'utiliseront pas. Cette classe existe pour les catalogues	ayant une distinction entre les métadonnées sur le jeu de données et les métadonnées sur une entrée du jeu de données dans le catalogue."@fr)
AnnotationAssertion(skos:scopeNote dcat:CatalogRecord "Denne klasse er valgfri og ikke alle kataloger vil anvende denne klasse. Den kan anvendes i de kataloger hvor der skelnes mellem metadata om datasættet eller datatjenesten og metadata om selve posten til registreringen af datasættet eller datatjenesten i kataloget. Udgivelsesdatoen for datasættet afspejler for eksempel den dato hvor informationerne oprindeligt blev gjort tilgængelige af udgiveren, hvorimod udgivelsesdatoen for katalogposten er den dato hvor datasættet blev føjet til kataloget. I de tilfælde hvor de to datoer er forskellige eller hvor blot sidstnævnte er kendt, bør udgivelsesdatoen kun angives for katalogposten. Bemærk at W3Cs PROV ontologi gør til muligt at tilføje yderligere proveniensoplysninger eksempelvis om processen eller aktøren involveret i en given ændring af datasættet."@da)
AnnotationAssertion(skos:scopeNote dcat:CatalogRecord "Esta clase es opcional y no todos los catálogos la utilizarán. Esta clase existe para catálogos que hacen una distinción entre los metadatos acerca de un conjunto de datos o un servicio de datos y los metadatos acerca de una entrada en ese conjunto de datos en el catálogo. Por ejemplo, la propiedad sobre la fecha de la publicación de los datos refleja la fecha en que la información fue originalmente publicada, mientras que la fecha de publicación del registro del catálogo es la fecha en que los datos se agregaron al mismo. En caso en que ambas fechas fueran diferentes, o en que sólo la fecha de publicación del registro del catálogo estuviera disponible, sólo debe especificarse en el registro del catálogo. Tengan en cuenta que la ontología PROV de W3C permite describir otra información sobre la proveniencia de los datos, como por ejemplo detalles del proceso y de los agentes involucrados en algún cambio específico a los datos."@es)
AnnotationAssertion(skos:scopeNote dcat:CatalogRecord "Questa classe è opzionale e non tutti i cataloghi la utilizzeranno. Esiste per cataloghi in cui si opera una distinzione tra i metadati relativi al dataset ed i metadati relativi alla gestione del dataset nel catalogo. Ad esempio, la  proprietà per indicare la data di pubblicazione del dataset rifletterà la data in cui l'informazione è stata originariamente messa a disposizione dalla casa editrice, mentre la data di pubblicazione per il record nel catalogo rifletterà la data in cui il dataset è stato aggiunto al catalogo. Nei casi dove solo quest'ultima sia nota, si utilizzerà esclusivamente la data di  pubblicazione relativa al record del catalogo. Si noti che l'Ontologia W3C PROV permette di descrivere ulteriori informazioni sulla provenienza, quali i dettagli del processo, la procedura e l'agente coinvolto in una particolare modifica di un dataset."@it)
AnnotationAssertion(skos:scopeNote dcat:CatalogRecord "Tato třída je volitelná a ne všechny katalogy ji využijí. Existuje pro katalogy, ve kterých se rozlišují metadata datové sady či datové služby a metadata o záznamu o datové sadě či datové službě v katalogu. Například datum publikace datové sady odráží datum, kdy byla datová sada původně zveřejněna poskytovatelem dat, zatímco datum publikace katalogizačního záznamu je datum zanesení datové sady do katalogu. V případech kdy se obě data liší, nebo je známo jen to druhé, by mělo být specifikováno jen datum publikace katalogizačního záznamu. Všimněte si, že ontologie W3C PROV umožňuje popsat další informace o původu jako například podrobnosti o procesu konkrétní změny datové sady a jeho účastnících."@cs)
AnnotationAssertion(skos:scopeNote dcat:CatalogRecord "This class is optional and not all catalogs will use it. It exists for catalogs where a distinction is made between metadata about a dataset or data service and metadata about the entry for the dataset or data service in the catalog. For example, the publication date property of the dataset reflects the date when the information was originally made available by the publishing agency, while the publication date of the catalog record is the date when the dataset was added to the catalog. In cases where both dates differ, or where only the latter is known, the publication date should only be specified for the catalog record. Notice that the W3C PROV Ontology allows describing further provenance information such as the details of the process and the agent involved in a particular change to a dataset."@en)
AnnotationAssertion(skos:scopeNote dcat:CatalogRecord "Αυτή η κλάση είναι προαιρετική και δεν χρησιμοποιείται από όλους τους καταλόγους. Υπάρχει για τις περιπτώσεις καταλόγων όπου γίνεται διαχωρισμός μεταξύ των μεταδεδομένων για το σύνολο των δεδομένων και των μεταδεδομένων για την καταγραφή του συνόλου δεδομένων εντός του καταλόγου. Για παράδειγμα, η ιδιότητα της ημερομηνίας δημοσίευσης του συνόλου δεδομένων δείχνει την ημερομηνία κατά την οποία οι πληροφορίες έγιναν διαθέσιμες από τον φορέα δημοσίευσης, ενώ η ημερομηνία δημοσίευσης της καταγραφής του καταλόγου δείχνει την ημερομηνία που το σύνολο δεδομένων προστέθηκε στον κατάλογο. Σε περιπτώσεις που οι δύο ημερομηνίες διαφέρουν, ή που μόνο η τελευταία είναι γνωστή, η ημερομηνία δημοσίευσης θα πρέπει να δίνεται για την καταγραφή του καταλόγου. Να σημειωθεί πως η οντολογία W3C PROV επιτρέπει την περιγραφή επιπλέον πληροφοριών ιστορικού όπως λεπτομέρειες για τη διαδικασία και τον δράστη που εμπλέκονται σε μία συγκεκριμένη αλλαγή εντός του συνόλου δεδομένων."@el)
AnnotationAssertion(skos:scopeNote dcat:CatalogRecord "このクラスはオプションで、すべてのカタログがそれを用いるとは限りません。これは、データセットに関するメタデータとカタログ内のデータセットのエントリーに関するメタデータとで区別が行われるカタログのために存在しています。例えば、データセットの公開日プロパティーは、公開機関が情報を最初に利用可能とした日付を示しますが、カタログ・レコードの公開日は、データセットがカタログに追加された日付です。両方の日付が異っていたり、後者だけが分かっている場合は、カタログ・レコードに対してのみ公開日を指定すべきです。W3CのPROVオントロジー[prov-o]を用いれば、データセットに対する特定の変更に関連するプロセスやエージェントの詳細などの、さらに詳しい来歴情報の記述が可能となることに注意してください。"@ja)
SubClassOf(dcat:CatalogRecord ObjectAllValuesFrom(foaf:primaryTopic dcat:Resource))
SubClassOf(dcat:CatalogRecord ObjectExactCardinality(1 foaf:primaryTopic))

# Class: dcat:DataService (Servicio de datos)

AnnotationAssertion(rdfs:comment dcat:DataService "A site or end-point providing operations related to the discovery of, access to, or processing functions on, data or related resources."@en)
AnnotationAssertion(rdfs:comment dcat:DataService "Et websted eller endpoint der udstiller operationer relateret til opdagelse af, adgang til eller behandlende funktioner på data eller relaterede ressourcer."@da)
AnnotationAssertion(rdfs:comment dcat:DataService "Umístění či přístupový bod poskytující operace související s hledáním, přistupem k, či výkonem funkcí na datech či souvisejících zdrojích."@cs)
AnnotationAssertion(rdfs:comment dcat:DataService "Un sitio o end-point que provee operaciones relacionadas a funciones de descubrimiento, acceso, o procesamiento de datos o recursos relacionados."@es)
AnnotationAssertion(rdfs:comment dcat:DataService "Un sito o end-point che fornisce operazioni relative alla scoperta, all'accesso o all'elaborazione di funzioni su dati o risorse correlate."@it)
AnnotationAssertion(rdfs:label dcat:DataService "Data service"@en)
AnnotationAssertion(rdfs:label dcat:DataService "Datatjeneste"@da)
AnnotationAssertion(rdfs:label dcat:DataService "Servicio de datos"@es)
AnnotationAssertion(rdfs:label dcat:DataService "Servizio di dati"@it)
AnnotationAssertion(skos:altLabel dcat:DataService "Dataservice"@da)
AnnotationAssertion(skos:changeNote dcat:DataService "New class added in DCAT 2."@en)
AnnotationAssertion(skos:changeNote dcat:DataService "Nová třída přidaná ve verzi DCAT 2."@cs)
AnnotationAssertion(skos:changeNote dcat:DataService "Nueva clase añadida en DCAT 2."@es)
AnnotationAssertion(skos:changeNote dcat:DataService "Nuova classe aggiunta in DCAT 2."@it)
AnnotationAssertion(skos:changeNote dcat:DataService "Ny klasse tilføjet i DCAT 2."@da)
AnnotationAssertion(skos:definition dcat:DataService "A site or end-point providing operations related to the discovery of, access to, or processing functions on, data or related resources."@en)
AnnotationAssertion(skos:definition dcat:DataService "Et site eller endpoint der udstiller operationer relateret til opdagelse af, adgang til eller behandlende funktioner på data eller relaterede ressourcer."@da)
AnnotationAssertion(skos:definition dcat:DataService "Umístění či přístupový bod poskytující operace související s hledáním, přistupem k, či výkonem funkcí na datech či souvisejících zdrojích."@cs)
AnnotationAssertion(skos:definition dcat:DataService "Un sitio o end-point que provee operaciones relacionadas a funciones de descubrimiento, acceso, o procesamiento de datos o recursos relacionados."@es)
AnnotationAssertion(skos:definition dcat:DataService "Un sito o end-point che fornisce operazioni relative alla scoperta, all'accesso o all'elaborazione di funzioni su dati o risorse correlate."@it)
AnnotationAssertion(skos:scopeNote dcat:DataService "Datatjenestetypen kan indikeres ved hjælp af egenskaben dcterms:type. Værdien kan tages fra kontrollerede udfaldsrum såsom INSPIRE spatial data service vocabulary."@da)
AnnotationAssertion(skos:scopeNote dcat:DataService "Druh služby může být indikován vlastností dcterms:type. Její hodnota může být z řízeného slovníku, kterým je například slovník typů prostorových datových služeb INSPIRE."@cs)
AnnotationAssertion(skos:scopeNote dcat:DataService "El tipo de servicio puede indicarse usando la propiedad dcterms:type. Su valor puede provenir de un vocabulario controlado, como por ejemplo el vocabulario de servicios de datos espaciales de INSPIRE."@es)
AnnotationAssertion(skos:scopeNote dcat:DataService "Hvis en dcat:DataService er bundet til en eller flere specifikke datasæt kan dette indikeres ved hjælp af egenskaben dcat:servesDataset. "@da)
AnnotationAssertion(skos:scopeNote dcat:DataService "If a dcat:DataService is bound to one or more specified Datasets, they are indicated by the dcat:servesDataset property."@en)
AnnotationAssertion(skos:scopeNote dcat:DataService "Il tipo di servizio può essere indicato usando la proprietà dcterms:type. Il suo valore può essere preso da un vocabolario controllato come il vocabolario dei tipi di servizi per dati spaziali di INSPIRE."@it)
AnnotationAssertion(skos:scopeNote dcat:DataService "Pokud je dcat:DataService navázána na jednu či více Datových sad, jsou tyto indikovány vlstností dcat:servesDataset."@cs)
AnnotationAssertion(skos:scopeNote dcat:DataService "Se un dcat:DataService è associato a uno o più Dataset specificati, questi sono indicati dalla proprietà dcat:serveDataset."@it)
AnnotationAssertion(skos:scopeNote dcat:DataService "Si un dcat:DataService está asociado con uno o más conjuntos de datos especificados, dichos conjuntos de datos pueden indicarse con la propiedad dcat:servesDataset."@es)
AnnotationAssertion(skos:scopeNote dcat:DataService "The kind of service can be indicated using the dcterms:type property. Its value may be taken from a controlled vocabulary such as the INSPIRE spatial data service type vocabulary."@en)
SubClassOf(dcat:DataService dctype:Service)
SubClassOf(dcat:DataService dcat:Resource)

# Class: dcat:Dataset (データセット)

AnnotationAssertion(rdfs:comment dcat:Dataset "1つのエージェントによって公開またはキュレートされ、1つ以上の形式でアクセスまたはダウンロードできるデータの集合。"@ja)
AnnotationAssertion(rdfs:comment dcat:Dataset "A collection of data, published or curated by a single source, and available for access or download in one or more representations."@en)
AnnotationAssertion(rdfs:comment dcat:Dataset "En samling af data, udgivet eller udvalgt og arrangeret af en enkelt kilde og som er til råde for adgang til eller download af i en eller flere repræsentationer."@da)
AnnotationAssertion(rdfs:comment dcat:Dataset "Kolekce dat poskytovaná či řízená jedním zdrojem, která je k dispozici pro přístup či stažení v jednom či více formátech."@cs)
AnnotationAssertion(rdfs:comment dcat:Dataset "Raccolta di dati, pubblicati o curati da un'unica fonte, disponibili per l'accesso o il download in uno o più formati."@it)
AnnotationAssertion(rdfs:comment dcat:Dataset "Una colección de datos, publicados o conservados por una única fuente, y disponibles para ser accedidos o descargados en uno o más formatos."@es)
AnnotationAssertion(rdfs:comment dcat:Dataset "Une collection de données, publiée ou élaborée par une seule source, et disponible pour accès ou téléchargement dans un ou plusieurs formats."@fr)
AnnotationAssertion(rdfs:comment dcat:Dataset "Μία συλλογή από δεδομένα, δημοσιευμένη ή επιμελημένη από μία και μόνο πηγή, διαθέσιμη δε προς πρόσβαση ή μεταφόρτωση σε μία ή περισσότερες μορφές."@el)
AnnotationAssertion(rdfs:comment dcat:Dataset "قائمة بيانات منشورة أو مجموعة من قبل مصدر ما و متاح الوصول إليها أو تحميلها"@ar)
AnnotationAssertion(rdfs:isDefinedBy dcat:Dataset <http://www.w3.org/TR/vocab-dcat/>)
AnnotationAssertion(rdfs:label dcat:Dataset "Conjunto de datos"@es)
AnnotationAssertion(rdfs:label dcat:Dataset "Dataset"@en)
AnnotationAssertion(rdfs:label dcat:Dataset "Dataset"@it)
AnnotationAssertion(rdfs:label dcat:Dataset "Datasæt"@da)
AnnotationAssertion(rdfs:label dcat:Dataset "Datová sada"@cs)
AnnotationAssertion(rdfs:label dcat:Dataset "Jeu de données"@fr)
AnnotationAssertion(rdfs:label dcat:Dataset "Σύνολο Δεδομένων"@el)
AnnotationAssertion(rdfs:label dcat:Dataset "قائمة بيانات"@ar)
AnnotationAssertion(rdfs:label dcat:Dataset "データセット"@ja)
AnnotationAssertion(skos:altLabel dcat:Dataset "Datasamling"@da)
AnnotationAssertion(skos:changeNote dcat:Dataset "2018-02 - odstraněno tvrzení o podtřídě dctype:Dataset, jelikož rozsah dcat:Dataset zahrnuje několik dalších typů ze slovníku dctype."@cs)
AnnotationAssertion(skos:changeNote dcat:Dataset "2018-02 - se eliminó el axioma de subclase con dctype:Dataset porque el alcance de dcat:Dataset incluye muchos otros tipos del vocabulario dctype."@es)
AnnotationAssertion(skos:changeNote dcat:Dataset "2018-02 - sottoclasse di dctype:Dataset rimosso perché l'ambito di dcat:Dataset include diversi altri tipi dal vocabolario dctype."@it)
AnnotationAssertion(skos:changeNote dcat:Dataset "2018-02 - subclass of dctype:Dataset removed because scope of dcat:Dataset includes several other types from the dctype vocabulary."@en)
AnnotationAssertion(skos:changeNote dcat:Dataset "2018-02 - subklasse af dctype:Dataset fjernet da scope af dcat:Dataset omfatter flere forskellige typer fra dctype-vokabularet."@da)
AnnotationAssertion(skos:definition dcat:Dataset "1つのエージェントによって公開またはキュレートされ、1つ以上の形式でアクセスまたはダウンロードできるデータの集合。"@ja)
AnnotationAssertion(skos:definition dcat:Dataset "A collection of data, published or curated by a single source, and available for access or download in one or more representations."@en)
AnnotationAssertion(skos:definition dcat:Dataset "En samling a data, udgivet eller udvalgt og arrangeret af en enkelt kilde og som der er adgang til i en eller flere repræsentationer."@da)
AnnotationAssertion(skos:definition dcat:Dataset "Kolekce dat poskytovaná či řízená jedním zdrojem, která je k dispozici pro přístup či stažení v jednom či více formátech."@cs)
AnnotationAssertion(skos:definition dcat:Dataset "Raccolta di dati, pubblicati o curati da un'unica fonte, disponibili per l'accesso o il download in uno o più formati."@it)
AnnotationAssertion(skos:definition dcat:Dataset "Una colección de datos, publicados o conservados por una única fuente, y disponibles para ser accedidos o descargados en uno o más formatos."@es)
AnnotationAssertion(skos:definition dcat:Dataset "Une collection de données, publiée ou élaborée par une seule source, et disponible pour accès ou téléchargement dans un ou plusieurs formats."@fr)
AnnotationAssertion(skos:definition dcat:Dataset "Μία συλλογή από δεδομένα, δημοσιευμένη ή επιμελημένη από μία και μόνο πηγή, διαθέσιμη δε προς πρόσβαση ή μεταφόρτωση σε μία ή περισσότερες μορφές."@el)
AnnotationAssertion(skos:definition dcat:Dataset "قائمة بيانات منشورة أو مجموعة من قبل مصدر ما و متاح الوصول إليها أو تحميلها"@ar)
AnnotationAssertion(skos:editorialNote dcat:Dataset "2020-03-16 A new scopenote added and need to be translated"@en)
AnnotationAssertion(skos:scopeNote dcat:Dataset "Cette classe représente le jeu de données publié par le fournisseur de données. Dans les cas où une distinction est nécessaire entre le jeu de donénes et son entrée dans le catalogue, la classe registre de données peut être utilisée pour ce dernier."@fr)
AnnotationAssertion(skos:scopeNote dcat:Dataset "Denne klasse beskriver det konceptuelle datasæt. En eller flere repræsentationer kan være tilgængelige med forskellige skematiske opsætninger, formater eller serialiseringer."@da)
AnnotationAssertion(skos:scopeNote dcat:Dataset "Denne klasse repræsenterer det konkrete datasæt som det udgives af datasætleverandøren. I de tilfælde hvor det er nødvendigt at skelne mellem det konkrete datasæt og dets registrering i kataloget (fordi metadata såsom ændringsdato og vedligeholder er forskellige), så kan klassen katalogpost anvendes. "@da)
AnnotationAssertion(skos:scopeNote dcat:Dataset "Esta clase representa el conjunto de datos publicados. En los casos donde es necesario distinguir entre el conjunto de datos y su entrada en el catálogo de datos, se debe utilizar la clase 'registro del catálogo'."@es)
AnnotationAssertion(skos:scopeNote dcat:Dataset "Questa classe descrive il dataset dal punto di vista concettuale. Possono essere disponibili una o più rappresentazioni, con diversi layout e formati schematici o serializzazioni."@it)
AnnotationAssertion(skos:scopeNote dcat:Dataset "Questa classe rappresenta il dataset come pubblicato dall’editore. Nel caso in cui sia necessario operare  una distinzione fra i metadati originali del dataset e il record dei metadati ad esso associato nel catalogo (ad esempio, per distinguere la data di modifica del dataset da quella del dataset nel catalogo) si può impiegare la classe catalog record."@it)
AnnotationAssertion(skos:scopeNote dcat:Dataset "Tato třída reprezentuje datovou sadu tak, jak je publikována poskytovatelem dat. V případě potřeby rozlišení datové sady a jejího katalogizačního záznamu (jelikož metadata jako datum modifikace se mohou lišit) pro něj může být použita třída \"katalogizační záznam\"."@cs)
AnnotationAssertion(skos:scopeNote dcat:Dataset "The notion of dataset in DCAT is broad and inclusive, with the intention of accommodating resource types arising from all communities. Data comes in many forms including numbers, text, pixels, imagery, sound and other multi-media, and potentially other types, any of which might be collected into a dataset."@en)
AnnotationAssertion(skos:scopeNote dcat:Dataset "This class describes the conceptual dataset. One or more representations might be available, with differing schematic layouts and formats or serializations."@en)
AnnotationAssertion(skos:scopeNote dcat:Dataset "This class represents the actual dataset as published by the dataset provider. In cases where a distinction between the actual dataset and its entry in the catalog is necessary (because metadata such as modification date and maintainer might differ), the catalog record class can be used for the latter."@en)
AnnotationAssertion(skos:scopeNote dcat:Dataset "Η κλάση αυτή αναπαριστά το σύνολο δεδομένων αυτό καθ'εαυτό, όπως έχει δημοσιευθεί από τον εκδότη. Σε περιπτώσεις όπου είναι απαραίτητος ο διαχωρισμός μεταξύ του συνόλου δεδομένων και της καταγραφής αυτού στον κατάλογο (γιατί μεταδεδομένα όπως η ημερομηνία αλλαγής και ο συντηρητής μπορεί να διαφέρουν) η κλάση της καταγραφής καταλόγου μπορεί να χρησιμοποιηθεί για το τελευταίο."@el)
AnnotationAssertion(skos:scopeNote dcat:Dataset "このクラスは、データセットの公開者が公開する実際のデータセットを表わします。カタログ内の実際のデータセットとそのエントリーとの区別が必要な場合（修正日と維持者などのメタデータが異なるかもしれないので）は、後者にcatalog recordというクラスを使用できます。"@ja)
SubClassOf(dcat:Dataset dcat:Resource)

# Class: dcat:DatasetSeries (Serie de conjuntos de datos)

AnnotationAssertion(rdfs:comment dcat:DatasetSeries "A collection of datasets that are published separately, but share some characteristics that group them."@en)
AnnotationAssertion(rdfs:comment dcat:DatasetSeries "Una colección de conjuntos de datos publicados por separado, pero que comparten características que los agrupan."@es)
AnnotationAssertion(rdfs:comment dcat:DatasetSeries "Una collezione di dataset che sono pubblicati separatamente, ma che condividono caratteristiche che li rendono parte di uno stesso gruppo."@it)
AnnotationAssertion(rdfs:isDefinedBy dcat:DatasetSeries <https://www.w3.org/TR/vocab-dcat-3/>)
AnnotationAssertion(rdfs:label dcat:DatasetSeries "Dataset series"@en)
AnnotationAssertion(rdfs:label dcat:DatasetSeries "Serie de conjuntos de datos"@es)
AnnotationAssertion(rdfs:label dcat:DatasetSeries "Serie di dataset"@it)
AnnotationAssertion(skos:changeNote dcat:DatasetSeries "New class added in DCAT 3."@en)
AnnotationAssertion(skos:changeNote dcat:DatasetSeries "Nová třída přidaná ve verzi DCAT 3"@cs)
AnnotationAssertion(skos:changeNote dcat:DatasetSeries "Nueva clase agregada en DCAT 3."@es)
AnnotationAssertion(skos:changeNote dcat:DatasetSeries "Nuova classe aggiunta in DCAT 3"@it)
AnnotationAssertion(skos:changeNote dcat:DatasetSeries "Ny klasse tilføjet i DCAT 3"@da)
AnnotationAssertion(skos:definition dcat:DatasetSeries "A collection of datasets that are published separately, but share some common characteristics that groups them."@en)
AnnotationAssertion(skos:definition dcat:DatasetSeries "Una colección de conjuntos de datos publicados por separado, pero que comparten características comunes que los agrupan."@es)
AnnotationAssertion(skos:definition dcat:DatasetSeries "Una collezione di dataset che sono pubblicati separatamente, ma che condividono caratteristiche che li rendono parte di uno stesso gruppo."@it)
AnnotationAssertion(skos:editorialNote dcat:DatasetSeries "2022-05-08 Added to ttl file with annotations in English, Spanish and Italian, except notes that are in other languages too."@en)
AnnotationAssertion(skos:scopeNote dcat:DatasetSeries "Algunos escenarios comunes para series de conjuntos de datos son: series temporales compuestas de subconjuntos de datos publicados periódicamente; series de mapas compuestos de elementos del mismo tipo o tema pero con distintas huellas espaciales."@es)
AnnotationAssertion(skos:scopeNote dcat:DatasetSeries "Common scenarios for dataset series include: time series composed of periodically released subsets; map-series composed of items of the same type or theme but with differing spatial footprints."@en)
AnnotationAssertion(skos:scopeNote dcat:DatasetSeries "Dataset series can be also soft-typed via property dcterms:type as in the approach used in [GeoDCAT-AP], and adopted in [DCAT-AP-IT] and [GeoDCAT-AP-IT])."@en)
AnnotationAssertion(skos:scopeNote dcat:DatasetSeries "Le serie di dati possono anche essere denotate come tali usando la proprietà dcterms:type, secondo l'approccio usato in [GeoDCAT-AP], e adottato in [DCAT-AP-IT] e [GeoDCAT-AP-IT])."@it)
AnnotationAssertion(skos:scopeNote dcat:DatasetSeries "Scenari tipici per l'uso di serie di dataset: serie temporali costituite di dataset pubblicati regolarmente; serie di mappe costituite da elementi dello stesso tipo o tematica ma relative a differenti aree geografiche."@it)
AnnotationAssertion(skos:scopeNote dcat:DatasetSeries "También puede asignarse un tipo a las series de datos usando la propiedad dcterms:type como se hace en [GeoDCAT-AP], y adoptado en [DCAT-AP-IT] y [GeoDCAT-AP-IT])."@es)
SubClassOf(dcat:DatasetSeries dcat:Dataset)

# Class: dcat:Distribution (Distribution)

AnnotationAssertion(rdfs:comment dcat:Distribution "A specific representation of a dataset. A dataset might be available in multiple serializations that may differ in various ways, including natural language, media-type or format, schematic organization, temporal and spatial resolution, level of detail or profiles (which might specify any or all of the above)."@en)
AnnotationAssertion(rdfs:comment dcat:Distribution "En specifik repræsentation af et datasæt. Et datasæt kan være tilgængelig i mange serialiseringer der kan variere på forskellige vis, herunder sprog, medietype eller format, systemorganisering, tidslig- og geografisk opløsning, detaljeringsniveau eller profiler (der kan specificere en eller flere af ovenstående)."@da)
AnnotationAssertion(rdfs:comment dcat:Distribution "Konkrétní reprezentace datové sady. Datová sada může být dostupná v různých serializacích, které se mohou navzájem lišit různými způsoby, mimo jiné přirozeným jazykem, media-typem či formátem, schematickou organizací, časovým a prostorovým rozlišením, úrovní detailu či profily (které mohou specifikovat některé či všechny tyto rozdíly)."@cs)
AnnotationAssertion(rdfs:comment dcat:Distribution "Rappresenta una forma disponibile e specifica del dataset. Ciascun dataset può essere disponibile in forme differenti, che possono rappresentare formati diversi o diversi punti di accesso per un dataset. Esempi di distribuzioni sono un file CSV scaricabile, una API o un RSS feed."@it)
AnnotationAssertion(rdfs:comment dcat:Distribution "Représente une forme spécifique d'un jeu de données. Caque jeu de données peut être disponible sous différentes formes, celles-ci pouvant représenter différents formats du jeu de données ou différents endpoint. Des exemples de distribution sont des fichirs CSV, des API ou des flux RSS."@fr)
AnnotationAssertion(rdfs:comment dcat:Distribution "Una representación específica de los datos. Cada conjunto de datos puede estar disponible en formas diferentes, las cuáles pueden variar en distintas formas, incluyendo el idioma, 'media-type' o formato, organización esquemática, resolución temporal y espacial, nivel de detalle o perfiles (que pueden especificar cualquiera o todas las diferencias anteriores)."@es)
AnnotationAssertion(rdfs:comment dcat:Distribution "Αναπαριστά μία συγκεκριμένη διαθέσιμη μορφή ενός συνόλου δεδομένων. Κάθε σύνολο δεδομενων μπορεί να είναι διαθέσιμο σε διαφορετικές μορφές, οι μορφές αυτές μπορεί να αναπαριστούν διαφορετικές μορφές αρχείων ή διαφορετικά σημεία διάθεσης. Παραδείγματα διανομών συμπεριλαμβάνουν ένα μεταφορτώσιμο αρχείο μορφής CSV, ένα API ή ένα RSS feed."@el)
AnnotationAssertion(rdfs:comment dcat:Distribution "شكل محدد لقائمة البيانات يمكن الوصول إليه. قائمة بيانات ما يمكن أن تكون متاحه باشكال و أنواع متعددة.  ملف يمكن تحميله أو واجهة برمجية يمكن من خلالها الوصول إلى البيانات هي أمثلة على ذلك."@ar)
AnnotationAssertion(rdfs:comment dcat:Distribution "データセットの特定の利用可能な形式を表わします。各データセットは、異なる形式で利用できることがあり、これらの形式は、データセットの異なる形式や、異なるエンドポイントを表わす可能性があります。配信の例には、ダウンロード可能なCSVファイル、API、RSSフィードが含まれます。"@ja)
AnnotationAssertion(rdfs:isDefinedBy dcat:Distribution <http://www.w3.org/TR/vocab-dcat/>)
AnnotationAssertion(rdfs:label dcat:Distribution "Distribuce"@cs)
AnnotationAssertion(rdfs:label dcat:Distribution "Distribución"@es)
AnnotationAssertion(rdfs:label dcat:Distribution "Distribution"@da)
AnnotationAssertion(rdfs:label dcat:Distribution "Distribution"@en)
AnnotationAssertion(rdfs:label dcat:Distribution "Distribution"@fr)
AnnotationAssertion(rdfs:label dcat:Distribution "Distribuzione"@it)
AnnotationAssertion(rdfs:label dcat:Distribution "Διανομή"@el)
AnnotationAssertion(rdfs:label dcat:Distribution "التوزيع"@ar)
AnnotationAssertion(rdfs:label dcat:Distribution "配信"@ja)
AnnotationAssertion(skos:altLabel dcat:Distribution "Datadistribution"@da)
AnnotationAssertion(skos:altLabel dcat:Distribution "Datamanifestation"@da)
AnnotationAssertion(skos:altLabel dcat:Distribution "Datarepræsentation"@da)
AnnotationAssertion(skos:altLabel dcat:Distribution "Dataudstilling"@da)
AnnotationAssertion(skos:definition dcat:Distribution "A specific representation of a dataset. A dataset might be available in multiple serializations that may differ in various ways, including natural language, media-type or format, schematic organization, temporal and spatial resolution, level of detail or profiles (which might specify any or all of the above)."@en)
AnnotationAssertion(skos:definition dcat:Distribution "En specifik repræsentation af et datasæt. Et datasæt kan være tilgængelig i mange serialiseringer der kan variere på forskellige vis, herunder sprog, medietype eller format, systemorganisering, tidslig- og geografisk opløsning, detaljeringsniveau eller profiler (der kan specificere en eller flere af ovenstående)."@da)
AnnotationAssertion(skos:definition dcat:Distribution "Konkrétní reprezentace datové sady. Datová sada může být dostupná v různých serializacích, které se mohou navzájem lišit různými způsoby, mimo jiné přirozeným jazykem, media-typem či formátem, schematickou organizací, časovým a prostorovým rozlišením, úrovní detailu či profily (které mohou specifikovat některé či všechny tyto rozdíly)."@cs)
AnnotationAssertion(skos:definition dcat:Distribution "Rappresenta una forma disponibile e specifica del dataset. Ciascun dataset può essere disponibile in forme differenti, che possono rappresentare formati diversi o diversi punti di accesso per un dataset. Esempi di distribuzioni sono un file CSV scaricabile, una API o un RSS feed."@it)
AnnotationAssertion(skos:definition dcat:Distribution "Représente une forme spécifique d'un jeu de données. Caque jeu de données peut être disponible sous différentes formes, celles-ci pouvant représenter différents formats du jeu de données ou différents endpoint. Des exemples de distribution sont des fichirs CSV, des API ou des flux RSS."@fr)
AnnotationAssertion(skos:definition dcat:Distribution "Una representación específica de los datos. Cada conjunto de datos puede estar disponible en formas diferentes, las cuáles pueden variar en distintas formas, incluyendo el idioma, 'media-type' o formato, organización esquemática, resolución temporal y espacial, nivel de detalle o perfiles (que pueden especificar cualquiera o todas las diferencias anteriores)."@es)
AnnotationAssertion(skos:definition dcat:Distribution "Αναπαριστά μία συγκεκριμένη διαθέσιμη μορφή ενός συνόλου δεδομένων. Κάθε σύνολο δεδομενων μπορεί να είναι διαθέσιμο σε διαφορετικές μορφές, οι μορφές αυτές μπορεί να αναπαριστούν διαφορετικές μορφές αρχείων ή διαφορετικά σημεία διάθεσης. Παραδείγματα διανομών συμπεριλαμβάνουν ένα μεταφορτώσιμο αρχείο μορφής CSV, ένα API ή ένα RSS feed."@el)
AnnotationAssertion(skos:definition dcat:Distribution "شكل محدد لقائمة البيانات يمكن الوصول إليه. قائمة بيانات ما يمكن أن تكون متاحه باشكال و أنواع متعددة.  ملف يمكن تحميله أو واجهة برمجية يمكن من خلالها الوصول إلى البيانات هي أمثلة على ذلك."@ar)
AnnotationAssertion(skos:definition dcat:Distribution "データセットの特定の利用可能な形式を表わします。各データセットは、異なる形式で利用できることがあり、これらの形式は、データセットの異なる形式や、異なるエンドポイントを表わす可能性があります。配信の例には、ダウンロード可能なCSVファイル、API、RSSフィードが含まれます。"@ja)
AnnotationAssertion(skos:scopeNote dcat:Distribution "Ceci représente une disponibilité générale du jeu de données, et implique qu'il n'existe pas d'information sur la méthode d'accès réelle des données, par exple, si c'est un lien de téléchargement direct ou à travers une page Web."@fr)
AnnotationAssertion(skos:scopeNote dcat:Distribution "Denne klasse repræsenterer datasættets overordnede tilgængelighed og giver ikke oplysninger om hvilken metode der kan anvendes til at få adgang til data, dvs. om adgang til datasættet realiseres ved direkte download, API eller via et websted. Anvendelsen af egenskaben dcat:downloadURL indikerer at distributionen kan downloades direkte."@da)
AnnotationAssertion(skos:scopeNote dcat:Distribution "Esta clase representa una disponibilidad general de un conjunto de datos, e implica que no existe información acerca del método de acceso real a los datos, i.e., si es un enlace de descarga directa o a través de una página Web."@es)
AnnotationAssertion(skos:scopeNote dcat:Distribution "Questa classe rappresenta una disponibilità generale di un dataset e non implica alcuna informazione sul metodo di accesso effettivo ai dati, ad esempio se si tratta di un accesso a download diretto, API, o attraverso una pagina Web. L'utilizzo della proprietà dcat:downloadURL indica distribuzioni direttamente scaricabili."@it)
AnnotationAssertion(skos:scopeNote dcat:Distribution "This represents a general availability of a dataset it implies no information about the actual access method of the data, i.e. whether by direct download, API, or through a Web page. The use of dcat:downloadURL property indicates directly downloadable distributions."@en)
AnnotationAssertion(skos:scopeNote dcat:Distribution "Toto popisuje obecnou dostupnost datové sady. Neimplikuje žádnou informaci o skutečné metodě přístupu k datům, tj. zda jsou přímo ke stažení, skrze API či přes webovou stránku. Použití vlastnosti dcat:downloadURL indikuje přímo stažitelné distribuce."@cs)
AnnotationAssertion(skos:scopeNote dcat:Distribution "Αυτό αναπαριστά μία γενική διαθεσιμότητα ενός συνόλου δεδομένων και δεν υπονοεί τίποτα περί του πραγματικού τρόπου πρόσβασης στα δεδομένα, αν είναι άμεσα μεταφορτώσιμα, μέσω API ή μέσω μίας ιστοσελίδας. Η χρήση της ιδιότητας dcat:downloadURL δείχνει μόνο άμεσα μεταφορτώσιμες διανομές."@el)
AnnotationAssertion(skos:scopeNote dcat:Distribution "これは、データセットの一般的な利用可能性を表わし、データの実際のアクセス方式に関する情報（つまり、直接ダウンロードなのか、APIなのか、ウェブページを介したものなのか）を意味しません。dcat:downloadURLプロパティーの使用は、直接ダウンロード可能な配信を意味します。"@ja)

# Class: dcat:Relationship (Relazione)

AnnotationAssertion(rdfs:comment dcat:Relationship "An association class for attaching additional information to a relationship between DCAT Resources."@en)
AnnotationAssertion(rdfs:comment dcat:Relationship "Asociační třída pro připojení dodatečných informací ke vztahu mezi zdroji DCAT."@cs)
AnnotationAssertion(rdfs:comment dcat:Relationship "En associationsklasse til brug for tilknytning af yderligere information til en relation mellem DCAT-ressourcer."@da)
AnnotationAssertion(rdfs:comment dcat:Relationship "Una clase de asociación para adjuntar información adicional a una relación entre recursos DCAT."@es)
AnnotationAssertion(rdfs:comment dcat:Relationship "Una classe di associazione per il collegamento di informazioni aggiuntive a una relazione tra le risorse DCAT."@it)
AnnotationAssertion(rdfs:isDefinedBy dcat:Relationship <https://www.w3.org/TR/vocab-dcat-2/>)
AnnotationAssertion(rdfs:label dcat:Relationship "Relación"@es)
AnnotationAssertion(rdfs:label dcat:Relationship "Relation"@da)
AnnotationAssertion(rdfs:label dcat:Relationship "Relationship"@en)
AnnotationAssertion(rdfs:label dcat:Relationship "Relazione"@it)
AnnotationAssertion(rdfs:label dcat:Relationship "Vztah"@cs)
AnnotationAssertion(skos:changeNote dcat:Relationship "New class added in DCAT 2"@en)
AnnotationAssertion(skos:changeNote dcat:Relationship "Nová třída přidaná ve verzi DCAT 2"@cs)
AnnotationAssertion(skos:changeNote dcat:Relationship "Nueva clase añadida en DCAT 2"@es)
AnnotationAssertion(skos:changeNote dcat:Relationship "Nuova classe aggiunta in DCAT 2"@it)
AnnotationAssertion(skos:changeNote dcat:Relationship "Ny klasse i DCAT 2"@da)
AnnotationAssertion(skos:definition dcat:Relationship "An association class for attaching additional information to a relationship between DCAT Resources."@en)
AnnotationAssertion(skos:definition dcat:Relationship "Asociační třída pro připojení dodatečných informací ke vztahu mezi zdroji DCAT."@cs)
AnnotationAssertion(skos:definition dcat:Relationship "En associationsklasse til brug for tilknytning af yderligere information til en relation mellem DCAT-ressourcer."@da)
AnnotationAssertion(skos:definition dcat:Relationship "Una clase de asociación para adjuntar información adicional a una relación entre recursos DCAT."@es)
AnnotationAssertion(skos:definition dcat:Relationship "Una classe di associazione per il collegamento di informazioni aggiuntive a una relazione tra le risorse DCAT."@it)
AnnotationAssertion(skos:scopeNote dcat:Relationship "Anvendes til at karakterisere en relation mellem datasæt, og potentielt andre ressourcer, hvor relationen er kendt men ikke tilstrækkeligt beskrevet af de standardiserede egenskaber i Dublin Core (dcterms:hasPart, dcterms:isPartOf, dcterms:conformsTo, dcterms:isFormatOf, dcterms:hasFormat, dcterms:isVersionOf, dcterms:hasVersion, dcterms:replaces, dcterms:isReplacedBy, dcterms:references, dcterms:isReferencedBy, dcterms:requires, dcterms:isRequiredBy) eller PROV-O-egenskaber (prov:wasDerivedFrom, prov:wasInfluencedBy, prov:wasQuotedFrom, prov:wasRevisionOf, prov:hadPrimarySource, prov:alternateOf, prov:specializationOf)."@da)
AnnotationAssertion(skos:scopeNote dcat:Relationship "Používá se pro charakterizaci vztahu mezi datovými sadami a případně i jinými zdroji, kde druh vztahu je sice znám, ale není přiměřeně charakterizován standardními vlastnostmi slovníku Dublin Core (dcterms:hasPart, dcterms:isPartOf, dcterms:conformsTo, dcterms:isFormatOf, dcterms:hasFormat, dcterms:isVersionOf, dcterms:hasVersion, dcterms:replaces, dcterms:isReplacedBy, dcterms:references, dcterms:isReferencedBy, dcterms:requires, dcterms:isRequiredBy) či vlastnostmi slovníku PROV-O (prov:wasDerivedFrom, prov:wasInfluencedBy, prov:wasQuotedFrom, prov:wasRevisionOf, prov:hadPrimarySource, prov:alternateOf, prov:specializationOf)."@cs)
AnnotationAssertion(skos:scopeNote dcat:Relationship "Se usa para caracterizar la relación entre conjuntos de datos, y potencialmente otros recursos, donde la naturaleza de la relación se conoce pero no está caracterizada adecuadamente con propiedades del estándar 'Dublin Core' (dcterms:hasPart, dcterms:isPartOf, dcterms:conformsTo, dcterms:isFormatOf, dcterms:hasFormat, dcterms:isVersionOf, dcterms:hasVersion, dcterms:replaces, dcterms:isReplacedBy, dcterms:references, dcterms:isReferencedBy, dcterms:requires, dcterms:isRequiredBy) or PROV-O properties (prov:wasDerivedFrom, prov:wasInfluencedBy, prov:wasQuotedFrom, prov:wasRevisionOf, prov:hadPrimarySource, prov:alternateOf, prov:specializationOf)."@es)
AnnotationAssertion(skos:scopeNote dcat:Relationship "Use to characterize a relationship between datasets, and potentially other resources, where the nature of the relationship is known but is not adequately characterized by the standard Dublin Core properties (dcterms:hasPart, dcterms:isPartOf, dcterms:conformsTo, dcterms:isFormatOf, dcterms:hasFormat, dcterms:isVersionOf, dcterms:hasVersion, dcterms:replaces, dcterms:isReplacedBy, dcterms:references, dcterms:isReferencedBy, dcterms:requires, dcterms:isRequiredBy) or PROV-O properties (prov:wasDerivedFrom, prov:wasInfluencedBy, prov:wasQuotedFrom, prov:wasRevisionOf, prov:hadPrimarySource, prov:alternateOf, prov:specializationOf)."@en)
AnnotationAssertion(skos:scopeNote dcat:Relationship "Viene utilizzato per caratterizzare la relazione tra insiemi di dati, e potenzialmente altri tipi di risorse, nei casi in cui la natura della relazione è nota ma non adeguatamente caratterizzata dalle proprietà dello standard 'Dublin Core' (dcterms:hasPart, dcterms:isPartOf, dcterms:conformsTo, dcterms:isFormatOf, dcterms:hasFormat, dcterms:isVersionOf, dcterms:hasVersion, dcterms:replaces, dcterms:isReplacedBy, dcterms:references, dcterms:isReferencedBy, dcterms:require, dcterms:isRequiredBy) o dalle propietà fornite da PROV-O  (prov:wasDerivedFrom, prov:wasInfluencedBy, prov:wasQuotedFrom, prov:wasRevisionOf, prov: hadPrimarySource, prov:alternateOf, prov:specializationOf)."@it)

# Class: dcat:Resource (Risorsa catalogata)

AnnotationAssertion(rdfs:comment dcat:Resource "Recurso publicado o curado por un agente único."@es)
AnnotationAssertion(rdfs:comment dcat:Resource "Resource published or curated by a single agent."@en)
AnnotationAssertion(rdfs:comment dcat:Resource "Ressource udgivet eller udvalgt og arrangeret af en enkelt aktør."@da)
AnnotationAssertion(rdfs:comment dcat:Resource "Risorsa pubblicata o curata da un singolo agente."@it)
AnnotationAssertion(rdfs:comment dcat:Resource "Zdroj publikovaný či řízený jediným činitelem."@cs)
AnnotationAssertion(rdfs:isDefinedBy dcat:Resource <https://www.w3.org/TR/vocab-dcat-2/>)
AnnotationAssertion(rdfs:label dcat:Resource "Catalogued resource"@en)
AnnotationAssertion(rdfs:label dcat:Resource "Katalogiseret ressource"@da)
AnnotationAssertion(rdfs:label dcat:Resource "Katalogizovaný zdroj"@cs)
AnnotationAssertion(rdfs:label dcat:Resource "Recurso catalogado"@es)
AnnotationAssertion(rdfs:label dcat:Resource "Risorsa catalogata"@it)
AnnotationAssertion(skos:changeNote dcat:Resource "New class added in DCAT 2"@en)
AnnotationAssertion(skos:changeNote dcat:Resource "Nová třída přidaná ve verzi DCAT 2"@cs)
AnnotationAssertion(skos:changeNote dcat:Resource "Nueva clase agregada en DCAT 2"@es)
AnnotationAssertion(skos:changeNote dcat:Resource "Nuova classe aggiunta in DCAT 2"@it)
AnnotationAssertion(skos:changeNote dcat:Resource "Ny klasse i DCAT 2"@da)
AnnotationAssertion(skos:definition dcat:Resource "Recurso publicado o curado por un agente único."@es)
AnnotationAssertion(skos:definition dcat:Resource "Resource published or curated by a single agent."@en)
AnnotationAssertion(skos:definition dcat:Resource "Ressource udgivet eller udvalgt og arrangeret af en enkelt aktør."@da)
AnnotationAssertion(skos:definition dcat:Resource "Risorsa pubblicata o curata da un singolo agente."@it)
AnnotationAssertion(skos:definition dcat:Resource "Zdroj publikovaný či řízený jediným činitelem."@cs)
AnnotationAssertion(skos:editorialNote dcat:Resource "2020-08-23 Scopenote updated  and needs to be translated"@en)
AnnotationAssertion(skos:scopeNote dcat:Resource "Klassen for alle katalogiserede ressourcer, den overordnede klasse for dcat:Dataset, dcat:DataService, dcat:Catalog og enhvert medlem af et dcat:Catalog. Denne klasse bærer egenskaber der gælder alle katalogiserede ressourcer, herunder dataset og datatjenester. Det anbefales kraftigt at mere specifikke subklasser oprettes. Når der beskrives ressourcer der ikke er dcat:Dataset eller dcat:DataService, anbefales det at oprette passende subklasser af dcat:Resource eller at dcat:Resource anvendes sammen med egenskaben dcterms:type til opmærkning med en specifik typeangivelse."@da)
AnnotationAssertion(skos:scopeNote dcat:Resource "La clase de todos los recursos catalogados, la superclase de dcat:Dataset, dcat:DataService, dcat:Catalog y cualquier otro miembro de un dcat:Catalog. Esta clase tiene propiedades comunes a todos los recursos catalogados, incluyendo conjuntos de datos y servicios de datos. Se recomienda fuertemente que se use una clase más específica. Cuando se describe un recurso que no es un dcat:Dataset o dcat:DataService, se recomienda crear una sub-clase apropiada de dcat:Resource, o usar dcat:Resource con la propiedad dcterms:type to indicar el tipo específico."@es)
AnnotationAssertion(skos:scopeNote dcat:Resource "La classe di tutte le risorse catalogate, la Superclasse di dcat:Dataset, dcat:DataService, dcat:Catalog e qualsiasi altro membro di dcat:Catalog. Questa classe porta proprietà comuni a tutte le risorse catalogate, inclusi set di dati e servizi dati. Si raccomanda vivamente di utilizzare una sottoclasse più specifica. Quando si descrive una risorsa che non è un dcat:Dataset o dcat:DataService, si raccomanda di creare una sottoclasse di dcat:Resource appropriata, o utilizzare dcat:Resource con la proprietà dcterms:type per indicare il tipo specifico."@it)
AnnotationAssertion(skos:scopeNote dcat:Resource "The class of all catalogued resources, the Superclass of dcat:Dataset, dcat:DataService, dcat:Catalog and any other member of a dcat:Catalog. This class carries properties common to all catalogued resources, including datasets and data services. The instances of this class SHOULD be included in a catalog. The instances of this class SHOULD be included in a catalog. It is strongly recommended to use a more specific sub-class. When describing a resource which is not a dcat:Dataset or dcat:DataService, it is recommended to create a suitable sub-class of dcat:Resource, or use dcat:Resource with the dcterms:type property to indicate the specific type."@en)
AnnotationAssertion(skos:scopeNote dcat:Resource "Třída všech katalogizovaných zdrojů, nadtřída dcat:Dataset, dcat:DataService, dcat:Catalog a všech ostatních členů dcat:Catalog. Tato třída nese vlastnosti společné všem katalogizovaným zdrojům včetně datových sad a datových služeb. Je silně doporučeno používat specifičtější podtřídy, pokud je to možné. Při popisu zdroje, který není ani dcat:Dataset, ani dcat:DataService se doporučuje vytvořit odpovídající podtřídu dcat:Resrouce a nebo použít dcat:Resource s vlastností dcterms:type pro určení konkrétního typu."@cs)
AnnotationAssertion(skos:scopeNote dcat:Resource "dcat:Resource er et udvidelsespunkt der tillader oprettelsen af enhver type af kataloger. Yderligere subklasser kan defineres i en DCAT-profil eller i en applikation til kataloger med andre typer af ressourcer."@da)
AnnotationAssertion(skos:scopeNote dcat:Resource "dcat:Resource es un punto de extensión que permite la definición de cualquier tipo de catálogo. Se pueden definir subclases adicionales en perfil de DCAT o una aplicación para catálogos de otro tipo de recursos."@es)
AnnotationAssertion(skos:scopeNote dcat:Resource "dcat:Resource is an extension point that enables the definition of any kind of catalog. Additional subclasses may be defined in a DCAT profile or application for catalogs of other kinds of resources."@en)
AnnotationAssertion(skos:scopeNote dcat:Resource "dcat:Resource je bod pro rozšíření umožňující definici různých druhů katalogů. Další podtřídy lze definovat v profilech DCAT či aplikacích pro katalogy zdrojů jiných druhů."@cs)
AnnotationAssertion(skos:scopeNote dcat:Resource "dcat:Resource è un punto di estensione che consente la definizione di qualsiasi tipo di catalogo. Sottoclassi aggiuntive possono essere definite in un profilo DCAT o in un'applicazione per cataloghi di altri tipi di risorse."@it)

# Class: dcat:Role (Rolle)

AnnotationAssertion(rdfs:comment dcat:Role "A role is the function of a resource or agent with respect to another resource, in the context of resource attribution or resource relationships."@en)
AnnotationAssertion(rdfs:comment dcat:Role "En rolle er den funktion en ressource eller aktør har i forhold til en anden ressource, i forbindelse med ressourcekreditering eller ressourcerelationer."@da)
AnnotationAssertion(rdfs:comment dcat:Role "Role je funkce zdroje či agenta ve vztahu k jinému zdroji, v kontextu přiřazení zdrojů či vztahů mezi zdroji."@cs)
AnnotationAssertion(rdfs:comment dcat:Role "Un rol es la función de un recurso o agente con respecto a otro recuros, en el contexto de atribución del recurso o de las relaciones entre recursos."@es)
AnnotationAssertion(rdfs:comment dcat:Role "Un ruolo è la funzione di una risorsa o di un agente rispetto ad un'altra risorsa, nel contesto dell'attribuzione delle risorse o delle relazioni tra risorse."@it)
AnnotationAssertion(rdfs:isDefinedBy dcat:Role <https://www.w3.org/TR/vocab-dcat-2/>)
AnnotationAssertion(rdfs:label dcat:Role "Rol"@es)
AnnotationAssertion(rdfs:label dcat:Role "Role"@cs)
AnnotationAssertion(rdfs:label dcat:Role "Role"@en)
AnnotationAssertion(rdfs:label dcat:Role "Rolle"@da)
AnnotationAssertion(rdfs:label dcat:Role "Ruolo"@it)
AnnotationAssertion(rdfs:seeAlso dcat:Role dcat:hadRole)
AnnotationAssertion(skos:changeNote dcat:Role "New class added in DCAT 2"@en)
AnnotationAssertion(skos:changeNote dcat:Role "Nová třída přidaná ve verzi DCAT 2"@cs)
AnnotationAssertion(skos:changeNote dcat:Role "Nueva clase agregada en DCAT 2"@es)
AnnotationAssertion(skos:changeNote dcat:Role "Nuova classe aggiunta in DCAT 2"@it)
AnnotationAssertion(skos:changeNote dcat:Role "Ny klasse tilføjet i DCAT 2"@da)
AnnotationAssertion(skos:definition dcat:Role "A role is the function of a resource or agent with respect to another resource, in the context of resource attribution or resource relationships."@en)
AnnotationAssertion(skos:definition dcat:Role "En rolle er den funktion en ressource eller aktør har i forhold til en anden ressource, i forbindelse med ressourcekreditering eller ressourcerelationer."@da)
AnnotationAssertion(skos:definition dcat:Role "Role je funkce zdroje či agenta ve vztahu k jinému zdroji, v kontextu přiřazení zdrojů či vztahů mezi zdroji."@cs)
AnnotationAssertion(skos:definition dcat:Role "Un rol es la función de un recurso o agente con respecto a otro recuros, en el contexto de atribución del recurso o de las relaciones entre recursos."@es)
AnnotationAssertion(skos:definition dcat:Role "Un ruolo è la funzione di una risorsa o di un agente rispetto ad un'altra risorsa, nel contesto dell'attribuzione delle risorse o delle relazioni tra risorse."@it)
AnnotationAssertion(skos:editorialNote dcat:Role "Incluída en DCAT para complementar prov:Role (cuyo uso está limitado a roles en el contexto de una actividad, ya que es el rango es prov:hadRole)."@es)
AnnotationAssertion(skos:editorialNote dcat:Role "Introdotta in DCAT per completare prov:Role (il cui uso è limitato ai ruoli nel contesto di un'attività, in conseguenza alla definizione del codominio di prov:hadRole)."@it)
AnnotationAssertion(skos:editorialNote dcat:Role "Introduced into DCAT to complement prov:Role (whose use is limited to roles in the context of an activity, as the range of prov:hadRole)."@en)
AnnotationAssertion(skos:editorialNote dcat:Role "Introduceret i DCAT for at supplere prov:Role (hvis anvendelse er begrænset til roller i forbindelse med en aktivitet, som er rækkevidde for prov:hadRole)."@da)
AnnotationAssertion(skos:editorialNote dcat:Role "Přidáno do DCAT pro doplnění třídy prov:Role (jejíž užití je omezeno na role v kontextu aktivit, jakožto obor hodnot vlastnosti prov:hadRole)."@cs)
AnnotationAssertion(skos:scopeNote dcat:Role "Anvendes i forbindelse med kvalificerede krediteringer til at angive aktørens rolle i forhold til en entitet. Det anbefales at værdierne styres som et kontrolleret udfaldsrum med aktørroller, såsom http://registry.it.csiro.au/def/isotc211/CI_RoleCode."@da)
AnnotationAssertion(skos:scopeNote dcat:Role "Anvendes i forbindelse med kvalificerede relationer til at specificere en entitets rolle i forhold til en anden entitet. Det anbefales at værdierne styres med et kontrolleret udfaldsrum for for entitetsroller såsom: ISO 19115 DS_AssociationTypeCode http://registry.it.csiro.au/def/isotc211/DS_AssociationTypeCode; IANA Registry of Link Relations https://www.iana.org/assignments/link-relation;  DataCite metadata schema;  MARC relators https://id.loc.gov/vocabulary/relators."@da)
AnnotationAssertion(skos:scopeNote dcat:Role "Použito v kvalifikovaném přiřazení pro specifikaci role Agenta ve vztahu k Entitě. Je doporučeno množinu hodnot spravovat jako řízený slovník rolí agentů, jako například http://registry.it.csiro.au/def/isotc211/CI_RoleCode."@cs)
AnnotationAssertion(skos:scopeNote dcat:Role "Použito v kvalifikovaném vztahu pro specifikaci role Entity ve vztahu k jiné Entitě. Je doporučeno množinu hodnot spravovat jako řízený slovník rolí entit, jako například ISO 19115 DS_AssociationTypeCode http://registry.it.csiro.au/def/isotc211/DS_AssociationTypeCode, IANA Registry of Link Relations https://www.iana.org/assignments/link-relation, DataCite metadata schema, či MARC relators https://id.loc.gov/vocabulary/relators."@cs)
AnnotationAssertion(skos:scopeNote dcat:Role "Se usa en una atribución cualificada para especificar el rol de un Agente con respecto a una Entidad. Se recomienda que los valores se administren como un vocabulario controlado de roles de agente, como por ejemplo http://registry.it.csiro.au/def/isotc211/CI_RoleCode."@es)
AnnotationAssertion(skos:scopeNote dcat:Role "Se usa en una relación cualificada para especificar el rol de una Entidad con respecto a otra Entidad. Se recomienda que los valores se administren como los valores de un vocabulario controlado de roles de entidad como por ejemplo: ISO 19115 DS_AssociationTypeCode http://registry.it.csiro.au/def/isotc211/DS_AssociationTypeCode; IANA Registry of Link Relations https://www.iana.org/assignments/link-relation; el esquema de metadatos de DataCite; MARC relators https://id.loc.gov/vocabulary/relators."@es)
AnnotationAssertion(skos:scopeNote dcat:Role "Used in a qualified-attribution to specify the role of an Agent with respect to an Entity. It is recommended that the values be managed as a controlled vocabulary of agent roles, such as http://registry.it.csiro.au/def/isotc211/CI_RoleCode."@en)
AnnotationAssertion(skos:scopeNote dcat:Role "Used in a qualified-relation to specify the role of an Entity with respect to another Entity. It is recommended that the values be managed as a controlled vocabulary of entity roles such as: ISO 19115 DS_AssociationTypeCode http://registry.it.csiro.au/def/isotc211/DS_AssociationTypeCode; IANA Registry of Link Relations https://www.iana.org/assignments/link-relation;  DataCite metadata schema;  MARC relators https://id.loc.gov/vocabulary/relators."@en)
AnnotationAssertion(skos:scopeNote dcat:Role "Utilizzato in un'attribuzione qualificata per specificare il ruolo di un agente rispetto a un'entità. Si consiglia di attribuire i valori considerando un vocabolario controllato dei ruoli dell'agente, ad esempio http://registry.it.csiro.au/def/isotc211/CI_RoleCode."@it)
AnnotationAssertion(skos:scopeNote dcat:Role "Utilizzato in una relazione qualificata per specificare il ruolo di un'entità rispetto a un'altra entità. Si raccomanda che il valore sia preso da un vocabolario controllato di ruoli di entità come ISO 19115 DS_AssociationTypeCode http://registry.it.csiro.au/def/isotc211/DS_AssociationTypeCode, IANA Registry of Link Relations https://www.iana.org/assignments/link-relation, DataCite metadata schema, o MARC relators https://id.loc.gov/vocabulary/relators."@it)
SubClassOf(dcat:Role skos:Concept)


############################
#   Named Individuals
############################

# Individual: dcterms: (dcterms:)

AnnotationAssertion(dcterms:publisher <http://purl.org/dc/terms/> <http://purl.org/dc/aboutdcmi#DCMI>)
DataPropertyAssertion(dcterms:modified <http://purl.org/dc/terms/> "2012-06-14"^^xsd:date)
DataPropertyAssertion(dcterms:title <http://purl.org/dc/terms/> "DCMI Metadata Terms - other"@en)

# Individual: dcterms:Agent (Agent)

ClassAssertion(dcterms:AgentClass dcterms:Agent)
DataPropertyAssertion(dcterms:issued dcterms:Agent "2008-01-14"^^xsd:date)

# Individual: dcterms:AgentClass (Agent Class)

DataPropertyAssertion(dcterms:issued dcterms:AgentClass "2008-01-14"^^xsd:date)

# Individual: dcterms:BibliographicResource (Bibliographic Resource)

DataPropertyAssertion(dcterms:issued dcterms:BibliographicResource "2008-01-14"^^xsd:date)

# Individual: dcterms:Box (DCMI Box)

DataPropertyAssertion(dcterms:issued dcterms:Box "2000-07-11"^^xsd:date)

# Individual: dcterms:DCMIType (DCMI Type Vocabulary)

AnnotationAssertion(rdfs:comment dcterms:DCMIType "The set of classes specified by the DCMI Type Vocabulary, used to categorize the nature or genre of the resource."@en)
AnnotationAssertion(rdfs:isDefinedBy dcterms:DCMIType <http://purl.org/dc/terms/>)
AnnotationAssertion(rdfs:label dcterms:DCMIType "DCMI Type Vocabulary"@en)
AnnotationAssertion(rdfs:seeAlso dcterms:DCMIType <http://purl.org/dc/dcmitype/>)
ClassAssertion(<http://purl.org/dc/dcam/VocabularyEncodingScheme> dcterms:DCMIType)
DataPropertyAssertion(dcterms:issued dcterms:DCMIType "2000-07-11"^^xsd:date)

# Individual: dcterms:DDC (DDC)

AnnotationAssertion(rdfs:comment dcterms:DDC "The set of conceptual resources specified by the Dewey Decimal Classification."@en)
AnnotationAssertion(rdfs:isDefinedBy dcterms:DDC <http://purl.org/dc/terms/>)
AnnotationAssertion(rdfs:label dcterms:DDC "DDC"@en)
AnnotationAssertion(rdfs:seeAlso dcterms:DDC <http://www.oclc.org/dewey/>)
ClassAssertion(<http://purl.org/dc/dcam/VocabularyEncodingScheme> dcterms:DDC)
DataPropertyAssertion(dcterms:issued dcterms:DDC "2000-07-11"^^xsd:date)

# Individual: dcterms:FileFormat (File Format)

DataPropertyAssertion(dcterms:issued dcterms:FileFormat "2008-01-14"^^xsd:date)

# Individual: dcterms:Frequency (Frequency)

DataPropertyAssertion(dcterms:issued dcterms:Frequency "2008-01-14"^^xsd:date)

# Individual: dcterms:IMT (IMT)

AnnotationAssertion(rdfs:comment dcterms:IMT "The set of media types specified by the Internet Assigned Numbers Authority."@en)
AnnotationAssertion(rdfs:isDefinedBy dcterms:IMT <http://purl.org/dc/terms/>)
AnnotationAssertion(rdfs:label dcterms:IMT "IMT"@en)
AnnotationAssertion(rdfs:seeAlso dcterms:IMT <http://www.iana.org/assignments/media-types/>)
ClassAssertion(<http://purl.org/dc/dcam/VocabularyEncodingScheme> dcterms:IMT)
DataPropertyAssertion(dcterms:issued dcterms:IMT "2000-07-11"^^xsd:date)

# Individual: dcterms:ISO3166 (ISO 3166)

DataPropertyAssertion(dcterms:issued dcterms:ISO3166 "2000-07-11"^^xsd:date)

# Individual: dcterms:ISO639-2 (ISO 639-2)

DataPropertyAssertion(dcterms:issued dcterms:ISO639-2 "2000-07-11"^^xsd:date)

# Individual: dcterms:ISO639-3 (ISO 639-3)

DataPropertyAssertion(dcterms:issued dcterms:ISO639-3 "2008-01-14"^^xsd:date)

# Individual: dcterms:Jurisdiction (Jurisdiction)

DataPropertyAssertion(dcterms:issued dcterms:Jurisdiction "2008-01-14"^^xsd:date)

# Individual: dcterms:LCC (LCC)

AnnotationAssertion(rdfs:comment dcterms:LCC "The set of conceptual resources specified by the Library of Congress Classification."@en)
AnnotationAssertion(rdfs:isDefinedBy dcterms:LCC <http://purl.org/dc/terms/>)
AnnotationAssertion(rdfs:label dcterms:LCC "LCC"@en)
AnnotationAssertion(rdfs:seeAlso dcterms:LCC <http://lcweb.loc.gov/catdir/cpso/lcco/lcco.html>)
ClassAssertion(<http://purl.org/dc/dcam/VocabularyEncodingScheme> dcterms:LCC)
DataPropertyAssertion(dcterms:issued dcterms:LCC "2000-07-11"^^xsd:date)

# Individual: dcterms:LCSH (LCSH)

AnnotationAssertion(rdfs:comment dcterms:LCSH "The set of labeled concepts specified by the Library of Congress Subject Headings."@en)
AnnotationAssertion(rdfs:isDefinedBy dcterms:LCSH <http://purl.org/dc/terms/>)
AnnotationAssertion(rdfs:label dcterms:LCSH "LCSH"@en)
ClassAssertion(<http://purl.org/dc/dcam/VocabularyEncodingScheme> dcterms:LCSH)
DataPropertyAssertion(dcterms:issued dcterms:LCSH "2000-07-11"^^xsd:date)

# Individual: dcterms:LicenseDocument (License Document)

DataPropertyAssertion(dcterms:issued dcterms:LicenseDocument "2008-01-14"^^xsd:date)

# Individual: dcterms:LinguisticSystem (Linguistic System)

DataPropertyAssertion(dcterms:issued dcterms:LinguisticSystem "2008-01-14"^^xsd:date)

# Individual: dcterms:Location (Location)

DataPropertyAssertion(dcterms:issued dcterms:Location "2008-01-14"^^xsd:date)

# Individual: dcterms:LocationPeriodOrJurisdiction (Location, Period, or Jurisdiction)

DataPropertyAssertion(dcterms:issued dcterms:LocationPeriodOrJurisdiction "2008-01-14"^^xsd:date)

# Individual: dcterms:MESH (MeSH)

AnnotationAssertion(rdfs:comment dcterms:MESH "The set of labeled concepts specified by the Medical Subject Headings."@en)
AnnotationAssertion(rdfs:isDefinedBy dcterms:MESH <http://purl.org/dc/terms/>)
AnnotationAssertion(rdfs:label dcterms:MESH "MeSH"@en)
AnnotationAssertion(rdfs:seeAlso dcterms:MESH <http://www.nlm.nih.gov/mesh/meshhome.html>)
ClassAssertion(<http://purl.org/dc/dcam/VocabularyEncodingScheme> dcterms:MESH)
DataPropertyAssertion(dcterms:issued dcterms:MESH "2000-07-11"^^xsd:date)

# Individual: dcterms:MediaType (Media Type)

DataPropertyAssertion(dcterms:issued dcterms:MediaType "2008-01-14"^^xsd:date)

# Individual: dcterms:MediaTypeOrExtent (Media Type or Extent)

DataPropertyAssertion(dcterms:issued dcterms:MediaTypeOrExtent "2008-01-14"^^xsd:date)

# Individual: dcterms:MethodOfAccrual (Method of Accrual)

DataPropertyAssertion(dcterms:issued dcterms:MethodOfAccrual "2008-01-14"^^xsd:date)

# Individual: dcterms:MethodOfInstruction (Method of Instruction)

DataPropertyAssertion(dcterms:issued dcterms:MethodOfInstruction "2008-01-14"^^xsd:date)

# Individual: dcterms:NLM (NLM)

AnnotationAssertion(rdfs:comment dcterms:NLM "The set of conceptual resources specified by the National Library of Medicine Classification."@en)
AnnotationAssertion(rdfs:isDefinedBy dcterms:NLM <http://purl.org/dc/terms/>)
AnnotationAssertion(rdfs:label dcterms:NLM "NLM"@en)
AnnotationAssertion(rdfs:seeAlso dcterms:NLM <http://wwwcf.nlm.nih.gov/class/>)
ClassAssertion(<http://purl.org/dc/dcam/VocabularyEncodingScheme> dcterms:NLM)
DataPropertyAssertion(dcterms:issued dcterms:NLM "2005-06-13"^^xsd:date)

# Individual: dcterms:Period (DCMI Period)

DataPropertyAssertion(dcterms:issued dcterms:Period "2000-07-11"^^xsd:date)

# Individual: dcterms:PeriodOfTime (Period of Time)

DataPropertyAssertion(dcterms:issued dcterms:PeriodOfTime "2008-01-14"^^xsd:date)

# Individual: dcterms:PhysicalMedium (Physical Medium)

DataPropertyAssertion(dcterms:issued dcterms:PhysicalMedium "2008-01-14"^^xsd:date)

# Individual: dcterms:PhysicalResource (Physical Resource)

DataPropertyAssertion(dcterms:issued dcterms:PhysicalResource "2008-01-14"^^xsd:date)

# Individual: dcterms:Point (DCMI Point)

DataPropertyAssertion(dcterms:issued dcterms:Point "2000-07-11"^^xsd:date)

# Individual: dcterms:Policy (Policy)

DataPropertyAssertion(dcterms:issued dcterms:Policy "2008-01-14"^^xsd:date)

# Individual: dcterms:ProvenanceStatement (Provenance Statement)

DataPropertyAssertion(dcterms:issued dcterms:ProvenanceStatement "2008-01-14"^^xsd:date)

# Individual: dcterms:RFC1766 (RFC 1766)

DataPropertyAssertion(dcterms:issued dcterms:RFC1766 "2000-07-11"^^xsd:date)

# Individual: dcterms:RFC3066 (RFC 3066)

DataPropertyAssertion(dcterms:issued dcterms:RFC3066 "2002-07-13"^^xsd:date)

# Individual: dcterms:RFC4646 (RFC 4646)

DataPropertyAssertion(dcterms:issued dcterms:RFC4646 "2008-01-14"^^xsd:date)

# Individual: dcterms:RFC5646 (RFC 5646)

DataPropertyAssertion(dcterms:issued dcterms:RFC5646 "2010-10-11"^^xsd:date)

# Individual: dcterms:RightsStatement (Rights Statement)

DataPropertyAssertion(dcterms:issued dcterms:RightsStatement "2008-01-14"^^xsd:date)

# Individual: dcterms:SizeOrDuration (Size or Duration)

DataPropertyAssertion(dcterms:issued dcterms:SizeOrDuration "2008-01-14"^^xsd:date)

# Individual: dcterms:Standard (Standard)

DataPropertyAssertion(dcterms:issued dcterms:Standard "2008-01-14"^^xsd:date)

# Individual: dcterms:TGN (TGN)

AnnotationAssertion(rdfs:comment dcterms:TGN "The set of places specified by the Getty Thesaurus of Geographic Names."@en)
AnnotationAssertion(rdfs:isDefinedBy dcterms:TGN <http://purl.org/dc/terms/>)
AnnotationAssertion(rdfs:label dcterms:TGN "TGN"@en)
AnnotationAssertion(rdfs:seeAlso dcterms:TGN <http://www.getty.edu/research/tools/vocabulary/tgn/index.html>)
ClassAssertion(<http://purl.org/dc/dcam/VocabularyEncodingScheme> dcterms:TGN)
DataPropertyAssertion(dcterms:issued dcterms:TGN "2000-07-11"^^xsd:date)

# Individual: dcterms:UDC (UDC)

AnnotationAssertion(rdfs:comment dcterms:UDC "The set of conceptual resources specified by the Universal Decimal Classification."@en)
AnnotationAssertion(rdfs:isDefinedBy dcterms:UDC <http://purl.org/dc/terms/>)
AnnotationAssertion(rdfs:label dcterms:UDC "UDC"@en)
AnnotationAssertion(rdfs:seeAlso dcterms:UDC <http://www.udcc.org/>)
ClassAssertion(<http://purl.org/dc/dcam/VocabularyEncodingScheme> dcterms:UDC)
DataPropertyAssertion(dcterms:issued dcterms:UDC "2000-07-11"^^xsd:date)

# Individual: dcterms:URI (URI)

DataPropertyAssertion(dcterms:issued dcterms:URI "2000-07-11"^^xsd:date)

# Individual: dcterms:W3CDTF (W3C-DTF)

DataPropertyAssertion(dcterms:issued dcterms:W3CDTF "2000-07-11"^^xsd:date)

# Individual: dcterms:abstract (Abstract)

DataPropertyAssertion(dcterms:issued dcterms:abstract "2000-07-11"^^xsd:date)

# Individual: dcterms:accessRights (Access Rights)

DataPropertyAssertion(dcterms:issued dcterms:accessRights "2003-02-15"^^xsd:date)

# Individual: dcterms:accrualMethod (Accrual Method)

DataPropertyAssertion(dcterms:issued dcterms:accrualMethod "2005-06-13"^^xsd:date)

# Individual: dcterms:accrualPeriodicity (Accrual Periodicity)

DataPropertyAssertion(dcterms:issued dcterms:accrualPeriodicity "2005-06-13"^^xsd:date)

# Individual: dcterms:accrualPolicy (Accrual Policy)

DataPropertyAssertion(dcterms:issued dcterms:accrualPolicy "2005-06-13"^^xsd:date)

# Individual: dcterms:alternative (Alternative Title)

DataPropertyAssertion(dcterms:issued dcterms:alternative "2000-07-11"^^xsd:date)

# Individual: dcterms:audience (Audience)

DataPropertyAssertion(dcterms:issued dcterms:audience "2001-05-21"^^xsd:date)

# Individual: dcterms:available (Date Available)

DataPropertyAssertion(dcterms:issued dcterms:available "2000-07-11"^^xsd:date)

# Individual: dcterms:bibliographicCitation (Bibliographic Citation)

DataPropertyAssertion(dcterms:issued dcterms:bibliographicCitation "2003-02-15"^^xsd:date)

# Individual: dcterms:conformsTo (Conforms To)

DataPropertyAssertion(dcterms:issued dcterms:conformsTo "2001-05-21"^^xsd:date)

# Individual: dcterms:contributor (Contributor)

DataPropertyAssertion(dcterms:issued dcterms:contributor "2008-01-14"^^xsd:date)

# Individual: dcterms:coverage (Coverage)

DataPropertyAssertion(dcterms:issued dcterms:coverage "2008-01-14"^^xsd:date)

# Individual: dcterms:created (Date Created)

DataPropertyAssertion(dcterms:issued dcterms:created "2000-07-11"^^xsd:date)

# Individual: dcterms:creator (Creator)

DataPropertyAssertion(dcterms:issued dcterms:creator "2008-01-14"^^xsd:date)

# Individual: dcterms:date (Date)

DataPropertyAssertion(dcterms:issued dcterms:date "2008-01-14"^^xsd:date)

# Individual: dcterms:dateAccepted (Date Accepted)

DataPropertyAssertion(dcterms:issued dcterms:dateAccepted "2002-07-13"^^xsd:date)

# Individual: dcterms:dateCopyrighted (Date Copyrighted)

DataPropertyAssertion(dcterms:issued dcterms:dateCopyrighted "2002-07-13"^^xsd:date)

# Individual: dcterms:dateSubmitted (Date Submitted)

DataPropertyAssertion(dcterms:issued dcterms:dateSubmitted "2002-07-13"^^xsd:date)

# Individual: dcterms:description (Description)

DataPropertyAssertion(dcterms:issued dcterms:description "2008-01-14"^^xsd:date)

# Individual: dcterms:educationLevel (Audience Education Level)

DataPropertyAssertion(dcterms:issued dcterms:educationLevel "2002-07-13"^^xsd:date)

# Individual: dcterms:extent (Extent)

DataPropertyAssertion(dcterms:issued dcterms:extent "2000-07-11"^^xsd:date)

# Individual: dcterms:format (Format)

DataPropertyAssertion(dcterms:issued dcterms:format "2008-01-14"^^xsd:date)

# Individual: dcterms:hasFormat (Has Format)

DataPropertyAssertion(dcterms:issued dcterms:hasFormat "2000-07-11"^^xsd:date)

# Individual: dcterms:hasPart (Has Part)

DataPropertyAssertion(dcterms:issued dcterms:hasPart "2000-07-11"^^xsd:date)

# Individual: dcterms:hasVersion (Has Version)

DataPropertyAssertion(dcterms:issued dcterms:hasVersion "2000-07-11"^^xsd:date)

# Individual: dcterms:identifier (Identifier)

DataPropertyAssertion(dcterms:issued dcterms:identifier "2008-01-14"^^xsd:date)

# Individual: dcterms:instructionalMethod (Instructional Method)

AnnotationAssertion(<http://purl.org/dc/dcam/rangeIncludes> dcterms:instructionalMethod dcterms:MethodOfInstruction)
AnnotationAssertion(dcterms:description dcterms:instructionalMethod "Instructional Method typically includes ways of presenting instructional materials or conducting instructional activities, patterns of learner-to-learner and learner-to-instructor interactions, and mechanisms by which group and individual levels of learning are measured.  Instructional methods include all aspects of the instruction and learning processes from planning and implementation through evaluation and feedback."@en)
AnnotationAssertion(rdfs:comment dcterms:instructionalMethod "A process, used to engender knowledge, attitudes and skills, that the described resource is designed to support."@en)
AnnotationAssertion(rdfs:isDefinedBy dcterms:instructionalMethod <http://purl.org/dc/terms/>)
AnnotationAssertion(rdfs:label dcterms:instructionalMethod "Instructional Method"@en)
DataPropertyAssertion(dcterms:issued dcterms:instructionalMethod "2005-06-13"^^xsd:date)

# Individual: dcterms:isFormatOf (Is Format Of)

DataPropertyAssertion(dcterms:issued dcterms:isFormatOf "2000-07-11"^^xsd:date)

# Individual: dcterms:isPartOf (Is Part Of)

DataPropertyAssertion(dcterms:issued dcterms:isPartOf "2000-07-11"^^xsd:date)

# Individual: dcterms:isReferencedBy (Is Referenced By)

DataPropertyAssertion(dcterms:issued dcterms:isReferencedBy "2000-07-11"^^xsd:date)

# Individual: dcterms:isReplacedBy (Is Replaced By)

DataPropertyAssertion(dcterms:issued dcterms:isReplacedBy "2000-07-11"^^xsd:date)

# Individual: dcterms:isRequiredBy (Is Required By)

DataPropertyAssertion(dcterms:issued dcterms:isRequiredBy "2000-07-11"^^xsd:date)

# Individual: dcterms:isVersionOf (Is Version Of)

DataPropertyAssertion(dcterms:issued dcterms:isVersionOf "2000-07-11"^^xsd:date)

# Individual: dcterms:issued (Date Issued)

DataPropertyAssertion(dcterms:issued dcterms:issued "2000-07-11"^^xsd:date)

# Individual: dcterms:language (Language)

DataPropertyAssertion(dcterms:issued dcterms:language "2008-01-14"^^xsd:date)

# Individual: dcterms:license (License)

DataPropertyAssertion(dcterms:issued dcterms:license "2004-06-14"^^xsd:date)

# Individual: dcterms:mediator (Mediator)

DataPropertyAssertion(dcterms:issued dcterms:mediator "2001-05-21"^^xsd:date)

# Individual: dcterms:medium (Medium)

DataPropertyAssertion(dcterms:issued dcterms:medium "2000-07-11"^^xsd:date)

# Individual: dcterms:modified (Date Modified)

DataPropertyAssertion(dcterms:issued dcterms:modified "2000-07-11"^^xsd:date)

# Individual: dcterms:provenance (Provenance)

AnnotationAssertion(<http://purl.org/dc/dcam/rangeIncludes> dcterms:provenance dcterms:ProvenanceStatement)
AnnotationAssertion(dcterms:description dcterms:provenance "The statement may include a description of any changes successive custodians made to the resource."@en)
AnnotationAssertion(rdfs:comment dcterms:provenance "A statement of any changes in ownership and custody of the resource since its creation that are significant for its authenticity, integrity, and interpretation."@en)
AnnotationAssertion(rdfs:isDefinedBy dcterms:provenance <http://purl.org/dc/terms/>)
AnnotationAssertion(rdfs:label dcterms:provenance "Provenance"@en)
DataPropertyAssertion(dcterms:issued dcterms:provenance "2004-09-20"^^xsd:date)

# Individual: dcterms:publisher (Publisher)

DataPropertyAssertion(dcterms:issued dcterms:publisher "2008-01-14"^^xsd:date)

# Individual: dcterms:references (References)

DataPropertyAssertion(dcterms:issued dcterms:references "2000-07-11"^^xsd:date)

# Individual: dcterms:relation (Relation)

DataPropertyAssertion(dcterms:issued dcterms:relation "2008-01-14"^^xsd:date)

# Individual: dcterms:replaces (Replaces)

DataPropertyAssertion(dcterms:issued dcterms:replaces "2000-07-11"^^xsd:date)

# Individual: dcterms:requires (Requires)

DataPropertyAssertion(dcterms:issued dcterms:requires "2000-07-11"^^xsd:date)

# Individual: dcterms:rights (Rights)

DataPropertyAssertion(dcterms:issued dcterms:rights "2008-01-14"^^xsd:date)

# Individual: dcterms:rightsHolder (Rights Holder)

AnnotationAssertion(<http://purl.org/dc/dcam/rangeIncludes> dcterms:rightsHolder dcterms:Agent)
AnnotationAssertion(dcterms:description dcterms:rightsHolder "Recommended practice is to refer to the rights holder with a URI. If this is not possible or feasible, a literal value that identifies the rights holder may be provided."@en)
AnnotationAssertion(rdfs:comment dcterms:rightsHolder "A person or organization owning or managing rights over the resource."@en)
AnnotationAssertion(rdfs:isDefinedBy dcterms:rightsHolder <http://purl.org/dc/terms/>)
AnnotationAssertion(rdfs:label dcterms:rightsHolder "Rights Holder"@en)
DataPropertyAssertion(dcterms:issued dcterms:rightsHolder "2004-06-14"^^xsd:date)

# Individual: dcterms:source (Source)

DataPropertyAssertion(dcterms:issued dcterms:source "2008-01-14"^^xsd:date)

# Individual: dcterms:spatial (Spatial Coverage)

DataPropertyAssertion(dcterms:issued dcterms:spatial "2000-07-11"^^xsd:date)

# Individual: dcterms:subject (Subject)

DataPropertyAssertion(dcterms:issued dcterms:subject "2008-01-14"^^xsd:date)

# Individual: dcterms:tableOfContents (Table Of Contents)

DataPropertyAssertion(dcterms:issued dcterms:tableOfContents "2000-07-11"^^xsd:date)

# Individual: dcterms:temporal (Temporal Coverage)

DataPropertyAssertion(dcterms:issued dcterms:temporal "2000-07-11"^^xsd:date)

# Individual: dcterms:title (Title)

DataPropertyAssertion(dcterms:issued dcterms:title "2008-01-14"^^xsd:date)

# Individual: dcterms:type (Type)

DataPropertyAssertion(dcterms:issued dcterms:type "2008-01-14"^^xsd:date)

# Individual: dcterms:valid (Date Valid)

DataPropertyAssertion(dcterms:issued dcterms:valid "2000-07-11"^^xsd:date)

# Individual: <http://www.w3.org/ns/dcat> (<http://www.w3.org/ns/dcat>)

ObjectPropertyAssertion(dcat:hasCurrentVersion <http://www.w3.org/ns/dcat> <http://www.w3.org/ns/dcat3>)
ObjectPropertyAssertion(dcat:hasVersion <http://www.w3.org/ns/dcat> <http://www.w3.org/ns/dcat2>)
ObjectPropertyAssertion(dcat:hasVersion <http://www.w3.org/ns/dcat> <http://www.w3.org/ns/dcat2014>)
ObjectPropertyAssertion(dcat:hasVersion <http://www.w3.org/ns/dcat> <http://www.w3.org/ns/dcat3>)
ObjectPropertyAssertion(dcat:previousVersion <http://www.w3.org/ns/dcat> <http://www.w3.org/ns/dcat2>)
DataPropertyAssertion(dcterms:created <http://www.w3.org/ns/dcat> "2020-12-17"^^xsd:date)
DataPropertyAssertion(dcterms:modified <http://www.w3.org/ns/dcat> "2020-11-30"^^xsd:date)
DataPropertyAssertion(dcterms:modified <http://www.w3.org/ns/dcat> "2021-03-09"^^xsd:date)
DataPropertyAssertion(dcterms:modified <http://www.w3.org/ns/dcat> "2021-04-08"^^xsd:date)
DataPropertyAssertion(dcterms:modified <http://www.w3.org/ns/dcat> "2021-06-23"^^xsd:date)
DataPropertyAssertion(dcterms:modified <http://www.w3.org/ns/dcat> "2021-09-27"^^xsd:date)
DataPropertyAssertion(dcterms:modified <http://www.w3.org/ns/dcat> "2022-03-22"^^xsd:date)
DataPropertyAssertion(dcterms:modified <http://www.w3.org/ns/dcat> "2022-05-23"^^xsd:date)
DataPropertyAssertion(dcterms:modified <http://www.w3.org/ns/dcat> "2023-01-05"^^xsd:date)
DataPropertyAssertion(dcat:version <http://www.w3.org/ns/dcat> "3")


ClassAssertion(foaf:Person _:genid2147483648)
ClassAssertion(foaf:Person _:genid2147483649)
ClassAssertion(foaf:Person _:genid2147483650)
ClassAssertion(foaf:Person _:genid2147483651)
ClassAssertion(foaf:Person _:genid2147483652)
ClassAssertion(foaf:Person _:genid2147483653)
ClassAssertion(foaf:Person _:genid2147483654)
ClassAssertion(foaf:Person _:genid2147483655)
ClassAssertion(foaf:Person _:genid2147483656)
ClassAssertion(foaf:Person _:genid2147483657)
ClassAssertion(foaf:Person _:genid2147483658)
ClassAssertion(foaf:Person _:genid2147483659)
ClassAssertion(org:Organization _:genid2147483660)
ObjectPropertyAssertion(foaf:homepage _:genid2147483648 <https://w3id.org/people/ralbertoni/>)
ObjectPropertyAssertion(foaf:homepage _:genid2147483651 <https://agbeltran.github.io>)
ObjectPropertyAssertion(foaf:homepage _:genid2147483654 <http://www.asahi-net.or.jp/~ax2s-kmtn/>)
ObjectPropertyAssertion(foaf:homepage _:genid2147483655 <https://jakub.klímek.com/>)
ObjectPropertyAssertion(foaf:homepage _:genid2147483659 <http://makxdekkers.com/>)
ObjectPropertyAssertion(foaf:homepage _:genid2147483660 <https://www.w3.org/>)
ObjectPropertyAssertion(foaf:homepage _:genid2147483732 <http://www.deri.ie/>)
ObjectPropertyAssertion(foaf:homepage _:genid2147483733 <http://ec.europa.eu/dgs/informatics/>)
ObjectPropertyAssertion(foaf:homepage _:genid2147483734 <http://stfc.ac.uk>)
ObjectPropertyAssertion(foaf:homepage _:genid2147483735 <https://www.csiro.au>)
SubObjectPropertyOf(ObjectPropertyChain(dcat:accessService dcat:endpointURL) dcat:accessURL)
AnnotationAssertion(rdfs:seeAlso _:genid2147483648 <https://orcid.org/0000-0001-5648-2713>)
AnnotationAssertion(foaf:name _:genid2147483648 "Riccardo Albertoni")
AnnotationAssertion(foaf:name _:genid2147483649 "David Browning")
AnnotationAssertion(rdfs:seeAlso _:genid2147483650 <https://orcid.org/0000-0002-3884-3420>)
AnnotationAssertion(org:memberOf _:genid2147483650 _:genid2147483735)
AnnotationAssertion(foaf:name _:genid2147483650 "Simon J D Cox")
AnnotationAssertion(foaf:workInfoHomepage _:genid2147483650 <http://people.csiro.au/Simon-Cox>)
AnnotationAssertion(rdfs:seeAlso _:genid2147483651 <https://orcid.org/0000-0003-3499-8262>)
AnnotationAssertion(org:memberOf _:genid2147483651 _:genid2147483734)
AnnotationAssertion(foaf:name _:genid2147483651 "Alejandra Gonzalez-Beltran")
AnnotationAssertion(rdfs:seeAlso _:genid2147483652 <https://orcid.org/0000-0001-9300-2694>)
AnnotationAssertion(foaf:name _:genid2147483652 "Andrea Perego")
AnnotationAssertion(foaf:name _:genid2147483653 "Peter Winstanley")
AnnotationAssertion(foaf:name _:genid2147483654 "Shuji Kamitsuna")
AnnotationAssertion(rdfs:seeAlso _:genid2147483655 <https://jakub.klímek.com/#me>)
AnnotationAssertion(foaf:name _:genid2147483655 "Jakub Klímek")
AnnotationAssertion(org:memberOf _:genid2147483656 _:genid2147483732)
AnnotationAssertion(foaf:name _:genid2147483656 "Fadi Maali")
AnnotationAssertion(foaf:name _:genid2147483657 "Anna Odgaard Ingram")
AnnotationAssertion(org:memberOf _:genid2147483658 _:genid2147483733)
AnnotationAssertion(foaf:name _:genid2147483658 "Vassilios Peristeras")
AnnotationAssertion(rdfs:seeAlso _:genid2147483659 <http://makxdekkers.com/makxdekkers.rdf#me>)
AnnotationAssertion(foaf:name _:genid2147483659 "Makx Dekkers")
AnnotationAssertion(rdfs:seeAlso _:genid2147483660 <https://www.wikidata.org/entity/Q37033>)
AnnotationAssertion(foaf:name _:genid2147483660 "World Wide Web Consortium (W3C)")
AnnotationAssertion(foaf:name _:genid2147483732 "DERI, NUI Galway")
AnnotationAssertion(foaf:name _:genid2147483733 "European Commission, DG DIGIT")
AnnotationAssertion(foaf:name _:genid2147483734 "Science and Technology Facilities Council, UK")
AnnotationAssertion(foaf:name _:genid2147483735 "Commonwealth Scientific and Industrial Research Organisation")
)